ocaml2zoo/tests/zoo_prefix.ml
@@ -1,4 +1,0 @@
-[@@@zoo.prefix truc]
-
-let test () =
-  ()
