theories/language/state_interp.v
@@ -1,13 +1,11 @@
 From iris.bi Require Import
   lib.fractional.
-From iris.base_logic Require Export
+From iris.base_logic Require Import
   lib.gen_heap.
 
 From zoo Require Import
   prelude.
 From zoo.iris.base_logic Require Import
-  lib.mono_map.
-From zoo.iris.base_logic Require Export
   lib.prophet_map.
 From zoo.iris.program_logic Require Export
   wp.
@@ -15,22 +13,25 @@ From zoo.iris Require Import
   diaframe.
 From zoo.language Require Export
   language.
+From zoo.language Require Import
+  notations.
 From zoo Require Import
   options.
 
+Implicit Types hdr : header.
 Implicit Types σ : state.
 Implicit Types κ : list observation.
 
 Class ZooGpre Σ := {
   #[global] zoo_Gpre_inv_Gpre :: invGpreS Σ ;
-  #[local] zoo_Gpre_headers_G :: MonoMapG Σ location header ;
+  #[local] zoo_Gpre_headers_G :: gen_heapGpreS location header Σ ;
   #[local] zoo_Gpre_heap_Gpre :: gen_heapGpreS location val Σ ;
   #[local] zoo_Gpre_prophecy_Gpre :: ProphetMapGpre Σ prophet_id (val * val) ;
 }.
 
 Definition zoo_Σ := #[
   invΣ ;
-  mono_map_Σ location header ;
+  gen_heapΣ location header ;
   gen_heapΣ location val ;
   prophet_map_Σ prophet_id (val * val)
 ].
@@ -43,18 +44,17 @@ Qed.
 
 Class ZooG Σ := {
   zoo_G_inv_G : invGS Σ ;
-  #[local] zoo_G_headers_G :: MonoMapG Σ location header ;
-  zoo_G_headers : gname ;
-  #[global] zoo_G_heap_G :: gen_heapGS location val Σ ;
-  #[global] zoo_G_prophecy_map_G :: ProphetMapG Σ prophet_id (val * val) ;
+  #[local] zoo_G_headers_G :: gen_heapGS location header Σ ;
+  #[local] zoo_G_heap_G :: gen_heapGS location val Σ ;
+  #[local] zoo_G_prophecy_map_G :: ProphetMapG Σ prophet_id (val * val) ;
 }.
-#[global] Arguments Build_ZooG _ {_ _} _ {_ _} : assert.
+#[global] Arguments Build_ZooG _ {_ _ _ _} : assert.
 
 Section zoo_G.
   Context `{zoo_G : !ZooG Σ}.
 
   Definition zoo_state_interp (_ : nat) σ κ : iProp Σ :=
-    mono_map_auth zoo_G_headers (DfracOwn 1) σ.(state_headers) ∗
+    gen_heap_interp σ.(state_headers) ∗
     gen_heap_interp σ.(state_heap) ∗
     prophet_map_interp κ σ.(state_prophets).
   #[global] Instance zoo_G_iris_G : IrisG zoo Σ := {
@@ -67,7 +67,20 @@ Section zoo_G.
   }.
 
   Definition has_header l hdr :=
-    mono_map_elem zoo_G_headers l hdr.
+    pointsto l DfracDiscarded hdr.
+
+  Definition meta_token :=
+    meta_token (V := header).
+
+  Definition meta :=
+    @meta location _ _ header _ _.
+  #[global] Arguments meta {_ _ _} _ _ _ : assert.
+
+  Definition pointsto :=
+    pointsto (V := val).
+
+  Definition prophet_model :=
+    prophet_model.
 End zoo_G.
 
 Notation "l ↦ₕ hdr" := (
@@ -77,7 +90,7 @@ Notation "l ↦ₕ hdr" := (
 ) : bi_scope.
 
 Notation "l ↦ dq v" := (
-  pointsto (L := location) (V := val) l dq v%V
+  pointsto l dq v%V
 )(at level 20,
   dq custom dfrac at level 1,
   format "l  ↦ dq  v"
@@ -88,6 +101,13 @@ Notation "l ↦∗ dq vs" :=
 ( at level 20,
   dq custom dfrac at level 1,
   format "l  ↦∗ dq  vs"
+) : bi_scope.
+
+Notation "l ↦ᵣ dq v" := (
+  pointsto (location_add l (in_type "__ref__" 0)) dq v%V
+)(at level 20,
+  dq custom dfrac at level 1,
+  format "l  ↦ᵣ dq  v"
 ) : bi_scope.
 
 Section zoo_G.
@@ -103,6 +123,262 @@ Section zoo_G.
   Proof.
     apply _.
   Qed.
+
+  Lemma has_header_agree l hdr1 hdr2 :
+    l ↦ₕ hdr1 -∗
+    l ↦ₕ hdr2 -∗
+    ⌜hdr1 = hdr2⌝.
+  Proof.
+    apply pointsto_agree.
+  Qed.
+
+  #[global] Instance meta_token_timeless l N :
+    Timeless (meta_token l N).
+  Proof.
+    apply _.
+  Qed.
+  #[global] Instance meta_timeless `{Countable A} l N (x : A) :
+    Timeless (meta l N x).
+  Proof.
+    apply _.
+  Qed.
+  #[global] Instance meta_persistent `{Countable A} l N (x : A) :
+    Persistent (meta l N x).
+  Proof.
+    apply _.
+  Qed.
+
+  Lemma meta_token_difference l E1 E2 :
+    E1 ⊆ E2 →
+    meta_token l E2 ⊣⊢
+      meta_token l E1 ∗
+      meta_token l (E2 ∖ E1).
+  Proof.
+    apply meta_token_difference.
+  Qed.
+
+  Lemma meta_set `{Countable A} E l (x : A) N :
+    ↑ N ⊆ E →
+    meta_token l E ⊢ |==>
+    meta l N x.
+  Proof.
+    intros. apply bi.wand_entails', meta_set; done.
+  Qed.
+  Lemma meta_agree `{Countable A} l i (x1 x2 : A) :
+    meta l i x1 -∗
+    meta l i x2 -∗
+    ⌜x1 = x2⌝.
+  Proof.
+    apply meta_agree.
+  Qed.
+
+  #[global] Instance pointsto_timeless l dq v :
+    Timeless (l ↦{dq} v).
+  Proof.
+    apply _.
+  Qed.
+  #[global] Instance pointsto_fractional l v :
+    Fractional (λ q, l ↦{#q} v)%I.
+  Proof.
+    apply _.
+  Qed.
+  #[global] Instance pointsto_as_fractional l q v :
+    AsFractional (l ↦{#q} v) (λ q, l ↦{#q} v)%I q.
+  Proof.
+    apply _.
+  Qed.
+  #[global] Instance pointsto_persistent l v :
+    Persistent (l ↦□ v).
+  Proof.
+    apply _.
+  Qed.
+
+  Lemma pointsto_valid l dq v :
+    l ↦{dq} v ⊢
+    ⌜✓ dq⌝.
+  Proof.
+    apply bi.wand_entails', pointsto_valid.
+  Qed.
+  Lemma pointsto_combine l dq1 v1 dq2 v2 :
+    l ↦{dq1} v1 -∗
+    l ↦{dq2} v2 -∗
+      ⌜v1 = v2⌝ ∗
+      l ↦{dq1 ⋅ dq2} v1.
+  Proof.
+    rewrite comm. apply pointsto_combine.
+  Qed.
+  Lemma pointsto_valid_2 l dq1 v1 dq2 v2 :
+    l ↦{dq1} v1 -∗
+    l ↦{dq2} v2 -∗
+    ⌜✓ (dq1 ⋅ dq2) ∧ v1 = v2⌝.
+  Proof.
+    apply pointsto_valid_2.
+  Qed.
+  Lemma pointsto_agree l dq2 v1 dq1 v2 :
+    l ↦{dq1} v1 -∗
+    l ↦{dq2} v2 -∗
+    ⌜v1 = v2⌝.
+  Proof.
+    apply pointsto_agree.
+  Qed.
+  Lemma pointsto_dfrac_ne l1 dq1 v1 l2 dq2 v2 :
+    ¬ ✓ (dq1 ⋅ dq2) →
+    l1 ↦{dq1} v1 -∗
+    l2 ↦{dq2} v2 -∗
+    ⌜l1 ≠ l2⌝.
+  Proof.
+    apply pointsto_frac_ne.
+  Qed.
+  Lemma pointsto_ne l1 v1 l2 dq2 v2 :
+    l1 ↦ v1 -∗
+    l2 ↦{dq2} v2 -∗
+    ⌜l1 ≠ l2⌝.
+  Proof.
+    apply pointsto_ne.
+  Qed.
+  Lemma pointsto_exclusive l v1 v2 :
+    l ↦ v1 -∗
+    l ↦ v2 -∗
+    False.
+  Proof.
+    iIntros "H1 H2".
+    iDestruct (pointsto_ne with "H1 H2") as %?. done.
+  Qed.
+  Lemma pointsto_persist l dq v :
+    l ↦{dq} v ⊢ |==>
+    l ↦□ v.
+  Proof.
+    apply bi.wand_entails', pointsto_persist.
+  Qed.
+
+  #[global] Instance pointsto_combine_sep_gives l dq1 v1 dq2 v2 :
+    CombineSepGives (l ↦{dq1} v1) (l ↦{dq2} v2) ⌜✓ (dq1 ⋅ dq2) ∧ v1 = v2⌝
+  | 30.
+  Proof.
+    apply _.
+  Qed.
+  #[global] Instance pointsto_combine_as l dq1 dq2 v1 v2 :
+    CombineSepAs (l ↦{dq1} v1) (l ↦{dq2} v2) (l ↦{dq1 ⋅ dq2} v1)
+  | 60.
+  Proof.
+    apply _.
+  Qed.
+  #[global] Instance frame_pointsto p l v q1 q2 q :
+    FrameFractionalQp q1 q2 q →
+    Frame p (l ↦{#q1} v) (l ↦{#q2} v) (l ↦{#q} v)
+  | 5.
+  Proof.
+    apply _.
+  Qed.
+
+  #[global] Instance prophet_model_timeless pid prophs :
+    Timeless (prophet_model pid prophs).
+  Proof.
+    apply _.
+  Qed.
+
+  Lemma prophet_model_exclusive pid prophs1 prophs2 :
+    prophet_model pid prophs1 -∗
+    prophet_model pid prophs2 -∗
+    False.
+  Proof.
+    apply prophet_model_exclusive.
+  Qed.
+
+  #[local] Lemma big_sepM_heap_array (Φ : location → val → iProp Σ) l vs :
+    ([∗ map] l' ↦ v ∈ heap_array l vs, Φ l' v) ⊢
+    [∗ list] i ↦ v ∈ vs, Φ (l +ₗ i) v.
+  Proof.
+    iInduction vs as [| v vs] "IH" forall (l) => /=; first iSteps.
+    iIntros "H".
+    rewrite big_sepM_insert.
+    { clear. apply eq_None_ne_Some. intros v (k & Hk & Hl & _)%heap_array_lookup.
+      rewrite -{1}(location_add_0 l) in Hl. naive_solver lia.
+    }
+    rewrite location_add_0. iSteps.
+    setoid_rewrite Nat2Z.inj_succ. setoid_rewrite <- Z.add_1_l. setoid_rewrite <- location_add_assoc. iSteps.
+  Qed.
+
+  Lemma state_interp_alloc {nt σ κ} l tag vs :
+    σ.(state_headers) !! l = None →
+    ( ∀ i,
+      i < length vs →
+      σ.(state_heap) !! (l +ₗ i) = None
+    ) →
+    state_interp nt σ κ ⊢ |==>
+      let hdr := Header tag (length vs) in
+      state_interp nt (state_alloc l hdr vs σ) κ ∗
+      l ↦ₕ hdr ∗
+      meta_token l ⊤ ∗
+      l ↦∗ vs.
+  Proof.
+    iIntros "%Hheaders_lookup %Hheap_lookup (Hheaders & Hheap & $)".
+    iMod (gen_heap_alloc with "Hheaders") as "($ & Hhdr & $)"; first done.
+    iMod (gen_heap.pointsto_persist with "Hhdr") as "$".
+    iMod (gen_heap_alloc_big _ (heap_array _ _) with "Hheap") as "($ & Hl & _)".
+    { apply heap_array_map_disjoint. done. }
+    rewrite big_sepM_heap_array. iSteps.
+  Qed.
+  Lemma state_interp_has_header_valid nt σ κ l hdr :
+    state_interp nt σ κ -∗
+    l ↦ₕ hdr -∗
+    ⌜σ.(state_headers) !! l = Some hdr⌝.
+  Proof.
+    iIntros "(Hheaders & _ & _) Hhdr".
+    iApply (gen_heap_valid with "Hheaders Hhdr").
+  Qed.
+  Lemma state_interp_pointsto_valid nt σ κ l dq v :
+    state_interp nt σ κ -∗
+    l ↦{dq} v -∗
+    ⌜σ.(state_heap) !! l = Some v⌝.
+  Proof.
+    iIntros "(_ & Hheap & _) Hl".
+    iApply (gen_heap_valid with "Hheap Hl").
+  Qed.
+  Lemma state_interp_pointstos_valid nt σ κ l dq vs :
+    state_interp nt σ κ -∗
+    l ↦∗{dq} vs -∗
+    ⌜ ∀ (i : nat) v,
+      vs !! i = Some v →
+      σ.(state_heap) !! (l +ₗ i) = Some v
+    ⌝.
+  Proof.
+    iIntros "(_ & Hheap & _) Hl %i %v %Hvs_lookup".
+    iDestruct (big_sepL_lookup with "Hl") as "Hl"; first done.
+    iApply (gen_heap_valid with "Hheap Hl").
+  Qed.
+  Lemma state_interp_pointsto_update {nt σ κ l w} v :
+    state_interp nt σ κ -∗
+    l ↦ w ==∗
+      state_interp nt (state_update_heap (insert l v) σ) κ ∗
+      l ↦ v.
+  Proof.
+    iIntros "($ & Hheap & $) Hl".
+    iApply (gen_heap_update with "Hheap Hl").
+  Qed.
+  Lemma state_interp_prophet_new {nt σ κ} pid :
+    pid ∉ σ.(state_prophets) →
+    state_interp nt σ κ ⊢ |==>
+      ∃ prophs,
+      state_interp nt (state_update_prophets ({[pid]} ∪.) σ) κ ∗
+      prophet_model pid prophs.
+  Proof.
+    iIntros "%Hpid ($ & $ & Hκ)".
+    iMod (prophet_map_new with "Hκ") as "(Hκ & Hpid)"; first done.
+    iSteps.
+  Qed.
+  Lemma state_interp_prophet_resolve nt σ κ pid proph prophs :
+    state_interp nt σ ((pid, proph) :: κ) -∗
+    prophet_model pid prophs ==∗
+      ∃ prophs',
+      ⌜prophs = proph :: prophs'⌝ ∗
+      state_interp nt σ κ ∗
+      prophet_model pid prophs'.
+  Proof.
+    iIntros "($ & $ & Hκ) Hpid".
+    iMod (prophet_map_resolve with "Hκ Hpid") as "(%prophs' & -> & Hκ & Hpid)".
+    iSteps.
+  Qed.
 End zoo_G.
 
 Lemma zoo_init `{zoo_Gpre : !ZooGpre Σ} `{inv_G : !invGS Σ} nt σ κ :
@@ -110,10 +386,10 @@ Lemma zoo_init `{zoo_Gpre : !ZooGpre Σ} `{inv_G : !invGS Σ} nt σ κ :
     ∃ zoo_G : ZooG Σ,
     state_interp nt σ κ.
 Proof.
-  iMod mono_map_alloc as (γ_headers) "Hheaders".
+  iMod (gen_heap_init σ.(state_headers)) as (?) "(Hheaders & _)".
   iMod (gen_heap_init σ.(state_heap)) as (?) "(Hσ & _)".
   iMod (prophet_map_init κ σ.(state_prophets)) as "(% & Hκ)".
-  iExists (Build_ZooG Σ γ_headers). iFrame. iSteps.
+  iExists (Build_ZooG Σ). iFrame. iSteps.
 Qed.
 Lemma zoo_init' `{zoo_Gpre : !ZooGpre Σ} `{inv_G : !invGS Σ} σ κ :
   ⊢ |==>
@@ -123,4 +399,9 @@ Proof.
   apply zoo_init.
 Qed.
 
+#[global] Opaque zoo_state_interp.
 #[global] Opaque has_header.
+#[global] Opaque meta_token.
+#[global] Opaque meta.
+#[global] Opaque pointsto.
+#[global] Opaque prophet_model.
