theories/saturn/mpmc_bqueue.v
@@ -2,34 +2,38 @@
    https://github.com/ocaml-multicore/saturn/pull/83
 *)
 
+From iris.base_logic Require Import
+  lib.ghost_map.
+
 From zoo Require Import
   prelude.
+From zoo.iris.base_logic Require Import
+  lib.mono_list
+  lib.auth_nat_max
+  lib.twins
+  lib.saved_pred.
 From zoo.language Require Import
   notations
   diaframe.
 From zoo.std Require Import
-  option.
+  option
+  xchain.
 From zoo.saturn Require Export
   base.
 From zoo Require Import
   options.
 
+Implicit Types b : bool.
+Implicit Types l front node back new_back : location.
+Implicit Types hist past nodes : list location.
 Implicit Types v t : val.
 Implicit Types vs : list val.
 
-#[local] Notation "'node_next'" := (
-  in_type "node" 0
-)(in custom zoo_field
-).
-#[local] Notation "'node_data'" := (
-  in_type "node" 1
-)(in custom zoo_field
-).
-#[local] Notation "'node_capacity'" := (
+#[local] Notation "'xchain_index'" := (
   in_type "node" 2
 )(in custom zoo_field
 ).
-#[local] Notation "'node_count'" := (
+#[local] Notation "'xchain_capacity'" := (
   in_type "node" 3
 )(in custom zoo_field
 ).
@@ -47,13 +51,9 @@ Implicit Types vs : list val.
 )(in custom zoo_field
 ).
 
-#[local] Definition node_create : val :=
-  fun: "v1" "v2" "v3" "v4" =>
-    { "v1", "v2", "v3", "v4" }.
-
 Definition mpmc_bqueue_create : val :=
   fun: "cap" =>
-    let: "front" := node_create () () "cap" #0 in
+    let: "front" := { (), (), #0, "cap" } in
     { "cap", "front", "front" }.
 
 Definition mpmc_bqueue_capacity : val :=
@@ -62,56 +62,50 @@ Definition mpmc_bqueue_capacity : val :=
 
 Definition mpmc_bqueue_is_empty : val :=
   fun: "t" =>
-    "t".{front}.{node_next} = ().
+    "t".{front}.{xchain_next} = ().
 
 #[local] Definition mpmc_bqueue_fix_back : val :=
   rec: "mpmc_bqueue_fix_back" "t" "back" "new_back" =>
-    if: "new_back".{node_next} = () and ~ CAS "t".[back] "back" "new_back" then
+    if: "new_back".{xchain_next} = () and ~ CAS "t".[back] "back" "new_back" then
       "mpmc_bqueue_fix_back" "t" "t".{back} "new_back".
-#[local] Definition mpmc_bqueue_push_aux : val :=
-  rec: "mpmc_bqueue_push_aux" "t" "back" "new_back" "cap" =>
+#[local] Definition mpmc_bqueue_do_push : val :=
+  rec: "mpmc_bqueue_do_push" "t" "back" "new_back" "cap" =>
     if: "cap" = #0 then (
-      let: "cap" := "t".{capacity} - ("back".{node_count} - "t".{front}.{node_count}) in
+      let: "cap" := "t".{capacity} - ("back".{xchain_index} - "t".{front}.{xchain_index}) in
       if: "cap" ≤ #0 then (
         #false
       ) else (
-        "back" <-{node_capacity} "cap" ;;
-        "mpmc_bqueue_push_aux" "t" "back" "new_back" "cap"
+        "back" <-{xchain_capacity} "cap" ;;
+        "mpmc_bqueue_do_push" "t" "back" "new_back" "cap"
       )
     ) else (
-      "new_back" <-{node_capacity} "cap" - #1 ;;
-      "new_back" <-{node_count} #1 + "back".{node_count} ;;
-      if: CAS "back".[node_next] () "new_back" then (
+      "new_back" <-{xchain_capacity} "cap" - #1 ;;
+      "new_back" <-{xchain_index} #1 + "back".{xchain_index} ;;
+      if: CAS "back".[xchain_next] () "new_back" then (
         mpmc_bqueue_fix_back "t" "back" "new_back" ;;
         #true
       ) else (
-        let: "back" := "back".{node_next} in
-        "mpmc_bqueue_push_aux" "t" "back" "new_back" "back".{node_capacity}
+        let: "back" := "back".{xchain_next} in
+        "mpmc_bqueue_do_push" "t" "back" "new_back" "back".{xchain_capacity}
       )
     ).
 Definition mpmc_bqueue_push : val :=
   fun: "t" "v" =>
-    let: "new_back" := node_create () "v" #0 #0 in
+    let: "new_back" := { (), "v", #0, #0 } in
     let: "back" := "t".{back} in
-    mpmc_bqueue_push_aux "t" "back" "new_back" "back".{node_capacity}.
-
-#[local] Definition mpmc_queue_do_push : val :=
-  rec: "mpmc_queue_do_push" "node" "new_back" =>
-    let: "node'" := "node".{node_next} in
-    ifnot: "node'" = () and CAS "node".[node_next] () "new_back" then
-      "mpmc_queue_do_push" "node'" "new_back".
+    mpmc_bqueue_do_push "t" "back" "new_back" "back".{xchain_capacity}.
 
 Definition mpmc_bqueue_pop : val :=
   rec: "mpmc_bqueue_pop" "t" =>
     let: "old_front" := "t".{front} in
-    let: "front" := "old_front".{node_next} in
+    let: "front" := "old_front".{xchain_next} in
     if: "front" = () then (
       §None
     ) else (
       if: CAS "t".[front] "old_front" "front" then (
-        let: "v" := "front".{node_data} in
-        "front" <-{node_data} () ;;
-        ‘Some{ "v" }
+        let: "v" := "front".{xchain_data} in
+        "front" <-{xchain_data} () ;;
+        ‘Some( "v" )
       ) else (
         Yield ;;
         "mpmc_bqueue_pop" "t"
@@ -119,33 +113,266 @@ Definition mpmc_bqueue_pop : val :=
     ).
 
 Class MpmcBqueueG Σ `{zoo_G : !ZooG Σ} := {
+  #[local] mpmc_bqueue_G_history_G :: MonoListG Σ location ;
+  #[local] mpmc_bqueue_G_front_G :: AuthNatMaxG Σ ;
+  #[local] mpmc_bqueue_G_model_G :: TwinsG Σ (leibnizO (list val)) ;
+  #[local] mpmc_bqueue_G_waiters_G :: ghost_mapG Σ gname nat ;
+  #[local] mpmc_bqueue_G_saved_pred_G :: SavedPredG Σ bool ;
 }.
 
 Definition mpmc_bqueue_Σ := #[
+  mono_list_Σ location ;
+  auth_nat_max_Σ ;
+  twins_Σ (leibnizO (list val)) ;
+  ghost_mapΣ gname nat ;
+  saved_pred_Σ bool
 ].
 #[global] Instance subG_mpmc_bqueue_Σ Σ `{zoo_G : !ZooG Σ} :
   subG mpmc_bqueue_Σ Σ →
   MpmcBqueueG Σ.
 Proof.
+  solve_inG.
 Qed.
 
 Section mpmc_bqueue_G.
   Context `{mpmc_bqueue_G : MpmcBqueueG Σ}.
 
-  Definition mpmc_bqueue_inv t (ι : namespace) (cap : nat) : iProp Σ.
-  Proof. Admitted.
+  Record mpmc_bqueue_meta := {
+    mpmc_bqueue_meta_capacity : nat ;
+    mpmc_bqueue_meta_history : gname ;
+    mpmc_bqueue_meta_front : gname ;
+    mpmc_bqueue_meta_model : gname ;
+    mpmc_bqueue_meta_waiters : gname ;
+  }.
 
-  Definition mpmc_bqueue_model t vs : iProp Σ.
-  Proof. Admitted.
+  #[local] Instance mpmc_bqueue_meta_eq_dec : EqDecision mpmc_bqueue_meta :=
+    ltac:(solve_decision).
+  #[local] Instance mpmc_bqueue_meta_countable :
+    Countable mpmc_bqueue_meta.
+  Proof.
+    pose encode γ := (
+      γ.(mpmc_bqueue_meta_capacity),
+      γ.(mpmc_bqueue_meta_history),
+      γ.(mpmc_bqueue_meta_front),
+      γ.(mpmc_bqueue_meta_model),
+      γ.(mpmc_bqueue_meta_waiters)
+    ).
+    pose decode := λ '(cap, γ_history, γ_front, γ_model, γ_waiters), {|
+      mpmc_bqueue_meta_capacity := cap ;
+      mpmc_bqueue_meta_history := γ_history ;
+      mpmc_bqueue_meta_front := γ_front ;
+      mpmc_bqueue_meta_model := γ_model ;
+      mpmc_bqueue_meta_waiters := γ_waiters ;
+    |}.
+    refine (inj_countable' encode decode _). intros []. done.
+  Qed.
+
+  #[local] Definition mpmc_bqueue_history_auth' γ_history hist :=
+    mono_list_auth γ_history (DfracOwn 1) hist.
+  #[local] Definition mpmc_bqueue_history_auth γ hist :=
+    mpmc_bqueue_history_auth' γ.(mpmc_bqueue_meta_history) hist.
+  #[local] Definition mpmc_bqueue_history_elem γ i node :=
+    mono_list_elem γ.(mpmc_bqueue_meta_history) i node.
+
+  #[local] Definition mpmc_bqueue_front_auth' γ_front i :=
+    auth_nat_max_auth γ_front (DfracOwn 1) i.
+  #[local] Definition mpmc_bqueue_front_auth γ i :=
+    mpmc_bqueue_front_auth' γ.(mpmc_bqueue_meta_front) i.
+  #[local] Definition mpmc_bqueue_front_lb γ i :=
+    auth_nat_max_lb γ.(mpmc_bqueue_meta_front) i.
+
+  #[local] Definition mpmc_bqueue_model₁' γ_model vs :=
+    twins_twin1 γ_model (DfracOwn 1) vs.
+  #[local] Definition mpmc_bqueue_model₁ γ vs :=
+    mpmc_bqueue_model₁' γ.(mpmc_bqueue_meta_model) vs.
+  #[local] Definition mpmc_bqueue_model₂' γ_model vs :=
+    twins_twin2 γ_model vs.
+  #[local] Definition mpmc_bqueue_model₂ γ vs :=
+    mpmc_bqueue_model₂' γ.(mpmc_bqueue_meta_model) vs.
+
+  #[local] Definition mpmc_bqueue_waiters_auth' γ_waiters waiters :=
+    ghost_map_auth γ_waiters 1 waiters.
+  #[local] Definition mpmc_bqueue_waiters_auth γ waiters :=
+    mpmc_bqueue_waiters_auth' γ.(mpmc_bqueue_meta_waiters) waiters.
+  #[local] Definition mpmc_bqueue_waiters_frag γ waiter i :=
+    ghost_map_elem γ.(mpmc_bqueue_meta_waiters) waiter (DfracOwn 1) i.
+
+  #[local] Definition mpmc_bqueue_waiter_au γ ι (Ψ : bool → iProp Σ) : iProp Σ :=
+    AU <{
+      ∃∃ vs,
+      mpmc_bqueue_model₁ γ vs
+    }> @ ⊤ ∖ ↑ι, ∅ <{
+      mpmc_bqueue_model₁ γ vs
+    , COMM
+      Ψ (bool_decide (vs = []))
+    }>.
+  #[local] Definition mpmc_bqueue_waiter γ ι past waiter i : iProp Σ :=
+    ∃ Ψ,
+    saved_pred waiter Ψ ∗
+    if decide (i < length past) then
+      Ψ false
+    else
+      mpmc_bqueue_waiter_au γ ι Ψ.
+
+  #[local] Definition mpmc_bqueue_inv_inner l γ ι : iProp Σ :=
+    ∃ hist past front nodes back vs waiters,
+    ⌜hist = past ++ front :: nodes⌝ ∗
+    ⌜back ∈ hist⌝ ∗
+    l.[front] ↦ #front ∗
+    l.[back] ↦ #back ∗
+    xchain_model hist () ∗
+    ( [∗ list] node; v ∈ nodes; vs,
+      node.[xchain_data] ↦ v
+    ) ∗
+    ( [∗ list] i ↦ node ∈ past ++ front :: nodes,
+      ∃ cap,
+      ⌜i + cap ≤ length past + γ.(mpmc_bqueue_meta_capacity)⌝ ∗
+      node.[xchain_index] ↦ #i ∗
+      node.[xchain_capacity] ↦ #cap
+    ) ∗
+    mpmc_bqueue_history_auth γ hist ∗
+    mpmc_bqueue_front_auth γ (length past) ∗
+    mpmc_bqueue_model₂ γ vs ∗
+    mpmc_bqueue_waiters_auth γ waiters ∗
+    ( [∗ map] waiter ↦ i ∈ waiters,
+      mpmc_bqueue_waiter γ ι past waiter i
+    ).
+  Definition mpmc_bqueue_inv t ι cap : iProp Σ :=
+    ∃ l γ,
+    ⌜t = #l⌝ ∗
+    ⌜cap = γ.(mpmc_bqueue_meta_capacity)⌝ ∗
+    l.[capacity] ↦□ #cap ∗
+    meta l nroot γ ∗
+    inv ι (mpmc_bqueue_inv_inner l γ ι).
+
+  Definition mpmc_bqueue_model t vs : iProp Σ :=
+    ∃ l γ,
+    ⌜t = #l⌝ ∗
+    meta l nroot γ ∗
+    mpmc_bqueue_model₁ γ vs.
 
   #[global] Instance mpmc_bqueue_model_timeless t vs :
     Timeless (mpmc_bqueue_model t vs).
   Proof.
-  Admitted.
+    apply _.
+  Qed.
   #[global] Instance mpmc_bqueue_inv_persistent t ι cap :
     Persistent (mpmc_bqueue_inv t ι cap).
   Proof.
-  Admitted.
+    apply _.
+  Qed.
+
+  #[local] Lemma mpmc_bqueue_history_alloc front :
+    ⊢ |==>
+      ∃ γ_hist,
+      mpmc_bqueue_history_auth' γ_hist [front].
+  Proof.
+    apply mono_list_alloc.
+  Qed.
+  #[local] Lemma mpmc_bqueue_history_elem_get {γ hist} i node :
+    hist !! i = Some node →
+    mpmc_bqueue_history_auth γ hist ⊢
+    mpmc_bqueue_history_elem γ i node.
+  Proof.
+    setoid_rewrite mono_list_lb_get. apply mono_list_elem_get.
+  Qed.
+  #[local] Lemma mpmc_bqueue_history_agree γ hist i node :
+    mpmc_bqueue_history_auth γ hist -∗
+    mpmc_bqueue_history_elem γ i node -∗
+    ⌜hist !! i = Some node⌝.
+  Proof.
+    apply mono_list_lookup.
+  Qed.
+  #[local] Lemma mpmc_bqueue_history_update {γ hist} node :
+    mpmc_bqueue_history_auth γ hist ⊢ |==>
+    mpmc_bqueue_history_auth γ (hist ++ [node]).
+  Proof.
+    apply mono_list_update_app.
+  Qed.
+
+  #[local] Lemma mpmc_bqueue_front_alloc :
+    ⊢ |==>
+      ∃ γ_front,
+      mpmc_bqueue_front_auth' γ_front 0.
+  Proof.
+    apply auth_nat_max_alloc.
+  Qed.
+  #[local] Lemma mpmc_bqueue_front_lb_get γ i :
+    mpmc_bqueue_front_auth γ i ⊢
+    mpmc_bqueue_front_lb γ i.
+  Proof.
+    apply auth_nat_max_lb_get.
+  Qed.
+  #[local] Lemma mpmc_bqueue_front_lb_valid γ i1 i2 :
+    mpmc_bqueue_front_auth γ i1 -∗
+    mpmc_bqueue_front_lb γ i2 -∗
+    ⌜i2 ≤ i1⌝.
+  Proof.
+    apply auth_nat_max_lb_valid.
+  Qed.
+  #[local] Lemma mpmc_bqueue_front_update {γ i} i' :
+    i ≤ i' →
+    mpmc_bqueue_front_auth γ i ⊢ |==>
+    mpmc_bqueue_front_auth γ i'.
+  Proof.
+    apply auth_nat_max_update.
+  Qed.
+
+  #[local] Lemma mpmc_bqueue_model_alloc :
+    ⊢ |==>
+      ∃ γ_model,
+      mpmc_bqueue_model₁' γ_model [] ∗
+      mpmc_bqueue_model₂' γ_model [].
+  Proof.
+    apply twins_alloc'.
+  Qed.
+  #[local] Lemma mpmc_bqueue_model_agree γ model1 model2 :
+    mpmc_bqueue_model₁ γ model1 -∗
+    mpmc_bqueue_model₂ γ model2 -∗
+    ⌜model1 = model2⌝.
+  Proof.
+    apply: twins_agree_L.
+  Qed.
+  #[local] Lemma mpmc_bqueue_model_update {γ vs1 vs2} vs :
+    mpmc_bqueue_model₁ γ vs1 -∗
+    mpmc_bqueue_model₂ γ vs2 ==∗
+      mpmc_bqueue_model₁ γ vs ∗
+      mpmc_bqueue_model₂ γ vs.
+  Proof.
+    apply twins_update'.
+  Qed.
+
+  #[local] Lemma mpmc_bqueue_waiters_alloc :
+    ⊢ |==>
+      ∃ γ_waiters,
+      mpmc_bqueue_waiters_auth' γ_waiters ∅.
+  Proof.
+    iMod ghost_map_alloc as "(%γ_waiters & Hwaiters_auth & _)".
+    iSteps.
+  Qed.
+  #[local] Lemma mpmc_bqueue_waiters_lookup γ waiters waiter i :
+    mpmc_bqueue_waiters_auth γ waiters -∗
+    mpmc_bqueue_waiters_frag γ waiter i -∗
+    ⌜waiters !! waiter = Some i⌝.
+  Proof.
+    apply ghost_map_lookup.
+  Qed.
+  #[local] Lemma mpmc_bqueue_waiters_insert {γ waiters} waiter i :
+    waiters !! waiter = None →
+    mpmc_bqueue_waiters_auth γ waiters ⊢ |==>
+      mpmc_bqueue_waiters_auth γ (<[waiter := i]> waiters) ∗
+      mpmc_bqueue_waiters_frag γ waiter i.
+  Proof.
+    iIntros "%Hlookup Hwaiters_auth".
+    iApply (ghost_map_insert with "Hwaiters_auth"); first done.
+  Qed.
+  #[local] Lemma mpmc_bqueue_waiters_delete γ waiters waiter i :
+    mpmc_bqueue_waiters_auth γ waiters -∗
+    mpmc_bqueue_waiters_frag γ waiter i ==∗
+      mpmc_bqueue_waiters_auth γ (delete waiter waiters).
+  Proof.
+    apply ghost_map_delete.
+  Qed.
 
   Lemma mpmc_bqueue_create_spec ι cap :
     (0 ≤ cap)%Z →
@@ -157,7 +384,37 @@ Section mpmc_bqueue_G.
       mpmc_bqueue_model t []
     }}}.
   Proof.
-  Admitted.
+    iIntros "%Hcap %Φ _ HΦ".
+
+    wp_rec.
+
+    wp_block front as "(Hfront_next & Hfront_data & Hfront_index & Hfront_capacity & _)".
+    wp_block l as "Hmeta" "(Hl_capacity & Hl_front & Hl_back & _)".
+    iMod (pointsto_persist with "Hl_capacity") as "#Hcapacity".
+    rewrite -{1 3}(Z2Nat.id cap) //.
+
+    iMod mpmc_bqueue_history_alloc as "(%γ_history & Hhistory_auth)".
+    iMod mpmc_bqueue_front_alloc as "(%γ_front & Hfront_auth)".
+    iMod mpmc_bqueue_model_alloc as "(%γ_model & Hmodel₁ & Hmodel₂)".
+    iMod mpmc_bqueue_waiters_alloc as "(%γ_waiters & Hwaiters_auth)".
+
+    pose γ := {|
+      mpmc_bqueue_meta_capacity := Z.to_nat cap ;
+      mpmc_bqueue_meta_history := γ_history ;
+      mpmc_bqueue_meta_front := γ_front ;
+      mpmc_bqueue_meta_model := γ_model ;
+      mpmc_bqueue_meta_waiters := γ_waiters ;
+    |}.
+
+    iMod (meta_set _ _ γ with "Hmeta") as "#Hmeta"; first done.
+
+    iApply "HΦ".
+    iSplitR "Hmodel₁"; last iSteps.
+    iExists l, γ. iStep 4. iApply inv_alloc.
+    iExists [front], [], front, [], front, [], ∅. iFrame. iSteps.
+    - rewrite elem_of_list_singleton //.
+    - iExists (Z.to_nat cap). iSteps. rewrite big_sepM_empty //.
+  Qed.
 
   Lemma mpmc_bqueue_is_empty_spec t ι cap :
     <<<
