theories/std/array.v
@@ -1,13 +1,12 @@
 From zoo Require Import
   prelude.
-From zoo.iris.bi Require Import
-  big_op.
 From zoo.language Require Import
   notations
   diaframe.
 From zoo.std Require Export
   base.
 From zoo.std Require Import
+  for_upto
   assume
   chunk.
 From zoo Require Import
@@ -18,46 +17,25 @@ Implicit Types l : location.
 Implicit Types v t fn acc : val.
 Implicit Types vs : list val.
 
-#[local] Notation "'size'" := (
-  in_type "t" 0
-)(in custom zoo_field
-).
-#[local] Notation "'data'" := (
-  in_type "t" 1
-)(in custom zoo_field
-).
+Definition array_unsafe_alloc : val :=
+  fun: "sz" =>
+    Alloc #0 "sz".
+Definition array_alloc : val :=
+  fun: "sz" =>
+    assume (#0 ≤ "sz") ;;
+    array_unsafe_alloc "sz".
 
 Definition array_create : val :=
   fun: <> =>
-    chunk_make #1 #0.
-
-Definition array_make : val :=
-  fun: "sz" "v" =>
-    assume (#0 ≤ "sz") ;;
-    let: "t" := chunk_make (#1 + "sz") "v" in
-    "t" <-{size} "sz" ;;
-    "t".
-
-Definition array_initi : val :=
-  fun: "sz" "fn" =>
-    assume (#0 ≤ "sz") ;;
-    let: "t" := chunk_make (#1 + "sz") "sz" in
-    chunk_applyi "t".[data] "sz" (fun: "i" <> => "fn" "i") ;;
-    "t".
-Definition array_init : val :=
-  fun: "sz" "fn" =>
-    array_initi "sz" (fun: <> => "fn" ()).
+    array_unsafe_alloc #0.
 
 Definition array_size : val :=
   fun: "t" =>
-    "t".{size}.
-#[local] Definition array_data : val :=
-  fun: "t" =>
-    "t".[data].
+    GetSize "t".
 
 Definition array_unsafe_get : val :=
   fun: "t" "i" =>
-    !(array_data "t" +ₗ "i").
+    Load "t" "i".
 Definition array_get : val :=
   fun: "t" "i" =>
     assume (#0 ≤ "i") ;;
@@ -66,42 +44,117 @@ Definition array_get : val :=
 
 Definition array_unsafe_set : val :=
   fun: "t" "i" "v" =>
-    array_data "t" +ₗ "i" <- "v".
+    Store "t" "i" "v".
 Definition array_set : val :=
   fun: "t" "i" "v" =>
     assume (#0 ≤ "i") ;;
     assume ("i" < array_size "t") ;;
     array_unsafe_set "t" "i" "v".
 
+Definition array_unsafe_fill_slice : val :=
+  fun: "t" "i" "n" "v" =>
+    for: "j" := #0 to "n" begin
+      array_unsafe_set "t" ("i" + "j") "v"
+    end.
+Definition array_fill_slice : val :=
+  fun: "t" "i" "n" "v" =>
+    let: "sz" := array_size "t" in
+    assume (#0 ≤ "i") ;;
+    assume (#0 ≤ "n") ;;
+    assume ("i" + "n" ≤ "sz") ;;
+    array_unsafe_fill_slice "t" "i" "n" "v".
+Definition array_fill : val :=
+  fun: "t" "v" =>
+    array_unsafe_fill_slice "t" #0 (array_size "t") "v".
+
+Definition array_unsafe_make : val :=
+  fun: "sz" "v" =>
+    let: "t" := array_unsafe_alloc "sz" in
+    array_fill "t" "v" ;;
+    "t".
+Definition array_make : val :=
+  fun: "sz" "v" =>
+    assume (#0 ≤ "sz") ;;
+    array_unsafe_make "sz" "v".
+
+#[local] Definition array_foldli_aux : val :=
+  rec: "array_foldli_aux" "t" "sz" "acc" "fn" "i" =>
+    if: "sz" ≤ "i" then (
+      "acc"
+    ) else (
+      let: "v" := array_unsafe_get "t" "i" in
+      "array_foldli_aux" "t" "sz" ("fn" "acc" "i" "v") "fn" (#1 + "i")
+    ).
 Definition array_foldli : val :=
   fun: "t" "acc" "fn" =>
-    chunk_foldli (array_data "t") (array_size "t") "acc" "fn".
+    array_foldli_aux "t" (array_size "t") "acc" "fn" #0.
 Definition array_foldl : val :=
   fun: "t" "acc" "fn" =>
-    chunk_foldl (array_data "t") (array_size "t") "acc" "fn".
+    array_foldli "t" "acc" (fun: "acc" <> "v" => "fn" "acc" "v").
 
+#[local] Definition array_foldri_aux : val :=
+  rec: "array_foldri_aux" "t" "fn" "acc" "i" =>
+    if: "i" ≤ #0 then (
+      "acc"
+    ) else (
+      let: "i" := "i" - #1 in
+      let: "v" := array_unsafe_get "t" "i" in
+      "array_foldri_aux" "t" "fn" ("fn" "i" "v" "acc") "i"
+    ).
 Definition array_foldri : val :=
   fun: "t" "fn" "acc" =>
-    chunk_foldri (array_data "t") (array_size "t") "fn" "acc".
+    array_foldri_aux "t" "fn" "acc" (array_size "t").
 Definition array_foldr : val :=
   fun: "t" "fn" "acc" =>
-    chunk_foldr (array_data "t") (array_size "t") "fn" "acc".
+    array_foldri "t" (fun: <> => "fn") "acc".
 
 Definition array_iteri : val :=
   fun: "t" "fn" =>
-    chunk_iteri (array_data "t") (array_size "t") "fn".
+    for: "i" := #0 to array_size "t" begin
+      "fn" "i" (array_unsafe_get "t" "i")
+    end.
 Definition array_iter : val :=
   fun: "t" "fn" =>
-    chunk_iter (array_data "t") (array_size "t") "fn".
+    array_iteri "t" (fun: <> => "fn").
 
 Definition array_applyi : val :=
   fun: "t" "fn" =>
-    chunk_applyi (array_data "t") (array_size "t") "fn".
+    array_iteri "t" (fun: "i" "v" => array_unsafe_set "t" "i" ("fn" "i" "v")).
 Definition array_apply : val :=
   fun: "t" "fn" =>
-    chunk_apply (array_data "t") (array_size "t") "fn".
+    array_applyi "t" (fun: <> => "fn").
 
-Definition array_blit : val :=
+Definition array_unsafe_initi : val :=
+  fun: "sz" "fn" =>
+    let: "t" := array_unsafe_alloc "sz" in
+    array_applyi "t" (fun: "i" <> => "fn" "i") ;;
+    "t".
+Definition array_initi : val :=
+  fun: "sz" "fn" =>
+    assume (#0 ≤ "sz") ;;
+    array_unsafe_initi "sz" "fn".
+Definition array_unsafe_init : val :=
+  fun: "sz" "fn" =>
+    array_unsafe_initi "sz" (fun: <> => "fn" ()).
+Definition array_init : val :=
+  fun: "sz" "fn" =>
+    assume (#0 ≤ "sz") ;;
+    array_initi "sz" "fn".
+
+Definition array_mapi : val :=
+  fun: "t" "fn" =>
+    array_unsafe_initi (array_size "t") (fun: "i" => "fn" "i" (array_unsafe_get "i")).
+Definition array_map : val :=
+  fun: "t" "fn" =>
+    array_mapi "t" (fun: <> => "fn").
+
+Definition array_unsafe_copy_slice : val :=
+  fun: "t1" "i1" "t2" "i2" "n" =>
+    for: "i" := #0 to "n" begin
+      let: "v" := array_unsafe_get "t1" ("i1" + "n") in
+      array_unsafe_set "t2" ("i2" + "n") "v"
+    end.
+Definition array_copy_slice : val :=
   fun: "t1" "i1" "t2" "i2" "n" =>
     let: "sz1" := array_size "t1" in
     let: "sz2" := array_size "t2" in
@@ -110,61 +163,95 @@ Definition array_blit : val :=
     assume (#0 ≤ "n") ;;
     assume ("i1" + "n" ≤ "sz1") ;;
     assume ("i2" + "n" ≤ "sz2") ;;
-    chunk_copy (array_data "t1" +ₗ "i1") "n" (array_data "t2" +ₗ "i2").
-
+    array_unsafe_copy_slice "t1" "i1" "t2" "i2" "n".
+Definition array_unsafe_copy : val :=
+  fun: "t1" "t2" "i2" =>
+    array_unsafe_copy_slice "t1" #0 "t2" "i2" (array_size "t1").
 Definition array_copy : val :=
   fun: "t1" "t2" "i2" =>
-    array_blit "t1" #0 "t2" "i2" (array_size "t1").
+    assume (#0 ≤ "i2") ;;
+    assume ("i2" + array_size "t1" ≤ array_size "t2") ;;
+    array_unsafe_copy_slice "t1" "t2" "i2".
 
+Definition array_unsafe_grow : val :=
+  fun: "t" "sz'" "v'" =>
+    let: "sz" := array_size "t" in
+    let: "t'" := array_unsafe_alloc "sz'" in
+    array_unsafe_copy "t" "t'" #0 ;;
+    array_unsafe_fill_slice "t'" "sz" ("sz'" - "sz") "v'" ;;
+    "t'".
 Definition array_grow : val :=
   fun: "t" "sz'" "v'" =>
-    let: "t'" := array_make "sz'" "v'" in
-    array_copy "t" "t'" #0 ;;
-    "t'".
+    assume (array_size "t" ≤ "sz'") ;;
+    array_unsafe_grow "t" "sz'" "v'".
 
+Definition array_unsafe_sub : val :=
+  fun: "t" "i" "n" =>
+    let: "t'" := array_unsafe_alloc "n" in
+    array_unsafe_copy_slice "t" "i" "t'" #0 "n" ;;
+    "t'".
 Definition array_sub : val :=
   fun: "t" "i" "n" =>
-    let: "sz" := array_size "t" in
     assume (#0 ≤ "i") ;;
     assume (#0 ≤ "n") ;;
-    assume ("i" + "n" ≤ "sz") ;;
-    let: "t'" := array_make "n" () in
-    chunk_copy (array_data "t" +ₗ "i") "n" (array_data "t'") ;;
-    "t'".
+    assume ("i" + "n" ≤ array_size "t") ;;
+    array_unsafe_sub "t" "i" "n".
 
+Definition array_unsafe_shrink : val :=
+  fun: "t" "sz'" =>
+    array_unsafe_sub "t" #0 "sz'".
 Definition array_shrink : val :=
-  fun: "t" "n" =>
-    array_sub "t" #0 "n".
+  fun: "t" "sz'" =>
+    assume (#0 ≤ "sz'") ;;
+    assume ("sz'" ≤ array_size "t") ;;
+    array_unsafe_shrink "t" "sz'".
 
 Definition array_clone : val :=
   fun: "t" =>
-    array_shrink "t" (array_size "t").
+    array_unsafe_shrink "t" (array_size "t").
 
-Definition array_fill_slice : val :=
-  fun: "t" "i" "n" "v" =>
-    let: "sz" := array_size "t" in
-    assume (#0 ≤ "i") ;;
-    assume (#0 ≤ "n") ;;
-    assume ("i" + "n" ≤ "sz") ;;
-    chunk_fill (array_data "t" +ₗ "i") "n" "v".
-Definition array_fill : val :=
-  fun: "t" "v" =>
-    array_fill_slice "t" #0 (array_size "t") "v".
-
+Definition array_unsafe_cget : val :=
+  fun: "t" "i" =>
+    array_unsafe_get "t" ("i" `rem` array_size "t").
 Definition array_cget : val :=
   fun: "t" "i" =>
-    chunk_cget (array_data "t") (array_size "t") "i".
+    assume (#0 ≤ "i") ;;
+    array_unsafe_cget "t" "i".
+
+Definition array_unsafe_cset : val :=
+  fun: "t" "i" "v" =>
+    array_unsafe_set "t" ("i" `rem` array_size "t") "v".
 Definition array_cset : val :=
   fun: "t" "i" "v" =>
-    chunk_cset (array_data "t") (array_size "t") "i" "v".
+    assume (#0 ≤ "i") ;;
+    array_unsafe_cset "t" "i" "v".
 
-Definition array_cblit : val :=
+Definition array_unsafe_ccopy_slice : val :=
   fun: "t1" "i1" "t2" "i2" "n" =>
-    chunk_cblit (array_data "t1") (array_size "t1") "i1" (array_data "t2") (array_size "t2") "i2" "n".
+    let: "sz1" := array_size "t1" in
+    let: "sz2" := array_size "t2" in
+    for: "j" := #0 to "n" begin
+      let: "v" := array_unsafe_get "t1" (("i1" + "j") `rem` "sz1") in
+      array_unsafe_set "t2" (("i2" + "j") `rem` "sz2") "v"
+    end.
+Definition array_ccopy_slice : val :=
+  fun: "t1" "i1" "t2" "i2" "n" =>
+    assume (#0 ≤ "i1") ;;
+    assume (#0 ≤ "i2") ;;
+    assume (#0 ≤ "n") ;;
+    assume ("n" ≤ array_size "t1") ;;
+    assume ("n" ≤ array_size "t2") ;;
+    array_unsafe_ccopy_slice "t1" "i1" "t2" "i2" "n".
 
+Definition array_unsafe_ccopy : val :=
+  fun: "t1" "i1" "t2" "i2" =>
+    array_unsafe_ccopy_slice "t1" "i1" "t2" "i2" (array_size "t1").
 Definition array_ccopy : val :=
   fun: "t1" "i1" "t2" "i2" =>
-    array_cblit "t1" "i1" "t2" "i2" (array_size "t1").
+    assume (#0 ≤ "i1") ;;
+    assume (#0 ≤ "i2") ;;
+    assume (array_size "t1" ≤ array_size "t2") ;;
+    array_unsafe_ccopy "t1" "i1" "t2" "i2".
 
 Section zoo_G.
   Context `{zoo_G : !ZooG Σ}.
@@ -173,7 +260,7 @@ Section zoo_G.
     Definition array_inv t (sz : nat) : iProp Σ :=
       ∃ l,
       ⌜t = #l⌝ ∗
-      l.[size] ↦□ #sz.
+      l ↦ₕ Header 0 sz.
 
     #[global] Instance array_inv_timeless t sz :
       Timeless (array_inv t sz).
@@ -188,207 +275,187 @@ Section zoo_G.
   End array_inv.
 
   Section array_slice.
-    Definition array_slice t (sz : nat) i dq vs : iProp Σ :=
+    Definition array_slice t i dq vs : iProp Σ :=
       ∃ l,
       ⌜t = #l⌝ ∗
-      l.[size] ↦□ #sz ∗
-      chunk_model (l.[data] +ₗ i) dq vs.
+      chunk_model (l +ₗ i) dq vs.
 
-    #[global] Instance array_slice_timeless t sz i dq vs :
-      Timeless (array_slice t sz i dq vs).
+    #[global] Instance array_slice_timeless t i dq vs :
+      Timeless (array_slice t i dq vs).
     Proof.
       apply _.
     Qed.
-    #[global] Instance array_slice_persistent t sz i vs :
-      Persistent (array_slice t sz i DfracDiscarded vs).
+    #[global] Instance array_slice_persistent t i vs :
+      Persistent (array_slice t i DfracDiscarded vs).
     Proof.
       apply _.
     Qed.
 
-    #[global] Instance array_slice_fractional t sz i vs :
-      Fractional (λ q, array_slice t sz i (DfracOwn q) vs).
+    #[global] Instance array_slice_fractional t i vs :
+      Fractional (λ q, array_slice t i (DfracOwn q) vs).
     Proof.
       intros q1 q2. iSplit.
-      - iIntros "(%l & -> & #Hsz & Hmodel1 & Hmodel2)". iSteps.
-      - iIntros "((%l & -> & #Hsz & Hmodel1) & (%_l & %Heq & _ & Hmodel2))". injection Heq as <-.
+      - iIntros "(%l & -> & Hmodel1 & Hmodel2)". iSteps.
+      - iIntros "((%l & -> & Hmodel1) & (%_l & %Heq & Hmodel2))". injection Heq as <-.
         iExists l. iSteps.
         iApply chunk_model_fractional. iSteps.
     Qed.
-    #[global] Instance array_slice_as_fractional t sz i q vs :
-      AsFractional (array_slice t sz i (DfracOwn q) vs) (λ q, array_slice t sz i (DfracOwn q) vs) q.
+    #[global] Instance array_slice_as_fractional t i q vs :
+      AsFractional (array_slice t i (DfracOwn q) vs) (λ q, array_slice t i (DfracOwn q) vs) q.
     Proof.
       split; [done | apply _].
     Qed.
 
-    Lemma array_slice_to_inv t sz i dq vs :
-      array_slice t sz i dq vs ⊢
-      array_inv t sz.
-    Proof.
-      iSteps.
-    Qed.
-
-    Lemma array_slice_agree_size t sz1 i1 dq1 vs1 sz2 i2 dq2 vs2 :
-      array_slice t sz1 i1 dq1 vs1 -∗
-      array_slice t sz2 i2 dq2 vs2 -∗
-      ⌜sz1 = sz2⌝.
-    Proof.
-      iIntros "(%l & -> & #Hsz1 & Hmodel1) (%_l & %Heq & #Hsz2 & Hmodel2)". injection Heq as <-.
-      iDestruct (pointsto_agree with "Hsz1 Hsz2") as %[= <-%(inj _)].
-      iSteps.
-    Qed.
-
-    Lemma array_slice_valid t sz i dq vs :
+    Lemma array_slice_valid t i dq vs :
       0 < length vs →
-      array_slice t sz i dq vs ⊢
+      array_slice t i dq vs ⊢
       ⌜✓ dq⌝.
     Proof.
-      iIntros "% (%l & -> & #Hsz & Hmodel)".
+      iIntros "% (%l & -> & Hmodel)".
       iApply (chunk_model_valid with "Hmodel"); first done.
     Qed.
-    Lemma array_slice_combine t i sz1 dq1 vs1 sz2 dq2 vs2 :
+    Lemma array_slice_combine t i dq1 vs1 dq2 vs2 :
       length vs1 = length vs2 →
-      array_slice t sz1 i dq1 vs1 -∗
-      array_slice t sz2 i dq2 vs2 -∗
-        ⌜sz1 = sz2 ∧ vs1 = vs2⌝ ∗
-        array_slice t sz1 i (dq1 ⋅ dq2) vs1.
+      array_slice t i dq1 vs1 -∗
+      array_slice t i dq2 vs2 -∗
+        ⌜vs1 = vs2⌝ ∗
+        array_slice t i (dq1 ⋅ dq2) vs1.
     Proof.
-      iIntros "% (%l & -> & #Hsz1 & Hmodel1) (%_l & %Heq & #Hsz2 & Hmodel2)". injection Heq as <-.
-      iDestruct (pointsto_agree with "Hsz1 Hsz2") as %[= <-%(inj _)].
+      iIntros "% (%l & -> & Hmodel1) (%_l & %Heq & Hmodel2)". injection Heq as <-.
       iDestruct (chunk_model_combine with "Hmodel1 Hmodel2") as "(<- & Hmodel)"; first done.
       iSteps.
     Qed.
-    Lemma array_slice_valid_2 t i sz1 dq1 vs1 sz2 dq2 vs2 :
+    Lemma array_slice_valid_2 t i dq1 vs1 dq2 vs2 :
       0 < length vs1 →
       length vs1 = length vs2 →
-      array_slice t sz1 i dq1 vs1 -∗
-      array_slice t sz2 i dq2 vs2 -∗
-      ⌜sz1 = sz2 ∧ ✓ (dq1 ⋅ dq2) ∧ vs1 = vs2⌝.
+      array_slice t i dq1 vs1 -∗
+      array_slice t i dq2 vs2 -∗
+      ⌜✓ (dq1 ⋅ dq2) ∧ vs1 = vs2⌝.
     Proof.
       iIntros "% % Hslice1 Hslice2".
-      iDestruct (array_slice_combine with "Hslice1 Hslice2") as "((<- & <-) & Hslice)"; first done.
+      iDestruct (array_slice_combine with "Hslice1 Hslice2") as "(<- & Hslice)"; first done.
       iDestruct (array_slice_valid with "Hslice") as %?; done.
     Qed.
-    Lemma array_slice_agree t i sz1 dq1 vs1 sz2 dq2 vs2 :
+    Lemma array_slice_agree t i dq1 vs1 dq2 vs2 :
       length vs1 = length vs2 →
-      array_slice t sz1 i dq1 vs1 -∗
-      array_slice t sz2 i dq2 vs2 -∗
-      ⌜sz1 = sz2 ∧ vs1 = vs2⌝.
+      array_slice t i dq1 vs1 -∗
+      array_slice t i dq2 vs2 -∗
+      ⌜vs1 = vs2⌝.
     Proof.
       iIntros "% Hslice1 Hslice2".
       iDestruct (array_slice_combine with "Hslice1 Hslice2") as "(% & _)"; done.
     Qed.
-    Lemma array_slice_dfrac_ne t1 sz1 i1 dq1 vs1 t2 sz2 i2 dq2 vs2 :
+    Lemma array_slice_dfrac_ne t1 i1 dq1 vs1 t2 i2 dq2 vs2 :
       0 < length vs1 →
       length vs1 = length vs2 →
       ¬ ✓ (dq1 ⋅ dq2) →
-      array_slice t1 sz1 i1 dq1 vs1 -∗
-      array_slice t2 sz2 i2 dq2 vs2 -∗
+      array_slice t1 i1 dq1 vs1 -∗
+      array_slice t2 i2 dq2 vs2 -∗
       ⌜t1 ≠ t2 ∨ i1 ≠ i2⌝.
     Proof.
       rewrite -not_and_r. iIntros "% % % Hslice1 Hslice2" ((-> & ->)).
       iDestruct (array_slice_valid_2 with "Hslice1 Hslice2") as %?; naive_solver.
     Qed.
-    Lemma array_slice_ne t1 sz1 i1 vs1 t2 sz2 i2 dq2 vs2 :
+    Lemma array_slice_ne t1 i1 vs1 t2 i2 dq2 vs2 :
       0 < length vs1 →
       length vs1 = length vs2 →
-      array_slice t1 sz1 i1 (DfracOwn 1) vs1 -∗
-      array_slice t2 sz2 i2 dq2 vs2 -∗
+      array_slice t1 i1 (DfracOwn 1) vs1 -∗
+      array_slice t2 i2 dq2 vs2 -∗
       ⌜t1 ≠ t2 ∨ i1 ≠ i2⌝.
     Proof.
       intros.
       iApply array_slice_dfrac_ne; [done.. | intros []%(exclusive_l _)].
     Qed.
-    Lemma array_slice_exclusive t i sz1 vs1 sz2 vs2 :
+    Lemma array_slice_exclusive t i vs1 vs2 :
       0 < length vs1 →
       length vs1 = length vs2 →
-      array_slice t sz1 i (DfracOwn 1) vs1 -∗
-      array_slice t sz2 i (DfracOwn 1) vs2 -∗
+      array_slice t i (DfracOwn 1) vs1 -∗
+      array_slice t i (DfracOwn 1) vs2 -∗
       False.
     Proof.
       iIntros "% % Hslice1 Hslice2".
       iDestruct (array_slice_valid_2 with "Hslice1 Hslice2") as %?; naive_solver.
     Qed.
-    Lemma array_slice_persist t sz i dq vs :
-      array_slice t sz i dq vs ⊢ |==>
-      array_slice t sz i DfracDiscarded vs.
+    Lemma array_slice_persist t i dq vs :
+      array_slice t i dq vs ⊢ |==>
+      array_slice t i DfracDiscarded vs.
     Proof.
-      iIntros "(%l & -> & #Hsz & Hmodel)".
+      iIntros "(%l & -> & Hmodel)".
       iMod (chunk_model_persist with "Hmodel") as "Hmodel".
       iSteps.
     Qed.
 
-    Lemma array_slice_app t sz i dq vs1 vs2 :
-      array_slice t sz i dq vs1 ∗
-      array_slice t sz (i + length vs1) dq vs2 ⊣⊢
-      array_slice t sz i dq (vs1 ++ vs2).
+    Lemma array_slice_app t i dq vs1 vs2 :
+      array_slice t i dq vs1 ∗
+      array_slice t (i + length vs1) dq vs2 ⊣⊢
+      array_slice t i dq (vs1 ++ vs2).
     Proof.
       iSplit.
-      - iIntros "((%l & -> & #Hsz & Hmodel1) & (%_l & %Heq & _ & Hmodel2))". injection Heq as <-.
+      - iIntros "((%l & -> & Hmodel1) & (%_l & %Heq & Hmodel2))". injection Heq as <-.
         rewrite Nat2Z.inj_add -location_add_assoc.
         iDestruct (chunk_model_app_1 with "Hmodel1 Hmodel2") as "Hmodel"; first done.
         iSteps.
-      - iIntros "(%l & -> & #Hsz & Hmodel)".
+      - iIntros "(%l & -> & Hmodel)".
         iDestruct (chunk_model_app with "Hmodel") as "(Hmodel1 & Hmodel2)".
         iSplitL "Hmodel1"; iExists l; first iSteps.
         rewrite location_add_assoc -Nat2Z.inj_add. iSteps.
     Qed.
-    Lemma array_slice_app_1 t sz i dq sz1 vs1 vs2 :
-      sz1 = length vs1 →
-      array_slice t sz i dq vs1 -∗
-      array_slice t sz (i + sz1) dq vs2 -∗
-      array_slice t sz i dq (vs1 ++ vs2).
+    Lemma array_slice_app_1 t i dq vs1 vs2 :
+      array_slice t i dq vs1 -∗
+      array_slice t (i + length vs1) dq vs2 -∗
+      array_slice t i dq (vs1 ++ vs2).
     Proof.
-      intros ->. rewrite -array_slice_app. iSteps.
+      rewrite -array_slice_app. iSteps.
     Qed.
-    Lemma array_slice_app_2 {t sz i dq vs} vs1 vs2 :
+    Lemma array_slice_app_2 {t i dq vs} vs1 vs2 :
       vs = vs1 ++ vs2 →
-      array_slice t sz i dq vs ⊢
-        array_slice t sz i dq vs1 ∗
-        array_slice t sz (i + length vs1) dq vs2.
+      array_slice t i dq vs ⊢
+        array_slice t i dq vs1 ∗
+        array_slice t (i + length vs1) dq vs2.
     Proof.
       intros ->. rewrite array_slice_app //.
     Qed.
 
-    Lemma array_slice_app3 t sz i dq vs1 vs2 vs3 :
-      array_slice t sz i dq vs1 ∗
-      array_slice t sz (i + length vs1) dq vs2 ∗
-      array_slice t sz (i + length vs1 + length vs2) dq vs3 ⊣⊢
-      array_slice t sz i dq (vs1 ++ vs2 ++ vs3).
+    Lemma array_slice_app3 t i dq vs1 vs2 vs3 :
+      array_slice t i dq vs1 ∗
+      array_slice t (i + length vs1) dq vs2 ∗
+      array_slice t (i + length vs1 + length vs2) dq vs3 ⊣⊢
+      array_slice t i dq (vs1 ++ vs2 ++ vs3).
     Proof.
       rewrite !array_slice_app //.
     Qed.
-    Lemma array_slice_app3_1 t sz dq i1 vs1 i2 vs2 i3 vs3 :
+    Lemma array_slice_app3_1 t dq i1 vs1 i2 vs2 i3 vs3 :
       i2 = i1 + length vs1 →
       i3 = i1 + length vs1 + length vs2 →
-      array_slice t sz i1 dq vs1 -∗
-      array_slice t sz i2 dq vs2 -∗
-      array_slice t sz i3 dq vs3 -∗
-      array_slice t sz i1 dq (vs1 ++ vs2 ++ vs3).
+      array_slice t i1 dq vs1 -∗
+      array_slice t i2 dq vs2 -∗
+      array_slice t i3 dq vs3 -∗
+      array_slice t i1 dq (vs1 ++ vs2 ++ vs3).
     Proof.
       intros -> ->. rewrite -array_slice_app3. iSteps.
     Qed.
-    Lemma array_slice_app3_2 {t sz i dq vs} vs1 vs2 vs3 :
+    Lemma array_slice_app3_2 {t i dq vs} vs1 vs2 vs3 :
       vs = vs1 ++ vs2 ++ vs3 →
-      array_slice t sz i dq vs ⊢
-        array_slice t sz i dq vs1 ∗
-        array_slice t sz (i + length vs1) dq vs2 ∗
-        array_slice t sz (i + length vs1 + length vs2) dq vs3.
+      array_slice t i dq vs ⊢
+        array_slice t i dq vs1 ∗
+        array_slice t (i + length vs1) dq vs2 ∗
+        array_slice t (i + length vs1 + length vs2) dq vs3.
     Proof.
       intros ->. rewrite array_slice_app3 //.
     Qed.
 
-    Lemma array_slice_cons t sz i dq v vs :
-      array_slice t sz i dq (v :: vs) ⊢
-        array_slice t sz i dq [v] ∗
-        array_slice t sz (S i) dq vs.
+    Lemma array_slice_cons t i dq v vs :
+      array_slice t i dq (v :: vs) ⊢
+        array_slice t i dq [v] ∗
+        array_slice t (S i) dq vs.
     Proof.
       rewrite -Nat.add_1_r (array_slice_app_2 [v] vs) //.
     Qed.
 
-    Lemma array_slice_atomize t sz i dq vs :
-      array_slice t sz i dq vs ⊢
+    Lemma array_slice_atomize t i dq vs :
+      array_slice t i dq vs ⊢
       [∗ list] j ↦ v ∈ vs,
-        array_slice t sz (i + j) dq [v].
+        array_slice t (i + j) dq [v].
     Proof.
       iInduction vs as [| v vs] "IH" forall (i); first iSteps.
       iIntros "Hvs".
@@ -398,13 +465,13 @@ Section zoo_G.
       setoid_rewrite Nat.add_succ_comm. iSteps.
     Qed.
 
-    Lemma array_slice_update {t sz i dq vs} j v :
+    Lemma array_slice_update {t i dq vs} j v :
       vs !! j = Some v →
-      array_slice t sz i dq vs ⊢
-        array_slice t sz (i + j) dq [v] ∗
+      array_slice t i dq vs ⊢
+        array_slice t (i + j) dq [v] ∗
         ( ∀ w,
-          array_slice t sz (i + j) dq [w] -∗
-          array_slice t sz i dq (<[j := w]> vs)
+          array_slice t (i + j) dq [w] -∗
+          array_slice t i dq (<[j := w]> vs)
         ).
     Proof.
       iIntros "%Hlookup Hslice".
@@ -416,22 +483,22 @@ Section zoo_G.
       iFrame. iIntros "%w Hslice2".
       iApply (array_slice_app3_1 with "Hslice1 Hslice2 Hslice3"); rewrite take_length /=; lia.
     Qed.
-    Lemma array_slice_lookup_acc {t sz i dq vs} j v :
+    Lemma array_slice_lookup_acc {t i dq vs} j v :
       vs !! j = Some v →
-      array_slice t sz i dq vs ⊢
-        array_slice t sz (i + j) dq [v] ∗
-        ( array_slice t sz (i + j) dq [v] -∗
-          array_slice t sz i dq vs
+      array_slice t i dq vs ⊢
+        array_slice t (i + j) dq [v] ∗
+        ( array_slice t (i + j) dq [v] -∗
+          array_slice t i dq vs
         ).
     Proof.
       iIntros "%Hlookup Hslice".
       iDestruct (array_slice_update with "Hslice") as "(Hv & Hslice)"; first done.
       iSpecialize ("Hslice" $! v). rewrite list_insert_id //. iFrame.
     Qed.
-    Lemma array_slice_lookup {t sz i dq vs} j v :
+    Lemma array_slice_lookup {t i dq vs} j v :
       vs !! j = Some v →
-      array_slice t sz i dq vs ⊢
-      array_slice t sz (i + j) dq [v].
+      array_slice t i dq vs ⊢
+      array_slice t (i + j) dq [v].
     Proof.
       intros. rewrite array_slice_lookup_acc //. iSteps.
     Qed.
@@ -439,20 +506,38 @@ Section zoo_G.
 
   Section array_model.
     Definition array_model t dq vs : iProp Σ :=
-      array_slice t (length vs) 0 dq vs.
+      ∃ l,
+      ⌜t = #l⌝ ∗
+      l ↦ₕ Header 0 (length vs) ∗
+      chunk_model l dq vs.
 
-    Lemma array_slice_model t sz dq vs :
-      sz = length vs →
-      array_slice t sz 0 dq vs ⊢
-      array_model t dq vs.
+    Lemma array_model_to_inv t dq vs :
+      array_model t dq vs ⊢
+      array_inv t (length vs).
     Proof.
       iSteps.
     Qed.
-    Lemma array_model_slice t dq vs :
-      array_model t dq vs ⊢
-      array_slice t (length vs) 0 dq vs.
+    Lemma array_slice_to_model t sz dq vs :
+      sz = length vs →
+      array_inv t sz -∗
+      array_slice t 0 dq vs -∗
+      array_model t dq vs.
     Proof.
-      iSteps.
+      iSteps. rewrite location_add_0 //.
+    Qed.
+    Lemma array_model_to_slice t dq vs :
+      array_model t dq vs ⊣⊢
+        array_inv t (length vs) ∗
+        array_slice t 0 dq vs.
+    Proof.
+      iSteps; rewrite location_add_0 //.
+    Qed.
+    Lemma array_model_to_slice' t dq vs :
+      array_model t dq vs ⊢
+        array_slice t 0 dq vs ∗
+        □ (array_slice t 0 dq vs -∗ array_model t dq vs).
+    Proof.
+      rewrite array_model_to_slice. iSteps.
     Qed.
 
     #[global] Instance array_model_timeless t dq vs :
@@ -469,19 +554,16 @@ Section zoo_G.
     #[global] Instance array_model_fractional t vs :
       Fractional (λ q, array_model t (DfracOwn q) vs).
     Proof.
-      apply _.
+      intros q1 q2. iSplit.
+      - iIntros "(%l & -> & #Hhdr & Hmodel1 & Hmodel2)". iSteps.
+      - iIntros "((%l & -> & #Hhdr & Hmodel1) & (%_l & %Heq & _ & Hmodel2))". injection Heq as <-.
+        iExists l. iSteps.
+        iApply chunk_model_fractional. iSteps.
     Qed.
     #[global] Instance array_model_as_fractional t q vs :
       AsFractional (array_model t (DfracOwn q) vs) (λ q, array_model t (DfracOwn q) vs) q.
     Proof.
-      apply _.
-    Qed.
-
-    Lemma array_model_to_inv t dq vs :
-      array_model t dq vs ⊢
-      array_inv t (length vs).
-    Proof.
-      iSteps.
+      split; [done | apply _].
     Qed.
 
     Lemma array_model_valid t dq vs :
@@ -489,7 +571,8 @@ Section zoo_G.
       array_model t dq vs ⊢
       ⌜✓ dq⌝.
     Proof.
-      apply array_slice_valid.
+      iIntros "% (%l & -> & #Hhdr & Hmodel)".
+      iApply (chunk_model_valid with "Hmodel"); first done.
     Qed.
     Lemma array_model_combine t dq1 vs1 dq2 vs2 :
       array_model t dq1 vs1 -∗
@@ -497,9 +580,10 @@ Section zoo_G.
         ⌜vs1 = vs2⌝ ∗
         array_model t (dq1 ⋅ dq2) vs1.
     Proof.
-      iIntros "Hmodel1 Hmodel2".
-      iDestruct (array_slice_agree_size with "Hmodel1 Hmodel2") as %?.
-      iDestruct (array_slice_combine with "Hmodel1 Hmodel2") as "(% & Hmodel)"; naive_solver.
+      iIntros "(%l & -> & #Hhdr1 & Hmodel1) (%_l & %Heq & #Hhdr2 & Hmodel2)". injection Heq as <-.
+      iDestruct (has_header_agree with "Hhdr1 Hhdr2") as %[= Hlength].
+      iDestruct (chunk_model_combine with "Hmodel1 Hmodel2") as "(<- & Hmodel)"; first done.
+      iSteps.
     Qed.
     Lemma array_model_valid_2 t dq1 vs1 dq2 vs2 :
       0 < length vs1 →
@@ -551,315 +635,80 @@ Section zoo_G.
       array_model t dq vs ⊢ |==>
       array_model t DfracDiscarded vs.
     Proof.
-      apply array_slice_persist.
+      iIntros "(%l & -> & #Hhdr & Hmodel)".
+      iMod (chunk_model_persist with "Hmodel") as "Hmodel".
+      iSteps.
     Qed.
 
     Lemma array_model_atomize t dq vs :
       array_model t dq vs ⊢
-      [∗ list] i ↦ v ∈ vs,
-        array_slice t (length vs) i dq [v].
+        array_inv t (length vs) ∗
+        [∗ list] i ↦ v ∈ vs,
+          array_slice t i dq [v].
     Proof.
-      apply array_slice_atomize.
+      rewrite array_model_to_slice array_slice_atomize.
+      iSteps.
     Qed.
 
+    #[local] Typeclasses Opaque array_slice.
     Lemma array_model_update {t dq vs} i v :
       vs !! i = Some v →
       array_model t dq vs ⊢
-        array_slice t (length vs) i dq [v] ∗
+        array_inv t (length vs) ∗
+        array_slice t i dq [v] ∗
         ( ∀ w,
-          array_slice t (length vs) i dq [w] -∗
+          array_slice t i dq [w] -∗
           array_model t dq (<[i := w]> vs)
         ).
     Proof.
-      rewrite /array_model. setoid_rewrite insert_length. rewrite -(Nat.add_0_l i).
-      apply array_slice_update.
+      intros.
+      setoid_rewrite array_model_to_slice.
+      rewrite array_slice_update //.
+      iSteps. rewrite insert_length. iSteps.
     Qed.
     Lemma array_model_lookup_acc {t dq vs} i v :
       vs !! i = Some v →
       array_model t dq vs ⊢
-        array_slice t (length vs) i dq [v] ∗
-        ( array_slice t (length vs) i dq [v] -∗
+        array_slice t i dq [v] ∗
+        ( array_slice t i dq [v] -∗
           array_model t dq vs
         ).
     Proof.
-      rewrite /array_model -(Nat.add_0_l i).
-      apply array_slice_lookup_acc.
+      intros.
+      rewrite array_model_to_slice {1}array_slice_lookup_acc //.
+      iSteps.
     Qed.
     Lemma array_model_lookup {t dq vs} i v :
       vs !! i = Some v →
       array_model t dq vs ⊢
-      array_slice t (length vs) i dq [v].
-    Proof.
-      rewrite /array_model -(Nat.add_0_l i).
-      apply array_slice_lookup.
-    Qed.
-  End array_model.
-
-  Section array_span.
-    Definition array_span t sz i dq n : iProp Σ :=
-      ∃ vs,
-      ⌜length vs = n⌝ ∗
-      array_slice t sz i dq vs.
-
-    #[global] Instance array_span_timeless t sz i dq n :
-      Timeless (array_span t sz i dq n).
-    Proof.
-      apply _.
-    Qed.
-    #[global] Instance array_span_persistent t sz i n :
-      Persistent (array_span t sz i DfracDiscarded n).
-    Proof.
-      apply _.
-    Qed.
-
-    #[global] Instance array_span_fractional t sz i n :
-      Fractional (λ q, array_span t sz i (DfracOwn q) n).
-    Proof.
-      intros q1 q2. iSplit.
-      - iIntros "(%vs & % & (Hslice1 & Hslice2))".
-        iSplitL "Hslice1"; iExists vs; auto.
-      - iIntros "((%vs & % & Hslice1) & (%_vs & % & Hslice2))".
-        iDestruct (array_slice_agree with "Hslice1 Hslice2") as %(_ & <-); [naive_solver.. |].
-        iCombine "Hslice1 Hslice2" as "Hslice".
-        iExists vs. auto.
-    Qed.
-    #[global] Instance array_span_as_fractional t sz i q vs :
-      AsFractional (array_slice t sz i (DfracOwn q) vs) (λ q, array_slice t sz i (DfracOwn q) vs) q.
-    Proof.
-      apply _.
-    Qed.
-
-    Lemma array_span_to_inv t sz i dq n :
-      array_span t sz i dq n ⊢
-      array_inv t sz.
-    Proof.
-      iSteps.
-    Qed.
-
-    Lemma array_span_to_slice t sz i dq n :
-      array_span t sz i dq n ⊢
-        ∃ vs,
-        ⌜length vs = n⌝ ∗
-        array_slice t sz i dq vs.
-    Proof.
-      iSteps.
-    Qed.
-    Lemma array_slice_to_span t sz i dq vs :
-      array_slice t sz i dq vs ⊢
-      array_span t sz i dq (length vs).
-    Proof.
-      iSteps.
-    Qed.
-
-    Lemma array_span_to_model t sz i dq n :
-      array_span t sz 0 dq sz -∗
-        ∃ vs,
-        array_model t dq vs.
-    Proof.
-      iSteps.
-    Qed.
-    Lemma array_model_to_span t dq vs :
-      array_model t dq vs ⊢
-      array_span t (length vs) 0 dq (length vs).
-    Proof.
-      iSteps.
-    Qed.
-
-    Lemma array_span_agree_size t sz1 i1 dq1 n1 sz2 i2 dq2 n2 :
-      array_span t sz1 i1 dq1 n1 -∗
-      array_span t sz2 i2 dq2 n2 -∗
-      ⌜sz1 = sz2⌝.
-    Proof.
-      iIntros "(%vs1 & % & Hslice1) (%vs2 & % & Hslice2)".
-      iApply (array_slice_agree_size with "Hslice1 Hslice2").
-    Qed.
-
-    Lemma array_span_valid t sz i dq n :
-      0 < n →
-      array_span t sz i dq n ⊢
-      ⌜✓ dq⌝.
-    Proof.
-      iIntros "% (%vs & % & Hslice)".
-      iDestruct (array_slice_valid with "Hslice") as %?; naive_solver.
-    Qed.
-    Lemma array_span_valid_2 t i sz1 dq1 n1 sz2 dq2 n2 :
-      n1 = n2 →
-      0 < n1 →
-      array_span t sz1 i dq1 n1 -∗
-      array_span t sz2 i dq2 n2 -∗
-      ⌜sz1 = sz2 ∧ ✓ (dq1 ⋅ dq2)⌝.
-    Proof.
-      iIntros (<- ?) "(%vs1 & % & Hslice1) (%vs2 & % & Hslice2)".
-      iDestruct (array_slice_valid_2 with "Hslice1 Hslice2") as %?; naive_solver.
-    Qed.
-    Lemma array_span_combine t i sz1 dq1 n1 sz2 dq2 n2 :
-      n1 = n2 →
-      array_span t sz1 i dq1 n1 -∗
-      array_span t sz2 i dq2 n2 -∗
-        ⌜sz1 = sz2⌝ ∗
-        array_span t sz1 i (dq1 ⋅ dq2) n1.
-    Proof.
-      iIntros "% (%vs & % & Hslice1) (%_vs & % & Hslice2)".
-      iDestruct (array_slice_combine with "Hslice1 Hslice2") as "(% & ?)"; first naive_solver.
-      iSplit; first iSteps. iExists vs. auto.
-    Qed.
-    Lemma array_span_dfrac_ne t1 sz1 i1 dq1 n1 t2 sz2 i2 dq2 n2 :
-      n1 = n2 →
-      0 < n1 →
-      ¬ ✓ (dq1 ⋅ dq2) →
-      array_span t1 sz1 i1 dq1 n1 -∗
-      array_span t2 sz2 i2 dq2 n2 -∗
-      ⌜t1 ≠ t2 ∨ i1 ≠ i2⌝.
-    Proof.
-      rewrite -not_and_r. iIntros "% % % Hspan1 Hspan2" ((-> & ->)).
-      iDestruct (array_span_valid_2 with "Hspan1 Hspan2") as %?; naive_solver.
-    Qed.
-    Lemma array_span_ne n t1 sz1 i1 n1 t2 sz2 i2 dq2 n2 :
-      n1 = n2 →
-      0 < n1 →
-      array_span t1 sz1 i1 (DfracOwn 1) n1 -∗
-      array_span t2 sz2 i2 dq2 n2 -∗
-      ⌜t1 ≠ t2 ∨ i1 ≠ i2⌝.
+      array_slice t i dq [v].
     Proof.
       intros.
-      iApply array_span_dfrac_ne; [done.. | intros []%(exclusive_l _)].
+      rewrite array_model_to_slice {1}array_slice_lookup //.
+      iSteps.
     Qed.
-    Lemma array_span_exclusive t i sz1 n1 sz2 n2 :
-      n1 = n2 →
-      0 < n1 →
-      array_span t sz1 i (DfracOwn 1) n1 -∗
-      array_span t sz2 i (DfracOwn 1) n2 -∗
-      False.
-    Proof.
-      iIntros "% % (%vs1 & % & Hslice1) (%vs2 & % & Hslice2)".
-      iApply (array_slice_exclusive with "Hslice1 Hslice2"); naive_solver.
-    Qed.
-    Lemma array_span_persist t sz i dq n :
-      array_span t sz i dq n ⊢ |==>
-      array_span t sz i DfracDiscarded n.
-    Proof.
-      iIntros "(%vs & % & Hslice)".
-      iExists vs. iSplitR; first iSteps.
-      iApply array_slice_persist. iSmash+.
-    Qed.
-
-    Lemma array_span_app t sz i dq n1 n2 :
-      array_span t sz i dq n1 ∗
-      array_span t sz (i + n1) dq n2 ⊣⊢
-      array_span t sz i dq (n1 + n2).
-    Proof.
-      iSplit.
-      - iIntros "((%vs1 & % & Hslice1) & (%vs2 & % & Hslice2))".
-        iExists (vs1 ++ vs2). iSplit; first (rewrite app_length; naive_solver).
-        iApply (array_slice_app_1 with "Hslice1 Hslice2"); first done.
-      - iIntros "(%vs & % & Hslice)".
-        iDestruct (array_slice_app_2 (take n1 vs) (drop n1 vs) with "Hslice") as "(Hslice1 & Hslice2)"; first rewrite take_drop //.
-        iSplitL "Hslice1".
-        + iExists (take n1 vs). iFrame. rewrite take_length_le //. lia.
-        + iExists (drop n1 vs). rewrite take_length_le; first lia. iFrame.
-          rewrite drop_length. iSteps.
-    Qed.
-    Lemma array_span_app_1 t sz i dq n1 n2 :
-      array_span t sz i dq n1 -∗
-      array_span t sz (i + n1) dq n2 -∗
-      array_span t sz i dq (n1 + n2).
-    Proof.
-      rewrite -array_span_app. iSteps.
-    Qed.
-    Lemma array_span_app_2 {t sz i dq n} n1 n2 :
-      n = n1 + n2 →
-      array_span t sz i dq n ⊢
-        array_span t sz i dq n1 ∗
-        array_span t sz (i + n1) dq n2.
-    Proof.
-      intros ->. rewrite array_span_app //.
-    Qed.
-
-    Lemma array_span_app3 t sz i dq n1 n2 n3 :
-      array_span t sz i dq n1 ∗
-      array_span t sz (i + n1) dq n2 ∗
-      array_span t sz (i + n1 + n2) dq n3 ⊣⊢
-      array_span t sz i dq (n1 + n2 + n3).
-    Proof.
-      iSplit.
-      - iIntros "((%vs1 & <- & Hspan1) & (%vs2 & <- & Hspan2) & (%vs3 & <- & Hspan3))".
-        iExists (vs1 ++ vs2 ++ vs3). rewrite -array_slice_app3. iFrame.
-        rewrite !app_length. iSteps.
-      - iIntros "(%vs & %Hvs & Hspan)".
-        rewrite -(take_drop n1 vs) -(take_drop n2 (drop n1 vs)) drop_drop.
-        iDestruct (array_slice_app3 with "Hspan") as "(Hspan1 & Hspan2 & Hspan3)".
-        rewrite !take_length !Nat.min_l; [lia | rewrite drop_length; lia |].
-        iSplitL "Hspan1"; last iSplitL "Hspan2".
-        all: iExists _; iFrame.
-        all: rewrite ?take_length ?drop_length.
-        all: iSteps.
-    Qed.
-    Lemma array_span_app3_1 t sz dq i1 n1 i2 n2 i3 n3 :
-      i2 = i1 + n1 →
-      i3 = i1 + n1 + n2 →
-      array_span t sz i1 dq n1 -∗
-      array_span t sz i2 dq n2 -∗
-      array_span t sz i3 dq n3 -∗
-      array_span t sz i1 dq (n1 + n2 + n3).
-    Proof.
-      rewrite -array_span_app3. iSteps.
-    Qed.
-    Lemma array_span_app3_2 {t sz i dq n} n1 n2 n3 :
-      n = n1 + n2 + n3 →
-      array_span t sz i dq n ⊢
-        array_span t sz i dq n1 ∗
-        array_span t sz (i + n1) dq n2 ∗
-        array_span t sz (i + n1 + n2) dq n3.
-    Proof.
-      rewrite array_span_app3. iSteps.
-    Qed.
-
-    Lemma array_span_update {t sz i dq n} j :
-      j < n →
-      array_span t sz i dq n ⊢
-        ∃ v,
-        array_slice t sz (i + j) dq [v] ∗
-        ( ∀ w,
-          array_slice t sz (i + j) dq [w] -∗
-          array_span t sz i dq n
-        ).
-    Proof.
-      iIntros "%Hj (%vs & %Hv & Hslice)".
-      iDestruct (array_slice_update j with "Hslice") as "(Hv & Hslice)".
-      { rewrite list_lookup_lookup_total_lt; naive_solver. }
-      iExists (vs !!! j). iFrame. iIntros "%w Hw".
-      iExists (<[j := w]> vs). iSplit; first rewrite insert_length //.
-      iApply ("Hslice" with "Hw").
-    Qed.
-    Lemma array_span_lookup_acc {t sz i dq n} j :
-      j < n →
-      array_span t sz i dq n ⊢
-        ∃ v,
-        array_slice t sz (i + j) dq [v] ∗
-        ( array_slice t sz (i + j) dq [v] -∗
-          array_span t sz i dq n
-        ).
-    Proof.
-      iIntros "%Hj Hspan".
-      iDestruct (array_span_update with "Hspan") as "(%v & Hv & Hspan)"; first done.
-      auto with iFrame.
-    Qed.
-    Lemma array_span_lookup {t sz i dq n} j :
-      j < n →
-      array_span t sz i dq n ⊢
-        ∃ v,
-        array_slice t sz (i + j) dq [v].
-    Proof.
-      intros. rewrite array_span_lookup_acc //. iSteps.
-    Qed.
-  End array_span.
+  End array_model.
 
   Section array_cslice.
     Definition array_cslice t (sz : nat) i dq vs : iProp Σ :=
       ∃ l,
       ⌜t = #l⌝ ∗
-      l.[size] ↦□ #sz ∗
-      chunk_cslice l.[data] sz i dq vs.
+      l ↦ₕ Header 0 sz ∗
+      chunk_cslice l sz i dq vs.
+
+    Lemma array_cslice_to_inv t sz i dq vs :
+      array_cslice t sz i dq vs ⊢
+      array_inv t sz.
+    Proof.
+      iSteps.
+    Qed.
+    Lemma array_model_to_cslice t dq vs :
+      array_model t dq vs ⊢
+      array_cslice t (length vs) 0 dq vs.
+    Proof.
+      rewrite /array_model /array_slice /array_cslice.
+      setoid_rewrite chunk_model_to_cslice. done.
+    Qed.
 
     #[global] Instance array_cslice_timeless t sz i dq vs :
       Timeless (array_cslice t sz i dq vs).
@@ -876,9 +725,9 @@ Section zoo_G.
       Fractional (λ q, array_cslice t sz i (DfracOwn q) vs).
     Proof.
       intros q1 q2. iSplit.
-      - iIntros "(%l & -> & #Hsz & (Hcslice1 & Hcslice2))".
+      - iIntros "(%l & -> & #Hhdr & (Hcslice1 & Hcslice2))".
         iSteps.
-      - iIntros "((%l & -> & #Hsz & Hcslice1) & (%_l & %Heq & _ & Hcslice2))". injection Heq as <-.
+      - iIntros "((%l & -> & #Hhdr & Hcslice1) & (%_l & %Heq & _ & Hcslice2))". injection Heq as <-.
         iCombine "Hcslice1 Hcslice2" as "Hcslice".
         iSteps.
     Qed.
@@ -886,23 +735,6 @@ Section zoo_G.
       AsFractional (array_cslice t sz i (DfracOwn q) vs) (λ q, array_cslice t sz i (DfracOwn q) vs) q.
     Proof.
       split; [done | apply _].
-    Qed.
-
-    Lemma array_cslice_to_inv t sz i dq vs :
-      array_cslice t sz i dq vs ⊢
-      array_inv t sz.
-    Proof.
-      iSteps.
-    Qed.
-
-    Lemma array_model_to_cslice t dq vs :
-      array_model t dq vs ⊢
-      array_cslice t (length vs) 0 dq vs.
-    Proof.
-      rewrite /array_model /array_slice /array_cslice.
-      setoid_rewrite chunk_model_to_cslice.
-      setoid_rewrite location_add_0.
-      done.
     Qed.
 
     Lemma array_cslice_nil t sz i dq :
@@ -1004,7 +836,7 @@ Section zoo_G.
         ⌜vs1 = vs2⌝ ∗
         array_cslice t sz i (dq1 ⋅ dq2) vs1.
     Proof.
-      iIntros "% (%l & -> & #Hsz & Hcslice1) (%_l & %Heq & _ & Hcslice2)". injection Heq as <-.
+      iIntros "% (%l & -> & #Hhdr & Hcslice1) (%_l & %Heq & _ & Hcslice2)". injection Heq as <-.
       iDestruct (chunk_cslice_combine with "Hcslice1 Hcslice2") as "($ & Hcslice)"; first done.
       iSteps.
     Qed.
@@ -1071,6 +903,60 @@ Section zoo_G.
     Qed.
   End array_cslice.
 
+  #[local] Typeclasses Opaque array_slice array_model.
+
+  Notation au_load t i Φ := (
+    AU <{
+      ∃∃ dq v,
+      array_slice t i dq [v]
+    }> @ ⊤, ∅ <{
+      array_slice t i dq [v],
+    COMM
+      Φ v
+    }>
+  )%I.
+  Notation au_store t i v P := (
+    AU <{
+      ∃∃ w,
+      array_slice t i (DfracOwn 1) [w]
+    }> @ ⊤, ∅ <{
+      array_slice t i (DfracOwn 1) [v],
+    COMM
+      P
+    }>
+  )%I.
+
+  Lemma array_unsafe_alloc_spec sz :
+    (0 ≤ sz)%Z →
+    {{{ True }}}
+      array_unsafe_alloc #sz
+    {{{ t,
+      RET t;
+      array_model t (DfracOwn 1) (replicate (Z.to_nat sz) ()%V)
+    }}}.
+  Proof.
+    rewrite /array_model /array_slice.
+    iIntros "%Hsz %Φ _ HΦ".
+    wp_rec.
+    wp_alloc l as "#Hhdr" "_" "Hl"; [done.. |].
+    iSteps. rewrite replicate_length. iSteps.
+  Qed.
+  Lemma array_alloc_spec sz :
+    {{{ True }}}
+      array_alloc #sz
+    {{{ t,
+      RET t;
+      ⌜0 ≤ sz⌝%Z ∗
+      array_model t (DfracOwn 1) (replicate (Z.to_nat sz) ()%V)
+    }}}.
+  Proof.
+    iIntros "%Φ _ HΦ".
+    wp_rec.
+    wp_smart_apply assume_spec' as "%Hsz".
+    wp_smart_apply (array_unsafe_alloc_spec with "[//]"); first done.
+    iSteps.
+  Qed.
+
   Lemma array_create_spec :
     {{{ True }}}
       array_create ()
@@ -1081,13 +967,687 @@ Section zoo_G.
   Proof.
     iIntros "%Φ _ HΦ".
     wp_rec.
-    iApply wp_fupd.
-    wp_apply (chunk_make_spec with "[//]") as "%l (Hl & _)".
-    iDestruct (chunk_model_cons_2 with "Hl") as "(Hsz & Hdata)". rewrite -{1}(location_add_0 l).
-    iMod (pointsto_persist with "Hsz") as "#Hsz".
-    iApply "HΦ". iSteps. rewrite location_add_0 //.
+    wp_apply (array_unsafe_alloc_spec with "[//]"); first done.
+    iSteps.
   Qed.
 
+  Lemma array_size_spec_inv t sz :
+    {{{
+      array_inv t sz
+    }}}
+      array_size t
+    {{{
+      RET #sz; True
+    }}}.
+  Proof.
+    iSteps.
+  Qed.
+  Lemma array_size_spec_atomic t :
+    <<<
+      True
+    | ∀∀ dq vs,
+      array_model t dq vs
+    >>>
+      array_size t
+    <<<
+      array_model t dq vs
+    | RET #(length vs);
+      £ 1
+    >>>.
+  Proof.
+    rewrite /array_model.
+    iIntros "!> %Φ _ HΦ".
+    wp_rec credit:"H£".
+    iMod "HΦ" as "(%dq & %vs & (%l & -> & #Hhdr & Hmodel) & _ & HΦ)".
+    wp_get_size.
+    iApply ("HΦ" with "[Hmodel] H£").
+    iSteps.
+  Qed.
+  Lemma array_size_spec_atomic_cslice t :
+    <<<
+      True
+    | ∀∀ sz i dq vs,
+      array_cslice t sz i dq vs
+    >>>
+      array_size t
+    <<<
+      array_cslice t sz i dq vs
+    | RET #sz;
+      £ 1
+    >>>.
+  Proof.
+    iIntros "!> %Φ _ HΦ".
+    wp_rec credit:"H£".
+    iMod "HΦ" as "(%sz & %i & %dq & %vs & (%l & -> & #Hhdr & Hcslice) & _ & HΦ)".
+    wp_get_size.
+    iApply ("HΦ" with "[Hcslice] H£").
+    iSteps.
+  Qed.
+  Lemma array_size_spec t dq vs :
+    {{{
+      array_model t dq vs
+    }}}
+      array_size t
+    {{{
+      RET #(length vs);
+      array_model t dq vs
+    }}}.
+  Proof.
+    rewrite /array_model. iSteps.
+  Qed.
+  Lemma array_size_spec_cslice t sz i dq vs :
+    {{{
+      array_cslice t sz i dq vs
+    }}}
+      array_size t
+    {{{
+      RET #sz;
+      array_cslice t sz i dq vs
+    }}}.
+  Proof.
+    iSteps.
+  Qed.
+
+  Lemma array_unsafe_get_spec_atomic_slice t (j : Z) :
+    <<<
+      True
+    | ∀∀ dq vs i v,
+      ⌜(i ≤ j)%Z ∧ vs !! (Z.to_nat j - i) = Some v⌝ ∗
+      array_slice t i dq vs
+    >>>
+      array_unsafe_get t #j
+    <<<
+      array_slice t i dq vs
+    | RET v;
+      £ 1
+    >>>.
+  Proof.
+    rewrite /array_slice.
+    iIntros "!> %Φ _ HΦ".
+    wp_rec credit:"H£". wp_pures.
+    iMod "HΦ" as "(%dq & %vs & %i & %v & ((%Hi & %Hlookup) & (%l & -> & Hmodel)) & _ & HΦ)".
+    iDestruct (chunk_model_lookup_acc' j with "Hmodel") as "(H↦ & Hmodel)"; [lia | done | lia |].
+    wp_load.
+    iApply ("HΦ" with "[H↦ Hmodel] H£").
+    iSteps.
+  Qed.
+  Lemma array_unsafe_get_spec_atomic_cell t (i : Z) :
+    <<<
+      True
+    | ∀∀ i_ dq v,
+      ⌜i = Z.of_nat i_⌝ ∗
+      array_slice t i_ dq [v]
+    >>>
+      array_unsafe_get t #i
+    <<<
+      array_slice t (Z.to_nat i) dq [v]
+    | RET v;
+      £ 1
+    >>>.
+  Proof.
+    iIntros "!> %Φ _ HΦ".
+    awp_apply (array_unsafe_get_spec_atomic_slice with "[//]").
+    iApply (aacc_aupd_commit with "HΦ"); first done. iIntros "%i_ %dq %v (-> & Hslice)".
+    rewrite /atomic_acc /= Nat2Z.id.
+    iExists dq, [v], i_, v. rewrite Nat.sub_diag. iSteps.
+  Qed.
+  Lemma array_unsafe_get_spec_atomic t (i : Z) :
+    (0 ≤ i)%Z →
+    <<<
+      True
+    | ∀∀ dq vs v,
+      ⌜vs !! Z.to_nat i = Some v⌝ ∗
+      array_model t dq vs
+    >>>
+      array_unsafe_get t #i
+    <<<
+      array_model t dq vs
+    | RET v;
+      £ 1
+    >>>.
+  Proof.
+    iIntros "%Hi !> %Φ _ HΦ".
+    awp_apply (array_unsafe_get_spec_atomic_slice with "[//]").
+    iApply (aacc_aupd_commit with "HΦ"); first done. iIntros "%dq %vs %v (%Hlookup & Hmodel)".
+    iDestruct (array_model_to_slice' with "Hmodel") as "(Hslice & #?)".
+    rewrite /atomic_acc /=.
+    iExists dq, vs, 0, v. rewrite Nat.sub_0_r. iSteps.
+  Qed.
+  Lemma array_unsafe_get_spec_slice k t i dq vs (j : Z) v :
+    (i ≤ j)%Z →
+    vs !! k = Some v →
+    k = Z.to_nat j - i →
+    {{{
+      array_slice t i dq vs
+    }}}
+      array_unsafe_get t #j
+    {{{
+      RET v;
+      array_slice t i dq vs
+    }}}.
+  Proof.
+    iIntros (Hj Hlookup ->) "%Φ Hslice HΦ".
+    iApply wp_fupd.
+    awp_apply (array_unsafe_get_spec_atomic_slice with "[//]") without "HΦ".
+    rewrite /atomic_acc /=.
+    iExists dq, vs, i, v.
+    iApply fupd_mask_intro; first done. iIntros "Hclose".
+    iSplitL "Hslice"; first auto. iSplit; first iSteps.
+    iIntros "Hslice". iMod "Hclose" as "_". iIntros "!> H£ HΦ".
+    iMod (lc_fupd_elim_later with "H£ HΦ") as "HΦ".
+    iSteps.
+  Qed.
+  Lemma array_unsafe_get_spec_cell t (i : Z) i_ dq v :
+    i = Z.to_nat i_ →
+    {{{
+      array_slice t i_ dq [v]
+    }}}
+      array_unsafe_get t #i
+    {{{
+      RET v;
+      array_slice t i_ dq [v]
+    }}}.
+  Proof.
+    intros.
+    eapply (array_unsafe_get_spec_slice 0); [lia | done | lia].
+  Qed.
+  Lemma array_unsafe_get_spec i_ t (i : Z) dq vs v :
+    (0 ≤ i)%Z →
+    vs !! i_ = Some v →
+    i_ = Z.to_nat i →
+    {{{
+      array_model t dq vs
+    }}}
+      array_unsafe_get t #i
+    {{{
+      RET v;
+      array_model t dq vs
+    }}}.
+  Proof.
+    iIntros (Hi Hlookup ->) "%Φ Hmodel HΦ".
+    iApply wp_fupd.
+    awp_apply (array_unsafe_get_spec_atomic with "[//]") without "HΦ"; first done.
+    rewrite /atomic_acc /=.
+    iExists dq, vs, v.
+    iApply fupd_mask_intro; first done. iIntros "Hclose".
+    iSplitL "Hmodel"; first auto. iSplit; first iSteps.
+    iIntros "Hmodel". iMod "Hclose" as "_". iIntros "!> H£ HΦ".
+    iMod (lc_fupd_elim_later with "H£ HΦ") as "HΦ".
+    iSteps.
+  Qed.
+
+  Lemma array_get_spec_atomic_slice t sz (j : Z) :
+    <<<
+      array_inv t sz
+    | ∀∀ dq vs i v,
+      ⌜(i ≤ j)%Z ∧ vs !! (Z.to_nat j - i) = Some v⌝ ∗
+      array_slice t i dq vs
+    >>>
+      array_get t #j
+    <<<
+      array_slice t i dq vs
+    | RET v;
+      £ 1
+    >>>.
+  Proof.
+    iIntros "!> %Φ #Hinv HΦ".
+    wp_rec.
+    wp_smart_apply assume_spec' as "_".
+    wp_smart_apply (array_size_spec_inv with "Hinv") as "_".
+    wp_smart_apply assume_spec' as "_".
+    wp_smart_apply (array_unsafe_get_spec_atomic_slice with "[//] HΦ").
+  Qed.
+  Lemma array_get_spec_atomic_cell t sz (i : Z) i_ :
+    i = Z.of_nat i_ →
+    <<<
+      array_inv t sz
+    | ∀∀ dq v,
+      array_slice t i_ dq [v]
+    >>>
+      array_get t #i
+    <<<
+      array_slice t i_ dq [v]
+    | RET v;
+      £ 1
+    >>>.
+  Proof.
+    iIntros (->) "!> %Φ #Hinv HΦ".
+    awp_apply (array_get_spec_atomic_slice with "Hinv").
+    iApply (aacc_aupd_commit with "HΦ"); first done. iIntros "%dq %v Hslice".
+    rewrite /atomic_acc /= Nat2Z.id.
+    iExists dq, [v], i_, v. rewrite Nat.sub_diag. iSteps.
+  Qed.
+  Lemma array_get_spec_atomic t (i : Z) :
+    (0 ≤ i)%Z →
+    <<<
+      True
+    | ∀∀ dq vs v,
+      ⌜vs !! Z.to_nat i = Some v⌝ ∗
+      array_model t dq vs
+    >>>
+      array_get t #i
+    <<<
+      array_model t dq vs
+    | RET v;
+      £ 1
+    >>>.
+  Proof.
+    iIntros "%Hi !> %Φ _ HΦ".
+    wp_rec.
+    wp_smart_apply assume_spec' as "_".
+    awp_smart_apply (array_size_spec_atomic with "[//]").
+    iApply (aacc_aupd_abort with "HΦ"); first done. iIntros "%dq %vs %v (% & Hmodel)".
+    iAaccIntro with "Hmodel"; first iSteps.
+    iIntros "Hmodel !>". iSplitL; first auto. iIntros "HΦ !> _".
+    wp_smart_apply assume_spec' as "_".
+    wp_smart_apply (array_unsafe_get_spec_atomic with "[//] HΦ"); first done.
+  Qed.
+  Lemma array_get_spec_slice k t sz i dq vs (j : Z) v :
+    (i ≤ j)%Z →
+    vs !! k = Some v →
+    k = Z.to_nat j - i →
+    {{{
+      array_inv t sz ∗
+      array_slice t i dq vs
+    }}}
+      array_get t #j
+    {{{
+      RET v;
+      array_slice t i dq vs
+    }}}.
+  Proof.
+    iIntros (Hi Hlookup ->) "%Φ (#Hinv & Hslice) HΦ".
+    wp_rec.
+    wp_smart_apply assume_spec' as "_".
+    wp_smart_apply (array_size_spec_inv with "Hinv") as "_".
+    wp_smart_apply assume_spec' as "_".
+    wp_smart_apply (array_unsafe_get_spec_slice with "Hslice"); done.
+  Qed.
+  Lemma array_get_spec_cell t sz (i : Z) i_ dq v :
+    i = Z.of_nat i_ →
+    {{{
+      array_inv t sz ∗
+      array_slice t i_ dq [v]
+    }}}
+      array_get t #i
+    {{{
+      RET v;
+      array_slice t i_ dq [v]
+    }}}.
+  Proof.
+    intros.
+    eapply (array_get_spec_slice 0); [lia | done | lia].
+  Qed.
+  Lemma array_get_spec i_ t (i : Z) dq vs v :
+    (0 ≤ i)%Z →
+    vs !! i_ = Some v →
+    i_ = Z.to_nat i →
+    {{{
+      array_model t dq vs
+    }}}
+      array_get t #i
+    {{{
+      RET v;
+      array_model t dq vs
+    }}}.
+  Proof.
+    iIntros (Hi Hlookup ->) "%Φ Hmodel HΦ".
+    wp_rec.
+    wp_smart_apply assume_spec' as "_".
+    wp_smart_apply (array_size_spec with "Hmodel") as "Hmodel".
+    wp_smart_apply assume_spec' as "_".
+    wp_smart_apply (array_unsafe_get_spec with "Hmodel"); done.
+  Qed.
+
+  Lemma array_unsafe_set_spec_atomic_slice t (j : Z) v :
+    <<<
+      True
+    | ∀∀ sz vs i,
+      ⌜i ≤ j < i + length vs⌝%Z ∗
+      array_slice t sz i (DfracOwn 1) vs
+    >>>
+      array_unsafe_set t #j v
+    <<<
+      array_slice t sz i (DfracOwn 1) (<[Z.to_nat j - i := v]> vs)
+    | RET ();
+      £ 1
+    >>>.
+  Proof.
+    rewrite /array_model /array_slice.
+    iIntros "!> %Φ _ HΦ".
+    wp_rec credit:"H£". wp_pures.
+    iMod "HΦ" as "(%sz & %vs & %i & (%Hj & (%l & -> & #Hhdr & Hmodel)) & _ & HΦ)".
+    iDestruct (chunk_model_update' j with "Hmodel") as "(H↦ & Hmodel)"; [lia | | done |].
+    { destruct (nth_lookup_or_length vs (Z.to_nat j - Z.to_nat i) inhabitant); [done | lia]. }
+    wp_store.
+    iApply ("HΦ" with "[H↦ Hmodel] [H£]"); last iSteps.
+    rewrite Nat2Z.id. iSteps.
+  Qed.
+  Lemma array_unsafe_set_spec_atomic_cell t (i : Z) v :
+    <<<
+      True
+    | ∀∀ sz i_ w,
+      ⌜i = Z.of_nat i_⌝ ∗
+      array_slice t sz i_ (DfracOwn 1) [w]
+    >>>
+      array_unsafe_set t #i v
+    <<<
+      array_slice t sz i_ (DfracOwn 1) [v]
+    | RET ();
+      £ 1
+    >>>.
+  Proof.
+    iIntros "!> %Φ _ HΦ".
+    awp_apply (array_unsafe_set_spec_atomic_slice with "[//]").
+    iApply (aacc_aupd_commit with "HΦ"); first done. iIntros "%sz %i_ %w (-> & Hslice)".
+    rewrite /atomic_acc /= Nat2Z.id.
+    iExists sz, [w], i_. rewrite Nat.sub_diag. iSteps.
+  Qed.
+  Lemma array_unsafe_set_spec_atomic t (i : Z) v :
+    (0 ≤ i)%Z →
+    <<<
+      True
+    | ∀∀ vs,
+      ⌜i < length vs⌝%Z ∗
+      array_model t (DfracOwn 1) vs
+    >>>
+      array_unsafe_set t #i v
+    <<<
+      array_model t (DfracOwn 1) (<[Z.to_nat i := v]> vs)
+    | RET ();
+      £ 1
+    >>>.
+  Proof.
+    rewrite /array_model.
+    iIntros "%Hi !> %Φ _ HΦ".
+    awp_apply (array_unsafe_set_spec_atomic_slice with "[//]").
+    iApply (aacc_aupd_commit with "HΦ"); first done. iIntros "%vs (%Hlookup & Hmodel)".
+    rewrite /atomic_acc /=.
+    iExists (length vs), vs, 0. rewrite Nat.sub_0_r insert_length. iSteps.
+  Qed.
+  Lemma array_unsafe_set_spec_slice t sz i vs (j : Z) v :
+    (i ≤ j < i + length vs)%Z →
+    {{{
+      array_slice t sz i (DfracOwn 1) vs
+    }}}
+      array_unsafe_set t #j v
+    {{{
+      RET ();
+      array_slice t sz i (DfracOwn 1) (<[Z.to_nat j - i := v]> vs)
+    }}}.
+  Proof.
+    iIntros "%Hj %Φ Hslice HΦ".
+    iApply wp_fupd.
+    awp_apply (array_unsafe_set_spec_atomic_slice with "[//]") without "HΦ".
+    rewrite /atomic_acc /=.
+    iExists sz, vs, i.
+    iApply fupd_mask_intro; first done. iIntros "Hclose".
+    iSplitL "Hslice"; first auto. iSplit; first iSteps.
+    iIntros "Hslice". iMod "Hclose" as "_". iIntros "!> H£ HΦ".
+    iMod (lc_fupd_elim_later with "H£ HΦ") as "HΦ".
+    iSteps.
+  Qed.
+  Lemma array_unsafe_set_spec_cell t sz (i : Z) i_ w v :
+    i = Z.of_nat i_ →
+    {{{
+      array_slice t sz i_ (DfracOwn 1) [w]
+    }}}
+      array_unsafe_set t #i v
+    {{{
+      RET ();
+      array_slice t sz i_ (DfracOwn 1) [v]
+    }}}.
+  Proof.
+    iIntros (->) "%Φ Hslice HΦ".
+    wp_apply (array_unsafe_set_spec_slice with "Hslice").
+    { simpl. lia. }
+    rewrite Nat2Z.id Nat.sub_diag //.
+  Qed.
+  Lemma array_unsafe_set_spec t (i : Z) vs v :
+    (0 ≤ i < length vs)%Z →
+    {{{
+      array_model t (DfracOwn 1) vs
+    }}}
+      array_unsafe_set t #i v
+    {{{
+      RET ();
+      array_model t (DfracOwn 1) (<[Z.to_nat i := v]> vs)
+    }}}.
+  Proof.
+    iIntros "%Hi %Φ Hmodel HΦ".
+    wp_apply (array_unsafe_set_spec_slice with "Hmodel"); first done.
+    rewrite Nat.sub_0_r /array_model insert_length //.
+  Qed.
+
+  Lemma array_set_spec_atomic_slice t (j : Z) v :
+    <<<
+      True
+    | ∀∀ sz vs i,
+      ⌜(i ≤ j < i + length vs)%Z⌝ ∗
+      array_slice t sz i (DfracOwn 1) vs
+    >>>
+      array_set t #j v
+    <<<
+      array_slice t sz i (DfracOwn 1) (<[Z.to_nat j - i := v]> vs)
+    | RET ();
+      £ 1
+    >>>.
+  Proof.
+    iIntros "!> %Φ _ HΦ".
+    wp_rec.
+    wp_smart_apply assume_spec' as "_".
+    awp_smart_apply (array_size_spec_atomic_slice with "[//]").
+    iApply (aacc_aupd_abort with "HΦ"); first done. iIntros "%sz %vs %i (%Hj & Hslice)".
+    iAaccIntro with "Hslice"; first iSteps.
+    iIntros "Hslice !>". iSplitL; first auto. iIntros "HΦ !> _".
+    wp_smart_apply assume_spec' as "_".
+    wp_smart_apply (array_unsafe_set_spec_atomic_slice with "[//] HΦ").
+  Qed.
+  Lemma array_set_spec_atomic_cell t (i : Z) v :
+    <<<
+      True
+    | ∀∀ sz i_ w,
+      ⌜i = Z.of_nat i_⌝ ∗
+      array_slice t sz i_ (DfracOwn 1) [w]
+    >>>
+      array_set t #i v
+    <<<
+      array_slice t sz i_ (DfracOwn 1) [v]
+    | RET ();
+      £ 1
+    >>>.
+  Proof.
+    iIntros "!> %Φ _ HΦ".
+    awp_apply (array_set_spec_atomic_slice with "[//]").
+    iApply (aacc_aupd_commit with "HΦ"); first done. iIntros "%sz %i_ %w (-> & Hslice)".
+    rewrite /atomic_acc /= Nat2Z.id.
+    iExists sz, [w], i_. rewrite Nat.sub_diag. iSteps.
+  Qed.
+  Lemma array_set_spec_atomic t (i : Z) v :
+    (0 ≤ i)%Z →
+    <<<
+      True
+    | ∀∀ vs,
+      ⌜(i < length vs)%Z⌝ ∗
+      array_model t (DfracOwn 1) vs
+    >>>
+      array_set t #i v
+    <<<
+      array_model t (DfracOwn 1) (<[Z.to_nat i := v]> vs)
+    | RET ();
+      £ 1
+    >>>.
+  Proof.
+    rewrite /array_model.
+    iIntros "%Hi !> %Φ _ HΦ".
+    awp_apply (array_set_spec_atomic_slice with "[//]").
+    iApply (aacc_aupd_commit with "HΦ"); first done. iIntros "%vs (%Hi'  & Hmodel)".
+    rewrite /atomic_acc /=.
+    iExists (length vs), vs, 0. rewrite Nat.sub_0_r insert_length. iSteps.
+  Qed.
+  Lemma array_set_spec_slice t sz i vs (j : Z) v :
+    (i ≤ j < i + length vs)%Z →
+    {{{
+      array_slice t sz i (DfracOwn 1) vs
+    }}}
+      array_set t #j v
+    {{{
+      RET ();
+      array_slice t sz i (DfracOwn 1) (<[Z.to_nat j - i := v]> vs)
+    }}}.
+  Proof.
+    iIntros "%Hj %Φ Hslice HΦ".
+    wp_rec.
+    wp_smart_apply assume_spec' as "_".
+    wp_smart_apply (array_size_spec_slice with "Hslice") as "Hslice".
+    wp_smart_apply assume_spec' as "_".
+    wp_smart_apply (array_unsafe_set_spec_slice with "Hslice"); done.
+  Qed.
+  Lemma array_set_spec_cell t sz (i : Z) i_ w v :
+    i = Z.of_nat i_ →
+    {{{
+      array_slice t sz i_ (DfracOwn 1) [w]
+    }}}
+      array_set t #i v
+    {{{
+      RET ();
+      array_slice t sz i_ (DfracOwn 1) [v]
+    }}}.
+  Proof.
+    iIntros (->) "%Φ Hslice HΦ".
+    wp_apply (array_set_spec_slice with "Hslice").
+    { simpl. lia. }
+    rewrite Nat2Z.id Nat.sub_diag //.
+  Qed.
+  Lemma array_set_spec t (i : Z) vs v :
+    (0 ≤ i < length vs)%Z →
+    {{{
+      array_model t (DfracOwn 1) vs
+    }}}
+      array_set t #i v
+    {{{
+      RET ();
+      array_model t (DfracOwn 1) (<[Z.to_nat i := v]> vs)
+    }}}.
+  Proof.
+    iIntros "%Hi %Φ Hmodel HΦ".
+    wp_apply (array_set_spec_slice with "Hmodel"); first done.
+    rewrite Nat.sub_0_r /array_model insert_length //.
+  Qed.
+
+  Lemma array_unsafe_fill_slice_spec_atomic Ψ t sz (i n : Z) v :
+    (0 ≤ i)%Z →
+    (0 ≤ n)%Z →
+    {{{
+      ▷ Ψ 0 ∗
+      □ (
+        ∀ j,
+        ⌜j < Z.to_nat n⌝ -∗
+        Ψ j -∗
+        au_store t sz (Z.to_nat i + j) v (
+          ▷ Ψ (S j)
+        )
+      )
+    }}}
+      array_unsafe_fill_slice t #i #n v
+    {{{
+      RET ();
+      Ψ (Z.to_nat n)
+    }}}.
+  Proof.
+    iIntros "%Hi %Hn %Φ (HΨ & #H) HΦ".
+    wp_rec.
+    pose Ψ' (_ : Z) i :=
+      Ψ i.
+    wp_smart_apply (for_upto_spec_strong Ψ' with "[$HΨ]"); last rewrite Z.sub_0_r //.
+    iIntros "!> %j_ %j (-> & %Hj) HΨ". rewrite Z.add_0_l in Hj |- *.
+    iDestruct ("H" with "[%] HΨ") as "H'"; first lia.
+    awp_smart_apply (array_unsafe_set_spec_atomic_cell with "[//]").
+    iApply (aacc_aupd_commit with "H'"); first done. iIntros "%w H↦".
+    rewrite /atomic_acc /=.
+    repeat iExists _. iFrame. iSteps.
+  Qed.
+  Lemma array_unsafe_fill_slice_spec t sz vs (i : Z) i_ (n : Z) v :
+    i = Z.of_nat i_ →
+    n = length vs →
+    {{{
+      array_slice t sz i_ (DfracOwn 1) vs
+    }}}
+      array_unsafe_fill_slice t #i #n v
+    {{{
+      RET ();
+      array_slice t sz i_ (DfracOwn 1) (replicate (Z.to_nat n) v)
+    }}}.
+  Proof.
+    iIntros (-> ->) "%Φ Hslice HΦ".
+    pose Ψ j :=
+      array_slice t sz i_ (DfracOwn 1) (replicate j v ++ drop j vs).
+    wp_apply (array_unsafe_fill_slice_spec_atomic Ψ with "[$Hslice]"); [lia.. | |]; last first.
+    { rewrite /Ψ skipn_all2; first lia. rewrite right_id //. }
+    iIntros "!> %j %Hj Hslice". rewrite Nat2Z.id.
+    opose proof* (list_lookup_lookup_total_lt vs j) as Hlookup; first lia.
+    iDestruct (array_slice_update j with "Hslice") as "(H↦ & Hslice)".
+    { rewrite lookup_app_r replicate_length // lookup_drop Nat.sub_diag right_id //. }
+    iAuIntro. iAaccIntro with "H↦"; first auto with iFrame. iIntros "H↦".
+    iDestruct ("Hslice" with "H↦") as "Hslice".
+    rewrite /Ψ replicate_S_end -assoc insert_app_r_alt replicate_length // Nat.sub_diag.
+    erewrite drop_S; done.
+  Qed.
+
+  Lemma array_fill_slice_spec t sz vs (i : Z) i_ (n : Z) v :
+
+    i = Z.of_nat i_ →
+    n = length vs →
+    {{{
+      array_slice t sz i_ (DfracOwn 1) vs
+    }}}
+      array_fill_slice t #i #n v
+    {{{
+      RET ();
+      array_slice t sz i_ (DfracOwn 1) (replicate (Z.to_nat n) v)
+    }}}.
+  Proof.
+    iIntros (-> ->) "%Φ Hslice HΦ".
+    wp_rec.
+    wp_smart_apply (array_size_spec_slice with "Hslice") as "Hslice".
+    repeat (wp_smart_apply assume_spec' as "_").
+    wp_smart_apply (array_unsafe_fill_slice_spec with "Hslice"); [done.. |].
+    iSteps.
+  Qed.
+
+  Lemma array_fill_spec t vs v :
+    {{{
+      array_model t (DfracOwn 1) vs
+    }}}
+      array_fill t v
+    {{{
+      RET ();
+      array_model t (DfracOwn 1) (replicate (length vs) v)
+    }}}.
+  Proof.
+    iIntros "%Φ Hmodel HΦ".
+    wp_rec.
+    wp_smart_apply (array_size_spec with "Hmodel") as "Hmodel".
+    wp_apply (array_unsafe_fill_slice_spec with "Hmodel") as "model"; [done.. |].
+    iApply "HΦ".
+    rewrite Nat2Z.id -{1}(replicate_length (length vs) v) //.
+  Qed.
+
+  Lemma array_unsafe_make_spec sz v :
+    (0 ≤ sz)%Z →
+    {{{ True }}}
+      array_unsafe_make #sz v
+    {{{ t,
+      RET t;
+      array_model t (DfracOwn 1) (replicate (Z.to_nat sz) v)
+    }}}.
+  Proof.
+    iIntros "% %Φ _ HΦ".
+    wp_rec.
+    wp_smart_apply (array_unsafe_alloc_spec with "[//]") as "%t Hmodel"; first done.
+    wp_smart_apply (array_fill_spec with "Hmodel").
+    rewrite replicate_length . iSteps.
+  Qed.
   Lemma array_make_spec sz v :
     (0 ≤ sz)%Z →
     {{{ True }}}
@@ -1098,19 +1658,1104 @@ Section zoo_G.
     }}}.
   Proof.
     iIntros "% %Φ _ HΦ".
-    Z_to_nat sz.
     wp_rec.
     wp_smart_apply assume_spec' as "_".
-    wp_smart_apply (chunk_make_spec with "[//]") as "%l (Hmodel & _)".
-    wp_pures.
-    rewrite Z.add_1_l -Nat2Z.inj_succ !Nat2Z.id.
-    iDestruct (chunk_model_cons with "Hmodel") as "(Hsz & Hmodel)".
-    iEval (setoid_rewrite <- (location_add_0 l)) in "Hsz".
-    wp_store. wp_pures.
-    iMod (pointsto_persist with "Hsz") as "#Hsz".
-    iApply "HΦ". iExists l.
-    rewrite replicate_length !location_add_0. iSteps.
+    wp_smart_apply (array_unsafe_make_spec with "[//]"); first done.
+    iSteps.
   Qed.
+
+  #[local] Lemma array_foldli_aux_spec i vs Ψ t sz acc fn :
+    i ≤ sz →
+    i = length vs →
+    {{{
+      ▷ Ψ i vs None acc ∗
+      □ (
+        ∀ i vs (o : option val) acc,
+        ⌜i < sz ∧ i = length vs⌝ -∗
+        Ψ i vs o acc -∗
+        match o with
+        | None =>
+            au_load t sz i (λ v,
+              ▷ Ψ i vs (Some v) acc
+            )
+        | Some v =>
+            WP fn acc #i v {{ acc,
+              ▷ Ψ (S i) (vs ++ [v]) None acc
+            }}
+        end
+      )
+    }}}
+      array_foldli_aux t #sz acc fn #i
+    {{{ vs' acc,
+      RET acc;
+      ⌜(length vs + length vs')%nat = sz⌝ ∗
+      Ψ sz (vs ++ vs') None acc
+    }}}.
+  Proof.
+    iIntros "%Hi1 %Hi2 %Φ (HΨ & #H) HΦ".
+    remember (sz - i) as j eqn:Hj.
+    iInduction j as [| j] "IH" forall (i vs acc Hi1 Hi2 Hj).
+    all: wp_rec; wp_pures.
+    - rewrite bool_decide_eq_true_2; first (repeat f_equal; lia). wp_pures.
+      iApply ("HΦ" $! []).
+      rewrite !right_id. assert (sz = i) as -> by lia. iSteps.
+    - rewrite bool_decide_eq_false_2; first naive_solver lia. wp_pures.
+      iDestruct ("H" with "[%] HΨ") as "H'"; first lia.
+      awp_smart_apply (array_unsafe_get_spec_atomic_cell with "[//]") without "HΦ".
+      iApply (aacc_aupd_commit with "H'"); first done. iIntros "%dq %v H↦".
+      rewrite /atomic_acc /= Nat2Z.id.
+      repeat iExists _. iFrame. iStep 2; first iSteps. iIntros "$ !> HΨ !> H£ HΦ".
+      iMod (lc_fupd_elim_later with "H£ HΨ") as "HΨ".
+      wp_smart_apply (wp_wand with "(H [%] HΨ)") as "%acc' HΨ"; first lia.
+      rewrite Z.add_1_l -Nat2Z.inj_succ.
+      wp_apply ("IH" with "[%] [%] [%] HΨ [HΦ]"); rewrite ?app_length; [naive_solver lia.. |].
+      clear acc. iIntros "!> %vs' %acc (<- & HΨ)".
+      iApply ("HΦ" $! (v :: vs')).
+      rewrite -(assoc (++)). iSteps.
+  Qed.
+  Lemma array_foldli_spec_atomic Ψ t sz acc fn :
+    {{{
+      array_inv t sz ∗
+      ▷ Ψ 0 [] None acc ∗
+      □ (
+        ∀ i vs (o : option val) acc,
+        ⌜i < sz ∧ i = length vs⌝ -∗
+        Ψ i vs o acc -∗
+        match o with
+        | None =>
+            au_load t sz i (λ v,
+              ▷ Ψ i vs (Some v) acc
+            )
+        | Some v =>
+            WP fn acc #i v {{ acc,
+              ▷ Ψ (S i) (vs ++ [v]) None acc
+            }}
+        end
+      )
+    }}}
+      array_foldli t acc fn
+    {{{ vs acc,
+      RET acc;
+      ⌜length vs = sz⌝ ∗
+      Ψ sz vs None acc
+    }}}.
+  Proof.
+    iIntros "%Φ (#Hinv & HΨ & #H) HΦ".
+    wp_rec.
+    wp_smart_apply (array_size_spec_inv with "Hinv") as "_".
+    rewrite -Nat2Z.inj_0.
+    wp_apply (array_foldli_aux_spec 0 [] Ψ with "[$HΨ] HΦ"); [lia | done |].
+    iSteps.
+  Qed.
+  Lemma array_foldli_spec Ψ t dq vs acc fn :
+    {{{
+      ▷ Ψ 0 [] acc ∗
+      array_model t dq vs ∗
+      □ (
+        ∀ i v acc,
+        ⌜vs !! i = Some v⌝ -∗
+        Ψ i (take i vs) acc -∗
+        WP fn acc #i v {{ acc,
+          ▷ Ψ (S i) (take i vs ++ [v]) acc
+        }}
+      )
+    }}}
+      array_foldli t acc fn
+    {{{ acc,
+      RET acc;
+      array_model t dq vs ∗
+      Ψ (length vs) vs acc
+    }}}.
+  Proof.
+    iIntros "%Φ (HΨ & Hmodel & #Hfn) HΦ".
+    iDestruct (array_model_to_inv with "Hmodel") as "#Hinv".
+    pose (Ψ' i vs_left o acc := (
+      ⌜vs_left = take i vs⌝ ∗
+      array_model t dq vs ∗
+      Ψ i vs_left acc ∗
+      ⌜from_option (λ v, v = vs !!! i) True o⌝%I
+    )%I).
+    wp_apply (array_foldli_spec_atomic Ψ' with "[$Hinv $Hmodel $HΨ]"); last first.
+    { clear acc. iIntros "%vs_left %acc (%Hvs_left & (-> & Hmodel & HΨ & _))".
+      rewrite /Ψ' firstn_all2 //.
+      iApply ("HΦ" with "[$Hmodel $HΨ]").
+    }
+    iStep. clear acc. iIntros "!> %i %vs_left %o %acc (%Hi1 & %Hi2) (-> & Hmodel & HΨ & %Ho)".
+    opose proof* (list_lookup_lookup_total_lt vs i); first lia.
+    destruct o as [v |].
+    - rewrite Ho.
+      wp_apply (wp_wand with "(Hfn [] HΨ)"); first iSteps. clear acc. iIntros "%acc HΨ". iFrame.
+      erewrite take_S_r; done.
+    - iDestruct (array_model_lookup_acc i with "Hmodel") as "(H↦ & Hmodel)"; first done.
+      iAuIntro. iAaccIntro with "H↦"; iSteps.
+  Qed.
+  Lemma array_foldli_spec' Ψ t dq vs acc fn :
+    {{{
+      ▷ Ψ 0 [] acc ∗
+      array_model t dq vs ∗
+      ( [∗ list] i ↦ v ∈ vs,
+        ∀ acc,
+        Ψ i (take i vs) acc -∗
+        WP fn acc #i v {{ acc,
+          ▷ Ψ (S i) (take i vs ++ [v]) acc
+        }}
+      )
+    }}}
+      array_foldli t acc fn
+    {{{ acc,
+      RET acc;
+      array_model t dq vs ∗
+      Ψ (length vs) vs acc
+    }}}.
+  Proof.
+    iIntros "%Φ (HΨ & Hmodel & Hfn) HΦ".
+    match goal with |- context [big_opL bi_sep ?Ξ' _] => set Ξ := Ξ' end.
+    pose (Ψ' i vs_left acc := (
+      Ψ i vs_left acc ∗
+      [∗ list] j ↦ v ∈ drop i vs, Ξ (i + j) v
+    )%I).
+    wp_apply (array_foldli_spec Ψ' with "[$HΨ $Hmodel $Hfn]"); last iSteps.
+    clear acc. iIntros "!> %i %v %acc %Hlookup (HΨ & HΞ)".
+    erewrite drop_S; last done.
+    iDestruct "HΞ" as "(Hfn & HΞ)".
+    rewrite Nat.add_0_r. setoid_rewrite Nat.add_succ_r. iSteps.
+  Qed.
+
+  Lemma array_foldl_spec_atomic Ψ t sz acc fn :
+    {{{
+      array_inv t sz ∗
+      ▷ Ψ 0 [] None acc ∗
+      □ (
+        ∀ i vs (o : option val) acc,
+        ⌜i < sz ∧ i = length vs⌝ -∗
+        Ψ i vs o acc -∗
+        match o with
+        | None =>
+            au_load t sz i (λ v,
+              ▷ Ψ i vs (Some v) acc
+            )
+        | Some v =>
+            WP fn acc v {{ acc,
+              ▷ Ψ (S i) (vs ++ [v]) None acc
+            }}
+        end
+      )
+    }}}
+      array_foldl t acc fn
+    {{{ vs acc,
+      RET acc;
+      ⌜length vs = sz⌝ ∗
+      Ψ sz vs None acc
+    }}}.
+  Proof.
+    iIntros "%Φ (#Hinv & HΨ & #H) HΦ".
+    wp_rec.
+    wp_smart_apply (array_foldli_spec_atomic Ψ with "[$Hinv $HΨ] HΦ"). clear acc. iIntros "!> %i %vs %o %acc %Hi HΨ".
+    case_match; try wp_pures; iApply ("H" with "[//] HΨ").
+  Qed.
+  Lemma array_foldl_spec Ψ t dq vs acc fn :
+    {{{
+      ▷ Ψ 0 [] acc ∗
+      array_model t dq vs ∗
+      □ (
+        ∀ i v acc,
+        ⌜vs !! i = Some v⌝ -∗
+        Ψ i (take i vs) acc -∗
+        WP fn acc v {{ acc,
+          ▷ Ψ (S i) (take i vs ++ [v]) acc
+        }}
+      )
+    }}}
+      array_foldl t acc fn
+    {{{ acc,
+      RET acc;
+      array_model t dq vs ∗
+      Ψ (length vs) vs acc
+    }}}.
+  Proof.
+    iIntros "%Φ (HΨ & Hmodel & #Hfn) HΦ".
+    wp_rec.
+    wp_smart_apply (array_foldli_spec Ψ with "[$HΨ $Hmodel] HΦ").
+    iSteps.
+  Qed.
+  Lemma array_foldl_spec' Ψ t dq vs acc fn :
+    {{{
+      ▷ Ψ 0 [] acc ∗
+      array_model t dq vs ∗
+      ( [∗ list] i ↦ v ∈ vs,
+        ∀ acc,
+        Ψ i (take i vs) acc -∗
+        WP fn acc v {{ acc,
+          ▷ Ψ (S i) (take i vs ++ [v]) acc
+        }}
+      )
+    }}}
+      array_foldl t acc fn
+    {{{ acc,
+      RET acc;
+      array_model t dq vs ∗
+      Ψ (length vs) vs acc
+    }}}.
+  Proof.
+    iIntros "%Φ (HΨ & Hmodel & Hfn) HΦ".
+    wp_rec.
+    wp_smart_apply (array_foldli_spec' Ψ with "[$HΨ $Hmodel Hfn] HΦ").
+    iApply (big_sepL_impl with "Hfn").
+    iSteps.
+  Qed.
+
+  #[local] Lemma array_foldri_aux_spec sz (i : Z) vs Ψ t fn acc :
+    Z.to_nat i + length vs = sz →
+    {{{
+      ▷ Ψ (Z.to_nat i) acc None vs ∗
+      □ (
+        ∀ i acc (o : option val) vs,
+        ⌜(S i + length vs)%nat = sz⌝ -∗
+        Ψ (S i) acc o vs -∗
+        match o with
+        | None =>
+            au_load t sz i (λ v,
+              ▷ Ψ (S i) acc (Some v) vs
+            )
+        | Some v =>
+            WP fn #i v acc {{ acc,
+              ▷ Ψ i acc None (v :: vs)
+            }}
+        end
+      )
+    }}}
+      array_foldri_aux t fn acc #i
+    {{{ acc vs',
+      RET acc;
+      ⌜(length vs' + length vs)%nat = sz⌝ ∗
+      Ψ 0 acc None (vs' ++ vs)
+    }}}.
+  Proof.
+    iIntros "%Hi %Φ (HΨ & #H) HΦ".
+    remember (Z.to_nat i) as j eqn:Hj.
+    iInduction j as [| j] "IH" forall (i vs acc Hi Hj);
+      wp_rec; wp_pures credit:"H£".
+    - rewrite bool_decide_eq_true_2; first lia. wp_pures.
+      iApply ("HΦ" $! _ []).
+      iSteps.
+    - rewrite bool_decide_eq_false_2; first lia. wp_pures.
+      assert (i = S j) as -> by lia. rewrite Z.sub_1_r -Nat2Z.inj_pred /=; first lia.
+      iDestruct ("H" with "[%] HΨ") as "H'"; first done.
+      awp_smart_apply (array_unsafe_get_spec_atomic_cell with "[//]") without "HΦ".
+      iApply (aacc_aupd_commit with "H'"); first done. iIntros "%dq %v H↦".
+      rewrite /atomic_acc /= Nat2Z.id.
+      repeat iExists _. iFrame. iStep 2; first iSteps. iIntros "$ !> HΨ !> H£ HΦ".
+      iMod (lc_fupd_elim_later with "H£ HΨ") as "HΨ".
+      wp_smart_apply (wp_wand with "(H [%] HΨ)") as "%acc' HΨ"; first lia.
+      wp_apply ("IH" with "[] [] HΨ [HΦ]"); rewrite ?app_length; [iSteps.. |]. clear acc. iIntros "!> %acc %vs' (<- & HΨ)".
+      iApply ("HΦ" $! _ (vs' ++ [v])).
+      rewrite app_length -(assoc (++)). iSteps.
+  Qed.
+  Lemma array_foldri_spec_atomic Ψ t sz fn acc :
+    {{{
+      array_inv t sz ∗
+      ▷ Ψ sz acc None [] ∗
+      □ (
+        ∀ i acc (o : option val) vs,
+        ⌜(S i + length vs)%nat = sz⌝ -∗
+        Ψ (S i) acc o vs -∗
+        match o with
+        | None =>
+            au_load t sz i (λ v,
+              ▷ Ψ (S i) acc (Some v) vs
+            )
+        | Some v =>
+            WP fn #i v acc {{ acc,
+              ▷ Ψ i acc None (v :: vs)
+            }}
+        end
+      )
+    }}}
+      array_foldri t fn acc
+    {{{ acc vs,
+      RET acc;
+      ⌜length vs = sz⌝ ∗
+      Ψ 0 acc None vs
+    }}}.
+  Proof.
+    iIntros "%Φ (#Hinv & HΨ & #H) HΦ".
+    wp_rec.
+    wp_smart_apply (array_size_spec_inv with "Hinv") as "_".
+    wp_apply (array_foldri_aux_spec sz sz [] Ψ with "[HΨ $H]").
+    { rewrite right_id. lia. }
+    { rewrite Nat2Z.id //. }
+    clear acc. iIntros "%acc %vs".
+    rewrite !right_id. iSteps.
+  Qed.
+  Lemma array_foldri_spec Ψ t dq vs fn acc :
+    {{{
+      array_model t dq vs ∗
+      ▷ Ψ (length vs) acc [] ∗
+      □ (
+        ∀ i v acc,
+        ⌜vs !! i = Some v⌝ -∗
+        Ψ (S i) acc (drop (S i) vs) -∗
+        WP fn #i v acc {{ acc,
+          ▷ Ψ i acc (v :: drop (S i) vs)
+        }}
+      )
+    }}}
+      array_foldri t fn acc
+    {{{ acc,
+      RET acc;
+      Ψ 0 acc vs ∗
+      array_model t dq vs
+    }}}.
+  Proof.
+    iIntros "%Φ (Hmodel & HΨ & #Hfn) HΦ".
+    iDestruct (array_model_to_inv with "Hmodel") as "#Hinv".
+    pose (Ψ' i acc o vs_right := (
+      ⌜vs_right = drop i vs⌝ ∗
+      array_model t dq vs ∗
+      Ψ i acc vs_right ∗
+      ⌜from_option (λ v, v = vs !!! (i - 1)) True o⌝%I
+    )%I).
+    wp_apply (array_foldri_spec_atomic Ψ' with "[$Hinv $Hmodel $HΨ]"); last iSteps.
+    iSplitR.
+    - rewrite drop_all. iSteps.
+    - clear acc. iIntros "!> %i %acc %o %vs_right %Hi (-> & Hmodel & HΨ & %Ho)".
+      opose proof* (list_lookup_lookup_total_lt vs i) as Hlookup; first lia.
+      destruct o as [v |].
+      + rewrite Ho.
+        wp_apply (wp_wand with "(Hfn [] HΨ)").
+        { iPureIntro. rewrite Hlookup. repeat f_equal. lia. }
+        clear acc. iIntros "%acc HΨ". iFrame.
+        iPureIntro. rewrite -drop_S ?Hlookup; repeat f_equal; lia.
+      + iDestruct (array_model_lookup_acc i with "Hmodel") as "(H↦ & Hmodel)"; first done.
+        iAuIntro. iAaccIntro with "H↦"; first iSteps. iIntros "H↦ !>".
+        iSteps; iPureIntro; rewrite drop_length; f_equal; lia.
+  Qed.
+  Lemma array_foldri_spec' Ψ t dq vs fn acc :
+    {{{
+      array_model t dq vs ∗
+      ▷ Ψ (length vs) acc [] ∗
+      ( [∗ list] i ↦ v ∈ vs,
+        ∀ acc,
+        Ψ (S i) acc (drop (S i) vs) -∗
+        WP fn #i v acc {{ acc,
+          ▷ Ψ i acc (v :: drop (S i) vs)
+        }}
+      )
+    }}}
+      array_foldri t fn acc
+    {{{ acc,
+      RET acc;
+      Ψ 0 acc vs ∗
+      array_model t dq vs
+    }}}.
+  Proof.
+    iIntros "%Φ (Hmodel & HΨ & Hfn) HΦ".
+    match goal with |- context [big_opL bi_sep ?Ξ' _] => set Ξ := Ξ' end.
+    pose (Ψ' i acc vs_right := (
+      Ψ i acc vs_right ∗
+      [∗ list] j ↦ v ∈ take i vs, Ξ j v
+    )%I).
+    wp_apply (array_foldri_spec Ψ' with "[$Hmodel HΨ Hfn]"); last iSteps.
+    iFrame. rewrite firstn_all2; first lia. iFrame.
+    clear acc. iIntros "!> %i %v %acc %Hlookup (HΨ & HΞ)".
+    pose proof Hlookup as Hi%lookup_lt_Some.
+    erewrite take_S_r; last done.
+    iDestruct "HΞ" as "(HΞ & Hfn & _)".
+    rewrite Nat.add_0_r take_length Nat.min_l; first lia. iSteps.
+  Qed.
+
+  Lemma array_foldr_spec_atomic Ψ t sz fn acc :
+    {{{
+      array_inv t sz ∗
+      ▷ Ψ sz acc None [] ∗
+      □ (
+        ∀ i acc (o : option val) vs,
+        ⌜(S i + length vs)%nat = sz⌝ -∗
+        Ψ (S i) acc o vs -∗
+        match o with
+        | None =>
+            au_load t sz i (λ v,
+              ▷ Ψ (S i) acc (Some v) vs
+            )
+        | Some v =>
+            WP fn v acc {{ acc,
+              ▷ Ψ i acc None (v :: vs)
+            }}
+        end
+      )
+    }}}
+      array_foldr t fn acc
+    {{{ acc vs,
+      RET acc;
+      ⌜length vs = sz⌝ ∗
+      Ψ 0 acc None vs
+    }}}.
+  Proof.
+    iIntros "%Φ (#Hinv & HΨ & #H) HΦ".
+    wp_rec.
+    wp_smart_apply (array_foldri_spec_atomic Ψ with "[$Hinv $HΨ] HΦ"). clear acc. iIntros "!> %i %acc %o %vs %Hi HΨ".
+    case_match; try wp_pures; iApply ("H" with "[//] HΨ").
+  Qed.
+  Lemma array_foldr_spec Ψ t dq vs fn acc :
+    {{{
+      array_model t dq vs ∗
+      ▷ Ψ (length vs) acc [] ∗
+      □ (
+        ∀ i v acc,
+        ⌜vs !! i = Some v⌝ -∗
+        Ψ (S i) acc (drop (S i) vs) -∗
+        WP fn v acc {{ acc,
+          ▷ Ψ i acc (v :: drop (S i) vs)
+        }}
+      )
+    }}}
+      array_foldr t fn acc
+    {{{ acc,
+      RET acc;
+      Ψ 0 acc vs ∗
+      array_model t dq vs
+    }}}.
+  Proof.
+    iIntros "%Φ (Hmodel & HΨ & #Hfn) HΦ".
+    wp_rec.
+    wp_smart_apply (array_foldri_spec Ψ with "[$Hmodel $HΨ] HΦ").
+    iSteps.
+  Qed.
+  Lemma array_foldr_spec' Ψ t dq vs fn acc :
+    {{{
+      array_model t dq vs ∗
+      ▷ Ψ (length vs) acc [] ∗
+      ( [∗ list] i ↦ v ∈ vs,
+        ∀ acc,
+        Ψ (S i) acc (drop (S i) vs) -∗
+        WP fn v acc {{ acc,
+          ▷ Ψ i acc (v :: drop (S i) vs)
+        }}
+      )
+    }}}
+      array_foldr t fn acc
+    {{{ acc,
+      RET acc;
+      Ψ 0 acc vs ∗
+      array_model t dq vs
+    }}}.
+  Proof.
+    iIntros "%Φ (Hmodel & HΨ & Hfn) HΦ".
+    wp_rec.
+    wp_smart_apply (array_foldri_spec' Ψ with "[$Hmodel $HΨ Hfn] HΦ").
+    iApply (big_sepL_impl with "Hfn").
+    iSteps.
+  Qed.
+
+  Lemma array_iteri_spec_atomic Ψ t sz fn :
+    {{{
+      array_inv t sz ∗
+      ▷ Ψ 0 [] None ∗
+      □ (
+        ∀ i vs (o : option val),
+        ⌜i < sz ∧ i = length vs⌝ -∗
+        Ψ i vs o -∗
+        match o with
+        | None =>
+            au_load t sz i (λ v,
+              ▷ Ψ i vs (Some v)
+            )
+        | Some v =>
+            WP fn #i v {{ res,
+              ⌜res = ()%V⌝ ∗
+              ▷ Ψ (S i) (vs ++ [v]) None
+            }}
+        end
+      )
+    }}}
+      array_iteri t fn
+    {{{ vs,
+      RET ();
+      ⌜length vs = sz⌝ ∗
+      Ψ sz vs None
+    }}}.
+  Proof.
+    iIntros "%Φ (#Hinv & HΨ & #H) HΦ".
+    wp_rec.
+    wp_smart_apply (array_size_spec_inv with "Hinv") as "_".
+    pose Ψ' (_ : Z) i := (
+      ∃ vs,
+      ⌜length vs = i⌝ ∗
+      Ψ i vs None
+    )%I.
+    wp_smart_apply (for_upto_spec_strong Ψ' with "[HΨ]").
+    { iSplitL. { iExists []. iSteps. }
+      iIntros "!> %i_ %i (-> & %Hi) (%vs & %Hvs & HΨ)". rewrite Z.add_0_l in Hi |- *.
+      iDestruct ("H" with "[%] HΨ") as "H'"; first lia.
+      awp_smart_apply (array_unsafe_get_spec_atomic_cell with "[//]").
+      iApply (aacc_aupd_commit with "H'"); first done. iIntros "%dq %v H↦".
+      rewrite /atomic_acc /= Nat2Z.id.
+      repeat iExists _. iStep 2; first iSteps. iIntros "$ !> HΨ !> H£".
+      iMod (lc_fupd_elim_later with "H£ HΨ") as "HΨ".
+      wp_smart_apply (wp_wand with "(H [%] HΨ)") as "%acc' (-> & HΨ)"; first lia.
+      iSteps. iExists (vs ++ [v]). rewrite app_length. iSteps.
+    }
+    rewrite Z.sub_0_r Nat2Z.id. iSteps.
+  Qed.
+  Lemma array_iteri_spec Ψ t dq vs fn :
+    {{{
+      ▷ Ψ 0 [] ∗
+      array_model t dq vs ∗
+      □ (
+        ∀ i v,
+        ⌜vs !! i = Some v⌝ -∗
+        Ψ i (take i vs) -∗
+        WP fn #i v {{ res,
+          ⌜res = ()%V⌝ ∗
+          ▷ Ψ (S i) (take i vs ++ [v])
+        }}
+      )
+    }}}
+      array_iteri t fn
+    {{{
+      RET ();
+      array_model t dq vs ∗
+      Ψ (length vs) vs
+    }}}.
+  Proof.
+    iIntros "%Φ (HΨ & Hmodel & #Hfn) HΦ".
+    iDestruct (array_model_to_inv with "Hmodel") as "#Hinv".
+    pose (Ψ' i vs_left o := (
+      ⌜vs_left = take i vs⌝ ∗
+      array_model t dq vs ∗
+      Ψ i vs_left ∗
+      ⌜from_option (λ v, v = vs !!! i) True o⌝%I
+    )%I).
+    wp_smart_apply (array_iteri_spec_atomic Ψ' with "[$Hinv $Hmodel $HΨ]"); last first.
+    { iSteps. rewrite firstn_all //. }
+    iStep. iIntros "!> %i %vs_left %o (%Hi1 & %Hi2) (-> & Hmodel & HΨ & %Ho)".
+    opose proof* (list_lookup_lookup_total_lt vs i); first lia.
+    destruct o as [v |].
+    - rewrite Ho.
+      wp_apply (wp_wand with "(Hfn [] HΨ)") as (res) "(-> & HΨ)"; first iSteps.
+      iSteps. erewrite take_S_r; done.
+    - iDestruct (array_model_lookup_acc i with "Hmodel") as "(H↦ & Hmodel)"; first done.
+      iAuIntro. iAaccIntro with "H↦"; iSteps.
+  Qed.
+  Lemma array_iteri_spec' Ψ t dq vs fn :
+    {{{
+      ▷ Ψ 0 [] ∗
+      array_model t dq vs ∗
+      ( [∗ list] i ↦ v ∈ vs,
+        Ψ i (take i vs) -∗
+        WP fn #i v {{ res,
+          ⌜res = ()%V⌝ ∗
+          ▷ Ψ (S i) (take i vs ++ [v])
+        }}
+      )
+    }}}
+      array_iteri t fn
+    {{{
+      RET ();
+      array_model t dq vs ∗
+      Ψ (length vs) vs
+    }}}.
+  Proof.
+    iIntros "%Φ (HΨ & Hmodel & Hfn) HΦ".
+    match goal with |- context [big_opL bi_sep ?Ξ' _] => set Ξ := Ξ' end.
+    pose (Ψ' i vs_left := (
+      Ψ i vs_left ∗
+      [∗ list] j ↦ v ∈ drop i vs, Ξ (i + j) v
+    )%I).
+    wp_apply (array_iteri_spec Ψ' with "[$HΨ $Hmodel $Hfn]"); last iSteps.
+    iIntros "!> %i %v %Hlookup (HΨ & HΞ)".
+    erewrite drop_S; last done.
+    iDestruct "HΞ" as "(Hfn & HΞ)".
+    rewrite Nat.add_0_r. setoid_rewrite Nat.add_succ_r. iSteps.
+  Qed.
+  Lemma array_iteri_spec_disentangled Ψ t dq vs fn :
+    {{{
+      array_model t dq vs ∗
+      □ (
+        ∀ i v,
+        ⌜vs !! i = Some v⌝ -∗
+        WP fn #i v {{ res,
+          ⌜res = ()%V⌝ ∗
+          ▷ Ψ i v
+        }}
+      )
+    }}}
+      array_iteri t fn
+    {{{
+      RET ();
+      array_model t dq vs ∗
+      ( [∗ list] i ↦ v ∈ vs,
+        Ψ i v
+      )
+    }}}.
+  Proof.
+    iIntros "%Φ (Hmodel & #Hfn) HΦ".
+    pose (Ψ' i vs := (
+      [∗ list] j ↦ v ∈ vs, Ψ j v
+    )%I).
+    wp_apply (array_iteri_spec Ψ' with "[$Hmodel]"); last iSteps.
+    rewrite /Ψ'. iSteps.
+    rewrite big_sepL_snoc take_length Nat.min_l; last iSteps.
+    eapply Nat.lt_le_incl, lookup_lt_Some. done.
+  Qed.
+  Lemma array_iteri_spec_disentangled' Ψ t dq vs fn :
+    {{{
+      array_model t dq vs ∗
+      ( [∗ list] i ↦ v ∈ vs,
+        WP fn #i v {{ res,
+          ⌜res = ()%V⌝ ∗
+          ▷ Ψ i v
+        }}
+      )
+    }}}
+      array_iteri t fn
+    {{{
+      RET ();
+      array_model t dq vs ∗
+      ( [∗ list] i ↦ v ∈ vs,
+        Ψ i v
+      )
+    }}}.
+  Proof.
+    iIntros "%Φ (Hmodel & Hfn) HΦ".
+    pose (Ψ' i vs := (
+      [∗ list] j ↦ v ∈ vs, Ψ j v
+    )%I).
+    wp_apply (array_iteri_spec' Ψ' with "[$Hmodel Hfn]"); last iSteps.
+    rewrite /Ψ'. iSteps.
+    iApply (big_sepL_impl with "Hfn"). iSteps.
+    rewrite big_sepL_snoc take_length Nat.min_l; last iSteps.
+    eapply Nat.lt_le_incl, lookup_lt_Some. done.
+  Qed.
+
+  Lemma array_iter_spec_atomic Ψ t sz fn :
+    {{{
+      array_inv t sz ∗
+      ▷ Ψ 0 [] None ∗
+      □ (
+        ∀ i vs (o : option val),
+        ⌜i < sz ∧ i = length vs⌝ -∗
+        Ψ i vs o -∗
+        match o with
+        | None =>
+            au_load t sz i (λ v,
+              ▷ Ψ i vs (Some v)
+            )
+        | Some v =>
+            WP fn v {{ res,
+              ⌜res = ()%V⌝ ∗
+              ▷ Ψ (S i) (vs ++ [v]) None
+            }}
+        end
+      )
+    }}}
+      array_iter t fn
+    {{{ vs,
+      RET ();
+      ⌜length vs = sz⌝ ∗
+      Ψ sz vs None
+    }}}.
+  Proof.
+    iIntros "%Φ (#Hinv & HΨ & #H) HΦ".
+    wp_rec.
+    wp_smart_apply (array_iteri_spec_atomic Ψ with "[$Hinv $HΨ] HΦ") as "!> %i %vs %o %Hi HΨ".
+    case_match; try wp_pures; iApply ("H" with "[//] HΨ").
+  Qed.
+  Lemma array_iter_spec Ψ t dq vs fn :
+    {{{
+      ▷ Ψ 0 [] ∗
+      array_model t dq vs ∗
+      □ (
+        ∀ i v,
+        ⌜vs !! i = Some v⌝ -∗
+        Ψ i (take i vs) -∗
+        WP fn v {{ res,
+          ⌜res = ()%V⌝ ∗
+          ▷ Ψ (S i) (take i vs ++ [v])
+        }}
+      )
+    }}}
+      array_iter t fn
+    {{{
+      RET ();
+      array_model t dq vs ∗
+      Ψ (length vs) vs
+    }}}.
+  Proof.
+    iIntros "%Φ (HΨ & Hmodel & #Hfn) HΦ".
+    wp_rec.
+    wp_smart_apply (array_iteri_spec Ψ with "[$HΨ $Hmodel] HΦ").
+    iSteps.
+  Qed.
+  Lemma array_iter_spec' Ψ t dq vs fn :
+    {{{
+      ▷ Ψ 0 [] ∗
+      array_model t dq vs ∗
+      ( [∗ list] i ↦ v ∈ vs,
+        Ψ i (take i vs) -∗
+        WP fn v {{ res,
+          ⌜res = ()%V⌝ ∗
+          ▷ Ψ (S i) (take i vs ++ [v])
+        }}
+      )
+    }}}
+      array_iter t fn
+    {{{
+      RET ();
+      array_model t dq vs ∗
+      Ψ (length vs) vs
+    }}}.
+  Proof.
+    iIntros "%Φ (HΨ & Hmodel & Hfn) HΦ".
+    wp_rec.
+    wp_smart_apply (array_iteri_spec' Ψ with "[$HΨ $Hmodel Hfn] HΦ").
+    iApply (big_sepL_impl with "Hfn").
+    iSteps.
+  Qed.
+  Lemma array_iter_spec_disentangled Ψ t dq vs fn :
+    {{{
+      array_model t dq vs ∗
+      □ (
+        ∀ i v,
+        ⌜vs !! i = Some v⌝ -∗
+        WP fn v {{ res,
+          ⌜res = ()%V⌝ ∗
+          ▷ Ψ i v
+        }}
+      )
+    }}}
+      array_iter t fn
+    {{{
+      RET ();
+      array_model t dq vs ∗
+      ( [∗ list] i ↦ v ∈ vs,
+        Ψ i v
+      )
+    }}}.
+  Proof.
+    iIntros "%Φ (Hmodel & #Hfn) HΦ".
+    wp_rec.
+    wp_smart_apply (array_iteri_spec_disentangled Ψ with "[$Hmodel] HΦ").
+    iSteps.
+  Qed.
+  Lemma array_iter_spec_disentangled' Ψ t dq vs fn :
+    {{{
+      array_model t dq vs ∗
+      ( [∗ list] i ↦ v ∈ vs,
+        WP fn v {{ res,
+          ⌜res = ()%V⌝ ∗
+          ▷ Ψ i v
+        }}
+      )
+    }}}
+      array_iter t fn
+    {{{
+      RET ();
+      array_model t dq vs ∗
+      ( [∗ list] i ↦ v ∈ vs,
+        Ψ i v
+      )
+    }}}.
+  Proof.
+    iIntros "%Φ (Hmodel & Hfn) HΦ".
+    wp_rec.
+    wp_smart_apply (array_iteri_spec_disentangled' Ψ with "[$Hmodel Hfn] HΦ").
+    iApply (big_sepL_impl with "Hfn").
+    iSteps.
+  Qed.
+
+  Lemma array_applyi_spec_atomic Ψ t sz fn :
+    {{{
+      array_inv t sz ∗
+      ▷ Ψ 0 [] None [] ∗
+      □ (
+        ∀ i vs (o : option (val + val * val)) ws,
+        ⌜i < sz ∧ i = length vs ∧ length vs = length ws⌝ -∗
+        Ψ i vs o ws -∗
+        match o with
+        | None =>
+            au_load t sz i (λ v,
+              ▷ Ψ i vs (Some $ inl v) ws
+            )
+        | Some (inl v) =>
+            WP fn #i v {{ w,
+              ▷ Ψ i vs (Some $ inr (v, w)) ws
+            }}
+        | Some (inr (v, w)) =>
+            au_store t sz i w (
+              ▷ Ψ (S i) (vs ++ [v]) None (ws ++ [w])
+            )
+        end
+      )
+    }}}
+      array_applyi t fn
+    {{{ vs ws,
+      RET ();
+      ⌜length vs = sz ∧ length vs = length ws⌝ ∗
+      Ψ sz vs None ws
+    }}}.
+  Proof.
+    iIntros "%Φ (#Hinv & HΨ & #H) HΦ".
+    wp_rec.
+    pose (Ψ' i vs o := (
+      ∃ ws,
+      ⌜length vs = length ws⌝ ∗
+      Ψ i vs (inl <$> o) ws
+    )%I).
+    wp_smart_apply (array_iteri_spec_atomic Ψ' with "[$Hinv HΨ]"); last iSteps.
+    iSplitL "HΨ". { iExists []. iSteps. }
+    iIntros "!> %i %vs %o (%Hi1 & %Hi2) (%ws & %Hws & HΨ)".
+    destruct o as [v |].
+    - wp_smart_apply (wp_wand with "(H [//] HΨ)") as "%w HΨ".
+      wp_rec. wp_pures.
+      iMod ("H" with "[//] HΨ") as "(%v' & H↦ & _ & H')".
+      rewrite /array_slice. setoid_rewrite <- chunk_model_singleton.
+      iDestruct "H↦" as "(%l & -> & #Hhdr & H↦)".
+      wp_store.
+      iStep. iExists (ws ++ [w]).
+      iMod ("H'" with "[H↦]") as "$"; first iSteps.
+      rewrite !app_length. iSteps.
+    - iApply (atomic_update_wand with "(H [//] HΨ)").
+      iSteps.
+  Qed.
+  Lemma array_applyi_spec Ψ t vs fn :
+    {{{
+      ▷ Ψ 0 [] [] ∗
+      array_model t (DfracOwn 1) vs ∗
+      □ (
+        ∀ i v ws,
+        ⌜i = length ws ∧ vs !! i = Some v⌝ -∗
+        Ψ i (take i vs) ws -∗
+        WP fn #i v {{ w,
+          ▷ Ψ (S i) (take i vs ++ [v]) (ws ++ [w])
+        }}
+      )
+    }}}
+      array_applyi t fn
+    {{{ ws,
+      RET ();
+      ⌜length vs = length ws⌝ ∗
+      array_model t (DfracOwn 1) ws ∗
+      Ψ (length vs) vs ws
+    }}}.
+  Proof.
+    iIntros "%Φ (HΨ & Hmodel & #Hfn) HΦ".
+    iDestruct (array_model_to_inv with "Hmodel") as "#Hinv".
+    pose (Ψ' i vs_left o ws := (
+      ⌜vs_left = take i vs⌝ ∗
+      array_model t (DfracOwn 1) (ws ++ drop i vs) ∗
+      match o with
+      | None =>
+          Ψ i vs_left ws
+      | Some (inl v) =>
+          ⌜v = vs !!! i⌝ ∗
+          Ψ i vs_left ws
+      | Some (inr (v, w)) =>
+          ⌜v = vs !!! i⌝ ∗
+          Ψ (S i) (vs_left ++ [v]) (ws ++ [w])
+      end
+    )%I).
+    wp_apply (array_applyi_spec_atomic Ψ' with "[$Hinv $HΨ $Hmodel]"); last first.
+    { iIntros "%vs_left %ws ((%Hvs_left_1 & %Hws) & (-> & Hmodel & HΨ))".
+      rewrite firstn_all2; first lia. rewrite skipn_all2; first lia. rewrite right_id.
+      iApply ("HΦ" $! ws). iSteps.
+    }
+    iStep. iIntros "!> %i %vs_left %o %ws (%Hvs_left & %Hi & %Hws) (-> & Hmodel & HΨ)".
+    opose proof* (list_lookup_lookup_total_lt vs i); first lia.
+    destruct o as [[v | (v & w)] |].
+    - iDestruct "HΨ" as "(-> & HΨ)".
+      wp_apply (wp_wand with "(Hfn [] HΨ)"); iSteps.
+    - iDestruct "HΨ" as "(-> & HΨ)".
+      assert ((ws ++ drop i vs) !! i = Some (vs !!! i)).
+      { rewrite lookup_app_r; first lia.
+        rewrite lookup_drop list_lookup_lookup_total_lt; first lia.
+        repeat f_equal. lia.
+      }
+      iDestruct (array_model_update i with "Hmodel") as "(H↦ & Hmodel)"; first done.
+      iAuIntro. iAaccIntro with "H↦"; first iSteps. iIntros "H↦ !>". iFrame.
+      iSplit; first rewrite -take_S_r //.
+      iDestruct ("Hmodel" with "H↦") as "Hmodel".
+      rewrite insert_app_r_alt; first lia.
+      erewrite drop_S; last done.
+      rewrite Hi Hws Nat.sub_diag -assoc //.
+    - assert ((ws ++ drop i vs) !! i = Some (vs !!! i)).
+      { rewrite lookup_app_r; first lia.
+        rewrite lookup_drop list_lookup_lookup_total_lt; first lia.
+        repeat f_equal. lia.
+      }
+      iDestruct (chunk_model_lookup_acc i with "Hmodel") as "(H↦ & Hmodel)"; [lia | done | lia |].
+      iAuIntro. iAaccIntro with "H↦"; iSteps.
+  Qed.
+  Lemma array_applyi_spec' Ψ t vs fn :
+    {{{
+      ▷ Ψ 0 [] [] ∗
+      array_model t (DfracOwn 1) vs ∗
+      ( [∗ list] i ↦ v ∈ vs,
+        ∀ ws,
+        ⌜i = length ws⌝ -∗
+        Ψ i (take i vs) ws -∗
+        WP fn #i v {{ w,
+          ▷ Ψ (S i) (take i vs ++ [v]) (ws ++ [w])
+        }}
+      )
+    }}}
+      array_applyi t fn
+    {{{ ws,
+      RET ();
+      ⌜length vs = length ws⌝ ∗
+      array_model t (DfracOwn 1) ws ∗
+      Ψ (length vs) vs ws
+    }}}.
+  Proof.
+    iIntros "%Hsz %Φ (HΨ & Hmodel & Hfn) HΦ".
+    match goal with |- context [big_opL bi_sep ?Ξ' _] => set Ξ := Ξ' end.
+    pose (Ψ' i vs_left ws := (
+      Ψ i vs_left ws ∗
+      [∗ list] j ↦ v ∈ drop i vs, Ξ (i + j) v
+    )%I).
+    wp_apply (chunk_applyi_spec Ψ' with "[HΨ $Hmodel Hfn]"); [done | | iSteps].
+    iFrame. iIntros "!> %i %v %ws (%Hi & %Hlookup) (HΨ & HΞ)".
+    erewrite drop_S; last done.
+    iDestruct "HΞ" as "(Hfn & HΞ)".
+    rewrite Nat.add_0_r. setoid_rewrite Nat.add_succ_r. iSteps.
+  Qed.
+  Lemma array_applyi_spec_disentangled Ψ t vs fn :
+    {{{
+      array_model t (DfracOwn 1) vs ∗
+      □ (
+        ∀ i v,
+        ⌜vs !! i = Some v⌝ -∗
+        WP fn #i v {{ w,
+          ▷ Ψ i w
+        }}
+      )
+    }}}
+      array_applyi t fn
+    {{{ ws,
+      RET ();
+      ⌜length vs = length ws⌝ ∗
+      array_model t (DfracOwn 1) ws ∗
+      ( [∗ list] i ↦ w ∈ ws,
+        Ψ i w
+      )
+    }}}.
+  Proof.
+    iIntros "%Hsz %Φ (Hmodel & #Hfn) HΦ".
+    pose (Ψ' i vs_left ws := (
+      [∗ list] j ↦ w ∈ ws, Ψ j w
+    )%I).
+    wp_apply (chunk_applyi_spec Ψ' with "[$Hmodel]"); [done | | iSteps].
+    rewrite /Ψ'. iSteps.
+    rewrite big_sepL_snoc. iSteps.
+  Qed.
+  Lemma array_applyi_spec_disentangled' Ψ t vs fn :
+    {{{
+      array_model t (DfracOwn 1) vs ∗
+      ( [∗ list] i ↦ v ∈ vs,
+        WP fn #i v {{ w,
+          ▷ Ψ i w
+        }}
+      )
+    }}}
+      array_applyi t fn
+    {{{ ws,
+      RET ();
+      array_model t (DfracOwn 1) ws ∗
+      ( [∗ list] i ↦ w ∈ ws,
+        Ψ i w
+      )
+    }}}.
+  Proof.
+    iIntros "%Hsz %Φ (Hmodel & Hfn) HΦ".
+    pose (Ψ' i vs_left ws := (
+      [∗ list] j ↦ w ∈ ws, Ψ j w
+    )%I).
+    wp_apply (chunk_applyi_spec' Ψ' with "[Hmodel Hfn]"); [done | | iSteps].
+    rewrite /Ψ'. iSteps.
+    iApply (big_sepL_impl with "Hfn"). iSteps.
+    rewrite big_sepL_snoc. iSteps.
+  Qed.
+
+  Proof.
+    iIntros "%Φ (HΨ & (%l & -> & #Hhdr & Hmodel) & Hfn) HΦ".
+    wp_rec. rewrite /array_data /array_size. wp_load.
+    rewrite !location_add_0.
+    wp_smart_apply (chunk_applyi_spec Ψ with "[$HΨ $Hmodel $Hfn]") as (ws) "(-> & Hmodel & HΨ)"; first lia.
+    iSteps. rewrite Nat2Z.id !location_add_0. iSteps.
+  Qed.
+  Proof.
+    iIntros "%Φ (HΨ & (%l & -> & #Hhdr & Hmodel) & Hfn) HΦ".
+    wp_rec. rewrite /array_data /array_size. wp_load.
+    rewrite !location_add_0.
+    wp_smart_apply (chunk_applyi_spec' Ψ with "[$HΨ $Hmodel $Hfn]") as (ws) "(-> & Hmodel & HΨ)"; first lia.
+    iSteps. rewrite Nat2Z.id !location_add_0. iSteps.
+  Qed.
+  Proof.
+    iIntros "%Φ ((%l & -> & #Hhdr & Hmodel) & Hfn) HΦ".
+    wp_rec. rewrite /array_data /array_size. wp_load.
+    rewrite !location_add_0.
+    wp_smart_apply (chunk_applyi_spec_disentangled Ψ with "[$Hmodel $Hfn]") as (ws) "(-> & Hmodel & HΨ)"; first lia.
+    iSteps. rewrite !location_add_0. iSteps.
+  Qed.
+  Proof.
+    iIntros "%Φ ((%l & -> & #Hhdr & Hmodel) & Hfn) HΦ".
+    wp_rec. rewrite /array_data /array_size. wp_load.
+    rewrite !location_add_0.
+    wp_smart_apply (chunk_applyi_spec_disentangled' Ψ with "[$Hmodel $Hfn]") as (ws) "(-> & Hmodel & HΨ)"; first lia.
+    iSteps. rewrite !location_add_0. iSteps.
+  Qed.
+
+#[global] Opaque array_apply.
+
+#[global] Opaque array_unsafe_initi.
+
+#[global] Opaque array_initi.
+
+#[global] Opaque array_unsafe_init.
+
+#[global] Opaque array_init.
+
+#[global] Opaque array_mapi.
+
+#[global] Opaque array_map.
+
+#[global] Opaque array_unsafe_copy_slice.
+
+#[global] Opaque array_copy_slice.
+
+#[global] Opaque array_unsafe_copy.
+
+#[global] Opaque array_copy.
+
+#[global] Opaque array_unsafe_grow.
+
+#[global] Opaque array_grow.
+
+#[global] Opaque array_unsafe_sub.
+
+#[global] Opaque array_sub.
+
+#[global] Opaque array_unsafe_shrink.
+
+#[global] Opaque array_shrink.
+
+#[global] Opaque array_clone.
+
+#[global] Opaque array_unsafe_cget.
+
+#[global] Opaque array_cget.
+
+#[global] Opaque array_unsafe_cset.
+
+#[global] Opaque array_cset.
+
+#[global] Opaque array_unsafe_ccopy_slice.
+
+#[global] Opaque array_ccopy_slice.
+
+#[global] Opaque array_unsafe_ccopy.
+
+#[global] Opaque array_ccopy.
 
   Lemma array_initi_spec Ψ sz fn :
     (0 ≤ sz)%Z →
@@ -1139,8 +2784,8 @@ Section zoo_G.
     wp_smart_apply (chunk_make_spec with "[//]") as "%l (Hmodel & _)".
     wp_pures.
     rewrite Z.add_1_l Z2Nat.inj_succ //.
-    iDestruct (chunk_model_cons with "Hmodel") as "(Hsz & Hmodel)".
-    iMod (pointsto_persist with "Hsz") as "#Hsz".
+    iDestruct (chunk_model_cons with "Hmodel") as "(Hhdr & Hmodel)".
+    iMod (pointsto_persist with "Hhdr") as "#Hhdr".
     pose Ψ' i (_ : list val) vs := (
       Ψ i vs
     )%I.
@@ -1350,1115 +2995,6 @@ Section zoo_G.
     iSteps.
   Qed.
 
-  Lemma array_size_spec_inv t sz :
-    {{{
-      array_inv t sz
-    }}}
-      array_size t
-    {{{
-      RET #sz; True
-    }}}.
-  Proof.
-    iSteps.
-  Qed.
-  Lemma array_size_spec_atomic_slice t :
-    <<<
-      True
-    | ∀∀ sz i dq vs,
-      array_slice t sz i dq vs
-    >>>
-      array_size t
-    <<<
-      array_slice t sz i dq vs
-    | RET #sz; £ 1
-    >>>.
-  Proof.
-    iIntros "!> %Φ _ HΦ".
-    iApply fupd_wp. iMod "HΦ" as "(%sz & %i & %dq & %vs & (%l & -> & Hslice) & HΦ & _)".
-    iMod ("HΦ" with "[Hslice]") as "HΦ"; first iSteps.
-    iModIntro. clear.
-    wp_rec. wp_pures credit:"H£".
-    iMod "HΦ" as "(%sz & %i & %dq & %vs & (%_l & %Heq & #Hsz & Hmodel) & _ & HΦ)". injection Heq as <-.
-    wp_load.
-    iApply ("HΦ" with "[Hmodel] H£").
-    iSteps.
-  Qed.
-  Lemma array_size_spec_atomic t :
-    <<<
-      True
-    | ∀∀ dq vs,
-      array_model t dq vs
-    >>>
-      array_size t
-    <<<
-      array_model t dq vs
-    | RET #(length vs); £ 1
-    >>>.
-  Proof.
-    iIntros "!> %Φ _ HΦ".
-    awp_apply (array_size_spec_atomic_slice with "[//]").
-    iApply (aacc_aupd with "HΦ"); first done. iIntros "%dq %vs Hmodel".
-    rewrite /atomic_acc /=. iModIntro. iExists (length vs), 0, dq, vs. iSplitL; iSmash+.
-  Qed.
-  Lemma array_size_spec_atomic_cslice t :
-    <<<
-      True
-    | ∀∀ sz i dq vs,
-      array_cslice t sz i dq vs
-    >>>
-      array_size t
-    <<<
-      array_cslice t sz i dq vs
-    | RET #sz; £ 1
-    >>>.
-  Proof.
-    iIntros "!> %Φ _ HΦ".
-    iApply fupd_wp. iMod "HΦ" as "(%sz & %i & %dq & %vs & (%l & -> & Hcslice) & HΦ & _)".
-    iMod ("HΦ" with "[Hcslice]") as "HΦ"; first iSteps.
-    iModIntro. clear.
-    wp_rec. wp_pures credit:"H£".
-    iMod "HΦ" as "(%sz & %i & %dq & %vs & (%_l & %Heq & #Hsz & Hcslice) & _ & HΦ)". injection Heq as <-.
-    wp_load.
-    iApply ("HΦ" with "[Hcslice] H£").
-    iSteps.
-  Qed.
-  Lemma array_size_spec_slice t sz i dq vs :
-    {{{
-      array_slice t sz i dq vs
-    }}}
-      array_size t
-    {{{
-      RET #sz;
-      array_slice t sz i dq vs
-    }}}.
-  Proof.
-    iSteps.
-  Qed.
-  Lemma array_size_spec t dq vs :
-    {{{
-      array_model t dq vs
-    }}}
-      array_size t
-    {{{
-      RET #(length vs);
-      array_model t dq vs
-    }}}.
-  Proof.
-    iSteps.
-  Qed.
-  Lemma array_size_spec_cslice t sz i dq vs :
-    {{{
-      array_cslice t sz i dq vs
-    }}}
-      array_size t
-    {{{
-      RET #sz;
-      array_cslice t sz i dq vs
-    }}}.
-  Proof.
-    iSteps.
-  Qed.
-
-  Lemma array_unsafe_get_spec_atomic_slice t (j : Z) :
-    <<<
-      True
-    | ∀∀ sz dq vs i v,
-      ⌜(i ≤ j)%Z ∧ vs !! (Z.to_nat j - i) = Some v⌝ ∗
-      array_slice t sz i dq vs
-    >>>
-      array_unsafe_get t #j
-    <<<
-      array_slice t sz i dq vs
-    | RET v; £ 1
-    >>>.
-  Proof.
-    iIntros "!> %Φ _ HΦ".
-    iApply fupd_wp. iMod "HΦ" as "(%sz & %dq & %vs & %i & %v & ((%Hi & %Hlookup) & (%l & -> & Hmodel)) & HΦ & _)".
-    iMod ("HΦ" with "[Hmodel]") as "HΦ"; first iSteps.
-    iModIntro. clear.
-    wp_rec. rewrite /array_data. wp_pures credit:"H£".
-    iMod "HΦ" as "(%sz & %dq & %vs & %i & %v & ((%Hi & %Hlookup) & (%_l & %Heq & #Hsz & Hmodel)) & _ & HΦ)". injection Heq as <-.
-    iApply (chunk_get_spec' with "Hmodel"); [lia | done | lia |]. iIntros "!> Hmodel".
-    iApply ("HΦ" with "[Hmodel] H£").
-    iSteps.
-  Qed.
-  Lemma array_unsafe_get_spec_atomic_cell t (i : Z) :
-    <<<
-      True
-    | ∀∀ sz i_ dq v,
-      ⌜i = Z.of_nat i_⌝ ∗
-      array_slice t sz i_ dq [v]
-    >>>
-      array_unsafe_get t #i
-    <<<
-      array_slice t sz (Z.to_nat i) dq [v]
-    | RET v; £ 1
-    >>>.
-  Proof.
-    iIntros "!> %Φ _ HΦ".
-    awp_apply (array_unsafe_get_spec_atomic_slice with "[//]").
-    iApply (aacc_aupd with "HΦ"); first done. iIntros "%sz %i_ %dq %v (-> & Hslice)".
-    rewrite Nat2Z.id.
-    rewrite /atomic_acc /=. iModIntro. iExists sz, dq, [v], i_, v. iSplitL.
-    { iFrame. rewrite Nat.sub_diag. iSteps. }
-    iSmash.
-  Qed.
-  Lemma array_unsafe_get_spec_atomic t (i : Z) :
-    (0 ≤ i)%Z →
-    <<<
-      True
-    | ∀∀ dq vs v,
-      ⌜vs !! Z.to_nat i = Some v⌝ ∗
-      array_model t dq vs
-    >>>
-      array_unsafe_get t #i
-    <<<
-      array_model t dq vs
-    | RET v; £ 1
-    >>>.
-  Proof.
-    iIntros "%Hi !> %Φ _ HΦ".
-    awp_apply (array_unsafe_get_spec_atomic_slice with "[//]").
-    iApply (aacc_aupd with "HΦ"); first done. iIntros "%dq %vs %v (%Hlookup & Hmodel)".
-    rewrite /atomic_acc /=. iModIntro. iExists (length vs), dq, vs, 0, v. iSplitL.
-    { iFrame. rewrite Nat.sub_0_r //. }
-    rewrite /array_model. iSmash.
-  Qed.
-  Lemma array_unsafe_get_spec_slice k t sz i dq vs (j : Z) v :
-    (i ≤ j)%Z →
-    vs !! k = Some v →
-    k = Z.to_nat j - i →
-    {{{
-      array_slice t sz i dq vs
-    }}}
-      array_unsafe_get t #j
-    {{{
-      RET v;
-      array_slice t sz i dq vs
-    }}}.
-  Proof.
-    iIntros (Hj Hlookup ->) "%Φ Hslice HΦ".
-    iApply wp_fupd.
-    awp_apply (array_unsafe_get_spec_atomic_slice with "[//]") without "HΦ".
-    rewrite /atomic_acc /=. iExists sz, dq, vs, i, v.
-    iApply fupd_mask_intro; first done. iIntros "Hclose".
-    iSplitL "Hslice"; first auto. iSplit; first iSteps.
-    iIntros "Hslice". iMod "Hclose" as "_". iIntros "!> H£ HΦ".
-    iMod (lc_fupd_elim_later with "H£ HΦ") as "HΦ".
-    iApply ("HΦ" with "Hslice").
-  Qed.
-  Lemma array_unsafe_get_spec_cell t sz (i : Z) i_ dq v :
-    i = Z.to_nat i_ →
-    {{{
-      array_slice t sz i_ dq [v]
-    }}}
-      array_unsafe_get t #i
-    {{{
-      RET v;
-      array_slice t sz i_ dq [v]
-    }}}.
-  Proof.
-    intros Hi.
-    eapply (array_unsafe_get_spec_slice 0); [lia | done | lia].
-  Qed.
-  Lemma array_unsafe_get_spec i_ t (i : Z) dq vs v :
-    (0 ≤ i)%Z →
-    vs !! i_ = Some v →
-    i_ = Z.to_nat i →
-    {{{
-      array_model t dq vs
-    }}}
-      array_unsafe_get t #i
-    {{{
-      RET v;
-      array_model t dq vs
-    }}}.
-  Proof.
-    intros Hi Hlookup ->.
-    eapply array_unsafe_get_spec_slice; [lia | done | lia].
-  Qed.
-
-  Lemma array_get_spec_atomic_slice t (j : Z) :
-    <<<
-      True
-    | ∀∀ sz dq vs i v,
-      ⌜(i ≤ j)%Z ∧ vs !! (Z.to_nat j - i) = Some v⌝ ∗
-      array_slice t sz i dq vs
-    >>>
-      array_get t #j
-    <<<
-      array_slice t sz i dq vs
-    | RET v; £ 1
-    >>>.
-  Proof.
-    iIntros "!> %Φ _ HΦ".
-    wp_rec.
-    wp_smart_apply assume_spec' as "_".
-    awp_smart_apply (array_size_spec_atomic_slice with "[//]").
-    iApply (aacc_aupd_abort with "HΦ"); first done. iIntros "%sz %dq %vs %i %v ((% & %) & Hslice)".
-    iAaccIntro with "Hslice"; first iSteps.
-    iIntros "Hslice !>". iSplitL; first auto. iIntros "HΦ !> _".
-    wp_smart_apply assume_spec' as "_".
-    wp_smart_apply (array_unsafe_get_spec_atomic_slice with "[//] HΦ").
-  Qed.
-  Lemma array_get_spec_atomic_cell t (i : Z) i_ :
-    i = Z.of_nat i_ →
-    <<<
-      True
-    | ∀∀ sz dq v,
-      array_slice t sz i_ dq [v]
-    >>>
-      array_get t #i
-    <<<
-      array_slice t sz i_ dq [v]
-    | RET v; £ 1
-    >>>.
-  Proof.
-    iIntros (->) "!> %Φ _ HΦ".
-    awp_apply (array_get_spec_atomic_slice with "[//]").
-    iApply (aacc_aupd with "HΦ"); first done. iIntros "%sz %dq %v Hslice".
-    rewrite Nat2Z.id.
-    rewrite /atomic_acc /=. iModIntro. iExists sz, dq, [v], i_, v. iSplitL.
-    { iFrame. rewrite Nat.sub_diag. iSteps. }
-    iSmash.
-  Qed.
-  Lemma array_get_spec_atomic t (i : Z) :
-    (0 ≤ i)%Z →
-    <<<
-      True
-    | ∀∀ dq vs v,
-      ⌜vs !! Z.to_nat i = Some v⌝ ∗
-      array_model t dq vs
-    >>>
-      array_get t #i
-    <<<
-      array_model t dq vs
-    | RET v; £ 1
-    >>>.
-  Proof.
-    iIntros "%Hi !> %Φ _ HΦ".
-    awp_apply (array_get_spec_atomic_slice with "[//]").
-    iApply (aacc_aupd with "HΦ"); first done. iIntros "%dq %vs %v (%Hlookup & Hmodel)".
-    rewrite /atomic_acc /=. iModIntro. iExists (length vs), dq, vs, 0, v. iSplitL.
-    { iFrame. rewrite Nat.sub_0_r //. }
-    rewrite /array_model. iSmash.
-  Qed.
-  Lemma array_get_spec_slice k t sz i dq vs (j : Z) v :
-    (i ≤ j)%Z →
-    vs !! k = Some v →
-    k = Z.to_nat j - i →
-    {{{
-      array_slice t sz i dq vs
-    }}}
-      array_get t #j
-    {{{
-      RET v;
-      array_slice t sz i dq vs
-    }}}.
-  Proof.
-    iIntros (Hi Hlookup ->) "%Φ Hslice HΦ".
-    wp_rec.
-    wp_smart_apply assume_spec' as "_".
-    wp_smart_apply (array_size_spec_slice with "Hslice") as "Hslice".
-    wp_smart_apply assume_spec' as "_".
-    wp_smart_apply (array_unsafe_get_spec_slice with "Hslice"); done.
-  Qed.
-  Lemma array_get_spec_cell t sz (i : Z) i_ dq v :
-    i = Z.of_nat i_ →
-    {{{
-      array_slice t sz i_ dq [v]
-    }}}
-      array_get t #i
-    {{{
-      RET v;
-      array_slice t sz i_ dq [v]
-    }}}.
-  Proof.
-    intros Hi.
-    eapply (array_get_spec_slice 0); [lia | done | lia].
-  Qed.
-  Lemma array_get_spec i_ t (i : Z) dq vs v :
-    (0 ≤ i)%Z →
-    vs !! i_ = Some v →
-    i_ = Z.to_nat i →
-    {{{
-      array_model t dq vs
-    }}}
-      array_get t #i
-    {{{
-      RET v;
-      array_model t dq vs
-    }}}.
-  Proof.
-    intros Hi Hlookup ->.
-    eapply array_get_spec_slice; [lia | done | lia].
-  Qed.
-
-  Lemma array_unsafe_set_spec_atomic_slice t (j : Z) v :
-    <<<
-      True
-    | ∀∀ sz vs i,
-      ⌜i ≤ j < i + length vs⌝%Z ∗
-      array_slice t sz i (DfracOwn 1) vs
-    >>>
-      array_unsafe_set t #j v
-    <<<
-      array_slice t sz i (DfracOwn 1) (<[Z.to_nat j - i := v]> vs)
-    | RET (); £ 1
-    >>>.
-  Proof.
-    iIntros "!> %Φ _ HΦ".
-    iApply fupd_wp. iMod "HΦ" as "(%sz & %vs & %i & (%Hj & (%l & -> & Hmodel)) & HΦ & _)".
-    iMod ("HΦ" with "[Hmodel]") as "HΦ"; first iSteps.
-    iModIntro. clear.
-    wp_rec. rewrite /array_data. wp_pures credit:"H£".
-    iMod "HΦ" as "(%sz & %vs & %i & (%Hj & (%_l & %Heq & #Hsz & Hmodel)) & _ & HΦ)". injection Heq as <-.
-    iApply (chunk_set_spec' with "Hmodel"); first lia. iIntros "!> Hmodel".
-    iApply ("HΦ" with "[Hmodel] [H£]"); last iSteps.
-    rewrite Nat2Z.id. iSteps.
-  Qed.
-  Lemma array_unsafe_set_spec_atomic_cell t (i : Z) v :
-    <<<
-      True
-    | ∀∀ sz i_ w,
-      ⌜i = Z.of_nat i_⌝ ∗
-      array_slice t sz i_ (DfracOwn 1) [w]
-    >>>
-      array_unsafe_set t #i v
-    <<<
-      array_slice t sz i_ (DfracOwn 1) [v]
-    | RET (); £ 1
-    >>>.
-  Proof.
-    iIntros "!> %Φ _ HΦ".
-    awp_apply (array_unsafe_set_spec_atomic_slice with "[//]").
-    iApply (aacc_aupd with "HΦ"); first done. iIntros "%sz %i_ %w (-> & Hslice)".
-    rewrite Nat2Z.id.
-    rewrite /atomic_acc /=. iModIntro. iExists sz, [w], i_. iSplitL.
-    { iFrame. iSteps. }
-    iSplit; first iSteps. iIntros "Hslisce !>". iRight.
-    rewrite Nat.sub_diag. auto with iFrame.
-  Qed.
-  Lemma array_unsafe_set_spec_atomic t (i : Z) v :
-    (0 ≤ i)%Z →
-    <<<
-      True
-    | ∀∀ vs,
-      ⌜i < length vs⌝%Z ∗
-      array_model t (DfracOwn 1) vs
-    >>>
-      array_unsafe_set t #i v
-    <<<
-      array_model t (DfracOwn 1) (<[Z.to_nat i := v]> vs)
-    | RET (); £ 1
-    >>>.
-  Proof.
-    iIntros "%Hi !> %Φ _ HΦ".
-    awp_apply (array_unsafe_set_spec_atomic_slice with "[//]").
-    iApply (aacc_aupd with "HΦ"); first done. iIntros "%vs (%Hlookup & Hmodel)".
-    rewrite /atomic_acc /=. iModIntro. iExists (length vs), vs, 0. iSplitL.
-    { iFrame. rewrite Z.add_0_l //. }
-    iSplit; first iSteps. iIntros "Hslisce !>". iRight.
-    rewrite Nat.sub_0_r /array_model insert_length. auto with iFrame.
-  Qed.
-  Lemma array_unsafe_set_spec_slice t sz i vs (j : Z) v :
-    (i ≤ j < i + length vs)%Z →
-    {{{
-      array_slice t sz i (DfracOwn 1) vs
-    }}}
-      array_unsafe_set t #j v
-    {{{
-      RET ();
-      array_slice t sz i (DfracOwn 1) (<[Z.to_nat j - i := v]> vs)
-    }}}.
-  Proof.
-    iIntros "%Hj %Φ Hslice HΦ".
-    iApply wp_fupd.
-    awp_apply (array_unsafe_set_spec_atomic_slice with "[//]") without "HΦ".
-    rewrite /atomic_acc /=. iExists sz, vs, i.
-    iApply fupd_mask_intro; first done. iIntros "Hclose".
-    iSplitL "Hslice"; first auto. iSplit; first iSteps.
-    iIntros "Hslice". iMod "Hclose" as "_". iIntros "!> H£ HΦ".
-    iMod (lc_fupd_elim_later with "H£ HΦ") as "HΦ".
-    iApply ("HΦ" with "Hslice").
-  Qed.
-  Lemma array_unsafe_set_spec_cell t sz (i : Z) i_ w v :
-    i = Z.of_nat i_ →
-    {{{
-      array_slice t sz i_ (DfracOwn 1) [w]
-    }}}
-      array_unsafe_set t #i v
-    {{{
-      RET ();
-      array_slice t sz i_ (DfracOwn 1) [v]
-    }}}.
-  Proof.
-    iIntros (->) "%Φ Hslice HΦ".
-    wp_apply (array_unsafe_set_spec_slice with "Hslice").
-    { simpl. lia. }
-    rewrite Nat2Z.id Nat.sub_diag. iSteps.
-  Qed.
-  Lemma array_unsafe_set_spec t (i : Z) vs v :
-    (0 ≤ i < length vs)%Z →
-    {{{
-      array_model t (DfracOwn 1) vs
-    }}}
-      array_unsafe_set t #i v
-    {{{
-      RET ();
-      array_model t (DfracOwn 1) (<[Z.to_nat i := v]> vs)
-    }}}.
-  Proof.
-    iIntros "%Hi %Φ Hmodel HΦ".
-    wp_apply (array_unsafe_set_spec_slice with "Hmodel"); first done.
-    rewrite Nat.sub_0_r /array_model insert_length //.
-  Qed.
-
-  Lemma array_set_spec_atomic_slice t (j : Z) v :
-    <<<
-      True
-    | ∀∀ sz vs i,
-      ⌜(i ≤ j < i + length vs)%Z⌝ ∗
-      array_slice t sz i (DfracOwn 1) vs
-    >>>
-      array_set t #j v
-    <<<
-      array_slice t sz i (DfracOwn 1) (<[Z.to_nat j - i := v]> vs)
-    | RET (); £ 1
-    >>>.
-  Proof.
-    iIntros "!> %Φ _ HΦ".
-    wp_rec.
-    wp_smart_apply assume_spec' as "_".
-    awp_smart_apply (array_size_spec_atomic_slice with "[//]").
-    iApply (aacc_aupd_abort with "HΦ"); first done. iIntros "%sz %vs %i (%Hj & Hslice)".
-    iAaccIntro with "Hslice"; first iSteps.
-    iIntros "Hslice !>". iSplitL; first auto. iIntros "HΦ !> _".
-    wp_smart_apply assume_spec' as "_".
-    wp_smart_apply (array_unsafe_set_spec_atomic_slice with "[//] HΦ").
-  Qed.
-  Lemma array_set_spec_atomic_cell t (i : Z) v :
-    <<<
-      True
-    | ∀∀ sz i_ w,
-      ⌜i = Z.of_nat i_⌝ ∗
-      array_slice t sz i_ (DfracOwn 1) [w]
-    >>>
-      array_set t #i v
-    <<<
-      array_slice t sz i_ (DfracOwn 1) [v]
-    | RET (); £ 1
-    >>>.
-  Proof.
-    iIntros "!> %Φ _ HΦ".
-    awp_apply (array_set_spec_atomic_slice with "[//]").
-    iApply (aacc_aupd with "HΦ"); first done. iIntros "%sz %i_ %w (-> & Hslice)".
-    rewrite Nat2Z.id.
-    rewrite /atomic_acc /=. iModIntro. iExists sz, [w], i_. iSplitL.
-    { iFrame. iSteps. }
-    iSplit; first iSteps. iIntros "Hslisce !>". iRight.
-    rewrite Nat.sub_diag. auto with iFrame.
-  Qed.
-  Lemma array_set_spec_atomic t (i : Z) v :
-    (0 ≤ i)%Z →
-    <<<
-      True
-    | ∀∀ vs,
-      ⌜(i < length vs)%Z⌝ ∗
-      array_model t (DfracOwn 1) vs
-    >>>
-      array_set t #i v
-    <<<
-      array_model t (DfracOwn 1) (<[Z.to_nat i := v]> vs)
-    | RET (); £ 1
-    >>>.
-  Proof.
-    iIntros "%Hi !> %Φ _ HΦ".
-    awp_apply (array_set_spec_atomic_slice with "[//]").
-    iApply (aacc_aupd with "HΦ"); first done. iIntros "%vs (%Hi'  & Hmodel)".
-    rewrite /atomic_acc /=. iModIntro. iExists (length vs), vs, 0. iSplitL.
-    { iFrame. rewrite Z.add_0_l //. }
-    iSplit; first iSteps. iIntros "Hslisce !>". iRight.
-    rewrite Nat.sub_0_r /array_model insert_length. auto with iFrame.
-  Qed.
-  Lemma array_set_spec_slice t sz i vs (j : Z) v :
-    (i ≤ j < i + length vs)%Z →
-    {{{
-      array_slice t sz i (DfracOwn 1) vs
-    }}}
-      array_set t #j v
-    {{{
-      RET ();
-      array_slice t sz i (DfracOwn 1) (<[Z.to_nat j - i := v]> vs)
-    }}}.
-  Proof.
-    iIntros "%Hj %Φ Hslice HΦ".
-    wp_rec.
-    wp_smart_apply assume_spec' as "_".
-    wp_smart_apply (array_size_spec_slice with "Hslice") as "Hslice".
-    wp_smart_apply assume_spec' as "_".
-    wp_smart_apply (array_unsafe_set_spec_slice with "Hslice"); done.
-  Qed.
-  Lemma array_set_spec_cell t sz (i : Z) i_ w v :
-    i = Z.of_nat i_ →
-    {{{
-      array_slice t sz i_ (DfracOwn 1) [w]
-    }}}
-      array_set t #i v
-    {{{
-      RET ();
-      array_slice t sz i_ (DfracOwn 1) [v]
-    }}}.
-  Proof.
-    iIntros (->) "%Φ Hslice HΦ".
-    wp_apply (array_set_spec_slice with "Hslice").
-    { simpl. lia. }
-    rewrite Nat2Z.id Nat.sub_diag. iSteps.
-  Qed.
-  Lemma array_set_spec t (i : Z) vs v :
-    (0 ≤ i < length vs)%Z →
-    {{{
-      array_model t (DfracOwn 1) vs
-    }}}
-      array_set t #i v
-    {{{
-      RET ();
-      array_model t (DfracOwn 1) (<[Z.to_nat i := v]> vs)
-    }}}.
-  Proof.
-    iIntros "%Hi %Φ Hmodel HΦ".
-    wp_apply (array_set_spec_slice with "Hmodel"); first done.
-    rewrite Nat.sub_0_r /array_model insert_length //.
-  Qed.
-
-  Lemma array_foldli_spec Ψ t dq vs acc fn :
-    {{{
-      ▷ Ψ 0 [] acc ∗
-      array_model t dq vs ∗
-      □ (
-        ∀ i v acc,
-        ⌜vs !! i = Some v⌝ -∗
-        Ψ i (take i vs) acc -∗
-        WP fn acc #i v {{ acc,
-          ▷ Ψ (S i) (take i vs ++ [v]) acc
-        }}
-      )
-    }}}
-      array_foldli t acc fn
-    {{{ acc,
-      RET acc;
-      array_model t dq vs ∗
-      Ψ (length vs) vs acc
-    }}}.
-  Proof.
-    iIntros "%Φ (HΨ & (%l & -> & #Hsz & Hmodel) & Hfn) HΦ".
-    wp_rec. rewrite /array_data /array_size. wp_load.
-    rewrite !location_add_0.
-    wp_smart_apply (chunk_foldli_spec Ψ with "[$HΨ $Hmodel $Hfn]"); first lia.
-    iSteps. rewrite Nat2Z.id !location_add_0. iSteps.
-  Qed.
-  Lemma array_foldli_spec' Ψ t dq vs acc fn :
-    {{{
-      ▷ Ψ 0 [] acc ∗
-      array_model t dq vs ∗
-      ( [∗ list] i ↦ v ∈ vs,
-        ∀ acc,
-        Ψ i (take i vs) acc -∗
-        WP fn acc #i v {{ acc,
-          ▷ Ψ (S i) (take i vs ++ [v]) acc
-        }}
-      )
-    }}}
-      array_foldli t acc fn
-    {{{ acc,
-      RET acc;
-      array_model t dq vs ∗
-      Ψ (length vs) vs acc
-    }}}.
-  Proof.
-    iIntros "%Φ (HΨ & (%l & -> & #Hsz & Hmodel) & Hfn) HΦ".
-    wp_rec. rewrite /array_data /array_size. wp_load.
-    rewrite !location_add_0.
-    wp_smart_apply (chunk_foldli_spec' Ψ with "[$HΨ $Hmodel $Hfn]"); first lia.
-    iSteps. rewrite Nat2Z.id !location_add_0. iSteps.
-  Qed.
-
-  Lemma array_foldl_spec Ψ t dq vs acc fn :
-    {{{
-      ▷ Ψ 0 [] acc ∗
-      array_model t dq vs ∗
-      □ (
-        ∀ i v acc,
-        ⌜vs !! i = Some v⌝ -∗
-        Ψ i (take i vs) acc -∗
-        WP fn acc v {{ acc,
-          ▷ Ψ (S i) (take i vs ++ [v]) acc
-        }}
-      )
-    }}}
-      array_foldl t acc fn
-    {{{ acc,
-      RET acc;
-      array_model t dq vs ∗
-      Ψ (length vs) vs acc
-    }}}.
-  Proof.
-    iIntros "%Φ (HΨ & (%l & -> & #Hsz & Hmodel) & Hfn) HΦ".
-    wp_rec. rewrite /array_data /array_size. wp_load.
-    rewrite !location_add_0.
-    wp_smart_apply (chunk_foldl_spec Ψ with "[$HΨ $Hmodel $Hfn]"); first lia.
-    iSteps. rewrite Nat2Z.id !location_add_0. iSteps.
-  Qed.
-  Lemma array_foldl_spec' Ψ t dq vs acc fn :
-    {{{
-      ▷ Ψ 0 [] acc ∗
-      array_model t dq vs ∗
-      ( [∗ list] i ↦ v ∈ vs,
-        ∀ acc,
-        Ψ i (take i vs) acc -∗
-        WP fn acc v {{ acc,
-          ▷ Ψ (S i) (take i vs ++ [v]) acc
-        }}
-      )
-    }}}
-      array_foldl t acc fn
-    {{{ acc,
-      RET acc;
-      array_model t dq vs ∗
-      Ψ (length vs) vs acc
-    }}}.
-  Proof.
-    iIntros "%Φ (HΨ & (%l & -> & #Hsz & Hmodel) & Hfn) HΦ".
-    wp_rec. rewrite /array_data /array_size. wp_load.
-    rewrite !location_add_0.
-    wp_smart_apply (chunk_foldl_spec' Ψ with "[$HΨ $Hmodel $Hfn]"); first lia.
-    iSteps. rewrite Nat2Z.id !location_add_0. iSteps.
-  Qed.
-
-  Lemma array_foldri_spec Ψ t dq vs fn acc :
-    {{{
-      array_model t dq vs ∗
-      ▷ Ψ (length vs) acc [] ∗
-      □ (
-        ∀ i v acc,
-        ⌜vs !! i = Some v⌝ -∗
-        Ψ (S i) acc (drop (S i) vs) -∗
-        WP fn #i v acc {{ acc,
-          ▷ Ψ i acc (v :: drop (S i) vs)
-        }}
-      )
-    }}}
-      array_foldri t fn acc
-    {{{ acc,
-      RET acc;
-      Ψ 0 acc vs ∗
-      array_model t dq vs
-    }}}.
-  Proof.
-    iIntros "%Φ ((%l & -> & #Hsz & Hmodel) & HΨ & Hfn) HΦ".
-    wp_rec. rewrite /array_data /array_size. wp_load.
-    rewrite !location_add_0.
-    wp_smart_apply (chunk_foldri_spec Ψ with "[$Hmodel HΨ $Hfn]"); first lia.
-    { rewrite Nat2Z.id. iSteps. }
-    iSteps. rewrite !location_add_0. iSteps.
-  Qed.
-  Lemma array_foldri_spec' Ψ t dq vs fn acc :
-    {{{
-      array_model t dq vs ∗
-      ▷ Ψ (length vs) acc [] ∗
-      ( [∗ list] i ↦ v ∈ vs,
-        ∀ acc,
-        Ψ (S i) acc (drop (S i) vs) -∗
-        WP fn #i v acc {{ acc,
-          ▷ Ψ i acc (v :: drop (S i) vs)
-        }}
-      )
-    }}}
-      array_foldri t fn acc
-    {{{ acc,
-      RET acc;
-      Ψ 0 acc vs ∗
-      array_model t dq vs
-    }}}.
-  Proof.
-    iIntros "%Φ ((%l & -> & #Hsz & Hmodel) & HΨ & Hfn) HΦ".
-    wp_rec. rewrite /array_data /array_size. wp_load.
-    rewrite !location_add_0.
-    wp_smart_apply (chunk_foldri_spec' Ψ with "[$Hmodel HΨ $Hfn]"); first lia.
-    { rewrite Nat2Z.id. iSteps. }
-    iSteps. rewrite !location_add_0. iSteps.
-  Qed.
-
-  Lemma array_foldr_spec Ψ t dq vs fn acc :
-    {{{
-      array_model t dq vs ∗
-      ▷ Ψ (length vs) acc [] ∗
-      □ (
-        ∀ i v acc,
-        ⌜vs !! i = Some v⌝ -∗
-        Ψ (S i) acc (drop (S i) vs) -∗
-        WP fn v acc {{ acc,
-          ▷ Ψ i acc (v :: drop (S i) vs)
-        }}
-      )
-    }}}
-      array_foldr t fn acc
-    {{{ acc,
-      RET acc;
-      Ψ 0 acc vs ∗
-      array_model t dq vs
-    }}}.
-  Proof.
-    iIntros "%Φ ((%l & -> & #Hsz & Hmodel) & HΨ & Hfn) HΦ".
-    wp_rec. rewrite /array_data /array_size. wp_load.
-    rewrite !location_add_0.
-    wp_smart_apply (chunk_foldr_spec Ψ with "[$Hmodel HΨ $Hfn]"); first lia.
-    { rewrite Nat2Z.id. iSteps. }
-    iSteps. rewrite !location_add_0. iSteps.
-  Qed.
-  Lemma array_foldr_spec' Ψ t dq vs fn acc :
-    {{{
-      array_model t dq vs ∗
-      ▷ Ψ (length vs) acc [] ∗
-      ( [∗ list] i ↦ v ∈ vs,
-        ∀ acc,
-        Ψ (S i) acc (drop (S i) vs) -∗
-        WP fn v acc {{ acc,
-          ▷ Ψ i acc (v :: drop (S i) vs)
-        }}
-      )
-    }}}
-      array_foldr t fn acc
-    {{{ acc,
-      RET acc;
-      Ψ 0 acc vs ∗
-      array_model t dq vs
-    }}}.
-  Proof.
-    iIntros "%Φ ((%l & -> & #Hsz & Hmodel) & HΨ & Hfn) HΦ".
-    wp_rec. rewrite /array_data /array_size. wp_load.
-    rewrite !location_add_0.
-    wp_smart_apply (chunk_foldr_spec' Ψ with "[$Hmodel HΨ $Hfn]"); first lia.
-    { rewrite Nat2Z.id. iSteps. }
-    iSteps. rewrite !location_add_0. iSteps.
-  Qed.
-
-  Lemma array_iteri_spec Ψ t dq vs fn :
-    {{{
-      ▷ Ψ 0 [] ∗
-      array_model t dq vs ∗
-      □ (
-        ∀ i v,
-        ⌜vs !! i = Some v⌝ -∗
-        Ψ i (take i vs) -∗
-        WP fn #i v {{ res,
-          ⌜res = ()%V⌝ ∗
-          ▷ Ψ (S i) (take i vs ++ [v])
-        }}
-      )
-    }}}
-      array_iteri t fn
-    {{{
-      RET ();
-      array_model t dq vs ∗
-      Ψ (length vs) vs
-    }}}.
-  Proof.
-    iIntros "%Φ (HΨ & (%l & -> & #Hsz & Hmodel) & Hfn) HΦ".
-    wp_rec. rewrite /array_data /array_size. wp_load.
-    rewrite !location_add_0.
-    wp_smart_apply (chunk_iteri_spec Ψ with "[$HΨ $Hmodel $Hfn]"); first lia.
-    iSteps. rewrite Nat2Z.id !location_add_0. iSteps.
-  Qed.
-  Lemma array_iteri_spec' Ψ t dq vs fn :
-    {{{
-      ▷ Ψ 0 [] ∗
-      array_model t dq vs ∗
-      ( [∗ list] i ↦ v ∈ vs,
-        Ψ i (take i vs) -∗
-        WP fn #i v {{ res,
-          ⌜res = ()%V⌝ ∗
-          ▷ Ψ (S i) (take i vs ++ [v])
-        }}
-      )
-    }}}
-      array_iteri t fn
-    {{{
-      RET ();
-      array_model t dq vs ∗
-      Ψ (length vs) vs
-    }}}.
-  Proof.
-    iIntros "%Φ (HΨ & (%l & -> & #Hsz & Hmodel) & Hfn) HΦ".
-    wp_rec. rewrite /array_data /array_size. wp_load.
-    rewrite !location_add_0.
-    wp_smart_apply (chunk_iteri_spec' Ψ with "[$HΨ $Hmodel $Hfn]"); first lia.
-    iSteps. rewrite Nat2Z.id !location_add_0. iSteps.
-  Qed.
-  Lemma array_iteri_spec_disentangled Ψ t dq vs fn :
-    {{{
-      array_model t dq vs ∗
-      □ (
-        ∀ i v,
-        ⌜vs !! i = Some v⌝ -∗
-        WP fn #i v {{ res,
-          ⌜res = ()%V⌝ ∗
-          ▷ Ψ i v
-        }}
-      )
-    }}}
-      array_iteri t fn
-    {{{
-      RET ();
-      array_model t dq vs ∗
-      ( [∗ list] i ↦ v ∈ vs,
-        Ψ i v
-      )
-    }}}.
-  Proof.
-    iIntros "%Φ ((%l & -> & #Hsz & Hmodel) & Hfn) HΦ".
-    wp_rec. rewrite /array_data /array_size. wp_load.
-    rewrite !location_add_0.
-    wp_smart_apply (chunk_iteri_spec_disentangled Ψ with "[$Hmodel $Hfn]"); first lia.
-    iSteps. rewrite !location_add_0. iSteps.
-  Qed.
-  Lemma array_iteri_spec_disentangled' Ψ t dq vs fn :
-    {{{
-      array_model t dq vs ∗
-      ( [∗ list] i ↦ v ∈ vs,
-        WP fn #i v {{ res,
-          ⌜res = ()%V⌝ ∗
-          ▷ Ψ i v
-        }}
-      )
-    }}}
-      array_iteri t fn
-    {{{
-      RET ();
-      array_model t dq vs ∗
-      ( [∗ list] i ↦ v ∈ vs,
-        Ψ i v
-      )
-    }}}.
-  Proof.
-    iIntros "%Φ ((%l & -> & #Hsz & Hmodel) & Hfn) HΦ".
-    wp_rec. rewrite /array_data /array_size. wp_load.
-    rewrite !location_add_0.
-    wp_smart_apply (chunk_iteri_spec_disentangled' Ψ with "[$Hmodel $Hfn]"); first lia.
-    iSteps. rewrite !location_add_0. iSteps.
-  Qed.
-
-  Lemma array_iter_spec Ψ t dq vs fn :
-    {{{
-      ▷ Ψ 0 [] ∗
-      array_model t dq vs ∗
-      □ (
-        ∀ i v,
-        ⌜vs !! i = Some v⌝ -∗
-        Ψ i (take i vs) -∗
-        WP fn v {{ res,
-          ⌜res = ()%V⌝ ∗
-          ▷ Ψ (S i) (take i vs ++ [v])
-        }}
-      )
-    }}}
-      array_iter t fn
-    {{{
-      RET ();
-      array_model t dq vs ∗
-      Ψ (length vs) vs
-    }}}.
-  Proof.
-    iIntros "%Φ (HΨ & (%l & -> & #Hsz & Hmodel) & Hfn) HΦ".
-    wp_rec. rewrite /array_data /array_size. wp_load.
-    rewrite !location_add_0.
-    wp_smart_apply (chunk_iter_spec Ψ with "[$HΨ $Hmodel $Hfn]"); first lia.
-    iSteps. rewrite Nat2Z.id !location_add_0. iSteps.
-  Qed.
-  Lemma array_iter_spec' Ψ t dq vs fn :
-    {{{
-      ▷ Ψ 0 [] ∗
-      array_model t dq vs ∗
-      ( [∗ list] i ↦ v ∈ vs,
-        Ψ i (take i vs) -∗
-        WP fn v {{ res,
-          ⌜res = ()%V⌝ ∗
-          ▷ Ψ (S i) (take i vs ++ [v])
-        }}
-      )
-    }}}
-      array_iter t fn
-    {{{
-      RET ();
-      array_model t dq vs ∗
-      Ψ (length vs) vs
-    }}}.
-  Proof.
-    iIntros "%Φ (HΨ & (%l & -> & #Hsz & Hmodel) & Hfn) HΦ".
-    wp_rec. rewrite /array_data /array_size. wp_load.
-    rewrite !location_add_0.
-    wp_smart_apply (chunk_iter_spec' Ψ with "[$HΨ $Hmodel $Hfn]"); first lia.
-    iSteps. rewrite Nat2Z.id !location_add_0. iSteps.
-  Qed.
-  Lemma array_iter_spec_disentangled Ψ t dq vs fn :
-    {{{
-      array_model t dq vs ∗
-      □ (
-        ∀ i v,
-        ⌜vs !! i = Some v⌝ -∗
-        WP fn v {{ res,
-          ⌜res = ()%V⌝ ∗
-          ▷ Ψ i v
-        }}
-      )
-    }}}
-      array_iter t fn
-    {{{
-      RET ();
-      array_model t dq vs ∗
-      ( [∗ list] i ↦ v ∈ vs,
-        Ψ i v
-      )
-    }}}.
-  Proof.
-    iIntros "%Φ ((%l & -> & #Hsz & Hmodel) & Hfn) HΦ".
-    wp_rec. rewrite /array_data /array_size. wp_load.
-    rewrite !location_add_0.
-    wp_smart_apply (chunk_iter_spec_disentangled Ψ with "[$Hmodel $Hfn]"); first lia.
-    iSteps. rewrite !location_add_0. iSteps.
-  Qed.
-  Lemma array_iter_spec_disentangled' Ψ t dq vs fn :
-    {{{
-      array_model t dq vs ∗
-      ( [∗ list] i ↦ v ∈ vs,
-        WP fn v {{ res,
-          ⌜res = ()%V⌝ ∗
-          ▷ Ψ i v
-        }}
-      )
-    }}}
-      array_iter t fn
-    {{{
-      RET ();
-      array_model t dq vs ∗
-      ( [∗ list] i ↦ v ∈ vs,
-        Ψ i v
-      )
-    }}}.
-  Proof.
-    iIntros "%Φ ((%l & -> & #Hsz & Hmodel) & Hfn) HΦ".
-    wp_rec. rewrite /array_data /array_size. wp_load.
-    rewrite !location_add_0.
-    wp_smart_apply (chunk_iter_spec_disentangled' Ψ with "[$Hmodel $Hfn]"); first lia.
-    iSteps. rewrite !location_add_0. iSteps.
-  Qed.
-
-  Lemma array_applyi_spec Ψ t vs fn :
-    {{{
-      ▷ Ψ 0 [] [] ∗
-      array_model t (DfracOwn 1) vs ∗
-      □ (
-        ∀ i v ws,
-        ⌜i = length ws ∧ vs !! i = Some v⌝ -∗
-        Ψ i (take i vs) ws -∗
-        WP fn #i v {{ w,
-          ▷ Ψ (S i) (take i vs ++ [v]) (ws ++ [w])
-        }}
-      )
-    }}}
-      array_applyi t fn
-    {{{ ws,
-      RET ();
-      ⌜length vs = length ws⌝ ∗
-      array_model t (DfracOwn 1) ws ∗
-      Ψ (length vs) vs ws
-    }}}.
-  Proof.
-    iIntros "%Φ (HΨ & (%l & -> & #Hsz & Hmodel) & Hfn) HΦ".
-    wp_rec. rewrite /array_data /array_size. wp_load.
-    rewrite !location_add_0.
-    wp_smart_apply (chunk_applyi_spec Ψ with "[$HΨ $Hmodel $Hfn]") as (ws) "(-> & Hmodel & HΨ)"; first lia.
-    iSteps. rewrite Nat2Z.id !location_add_0. iSteps.
-  Qed.
-  Lemma array_applyi_spec' Ψ t vs fn :
-    {{{
-      ▷ Ψ 0 [] [] ∗
-      array_model t (DfracOwn 1) vs ∗
-      ( [∗ list] i ↦ v ∈ vs,
-        ∀ ws,
-        ⌜i = length ws⌝ -∗
-        Ψ i (take i vs) ws -∗
-        WP fn #i v {{ w,
-          ▷ Ψ (S i) (take i vs ++ [v]) (ws ++ [w])
-        }}
-      )
-    }}}
-      array_applyi t fn
-    {{{ ws,
-      RET ();
-      ⌜length vs = length ws⌝ ∗
-      array_model t (DfracOwn 1) ws ∗
-      Ψ (length vs) vs ws
-    }}}.
-  Proof.
-    iIntros "%Φ (HΨ & (%l & -> & #Hsz & Hmodel) & Hfn) HΦ".
-    wp_rec. rewrite /array_data /array_size. wp_load.
-    rewrite !location_add_0.
-    wp_smart_apply (chunk_applyi_spec' Ψ with "[$HΨ $Hmodel $Hfn]") as (ws) "(-> & Hmodel & HΨ)"; first lia.
-    iSteps. rewrite Nat2Z.id !location_add_0. iSteps.
-  Qed.
-  Lemma array_applyi_spec_disentangled Ψ t vs fn :
-    {{{
-      array_model t (DfracOwn 1) vs ∗
-      □ (
-        ∀ i v,
-        ⌜vs !! i = Some v⌝ -∗
-        WP fn #i v {{ w,
-          ▷ Ψ i w
-        }}
-      )
-    }}}
-      array_applyi t fn
-    {{{ ws,
-      RET ();
-      ⌜length vs = length ws⌝ ∗
-      array_model t (DfracOwn 1) ws ∗
-      ( [∗ list] i ↦ w ∈ ws,
-        Ψ i w
-      )
-    }}}.
-  Proof.
-    iIntros "%Φ ((%l & -> & #Hsz & Hmodel) & Hfn) HΦ".
-    wp_rec. rewrite /array_data /array_size. wp_load.
-    rewrite !location_add_0.
-    wp_smart_apply (chunk_applyi_spec_disentangled Ψ with "[$Hmodel $Hfn]") as (ws) "(-> & Hmodel & HΨ)"; first lia.
-    iSteps. rewrite !location_add_0. iSteps.
-  Qed.
-  Lemma array_applyi_spec_disentangled' Ψ t vs fn :
-    {{{
-      array_model t (DfracOwn 1) vs ∗
-      ( [∗ list] i ↦ v ∈ vs,
-        WP fn #i v {{ w,
-          ▷ Ψ i w
-        }}
-      )
-    }}}
-      array_applyi t fn
-    {{{ ws,
-      RET ();
-      array_model t (DfracOwn 1) ws ∗
-      ( [∗ list] i ↦ w ∈ ws,
-        Ψ i w
-      )
-    }}}.
-  Proof.
-    iIntros "%Φ ((%l & -> & #Hsz & Hmodel) & Hfn) HΦ".
-    wp_rec. rewrite /array_data /array_size. wp_load.
-    rewrite !location_add_0.
-    wp_smart_apply (chunk_applyi_spec_disentangled' Ψ with "[$Hmodel $Hfn]") as (ws) "(-> & Hmodel & HΨ)"; first lia.
-    iSteps. rewrite !location_add_0. iSteps.
-  Qed.
-
   Lemma array_apply_spec Ψ t vs fn :
     {{{
       ▷ Ψ 0 [] [] ∗
@@ -2480,7 +3016,7 @@ Section zoo_G.
       Ψ (length vs) vs ws
     }}}.
   Proof.
-    iIntros "%Φ (HΨ & (%l & -> & #Hsz & Hmodel) & Hfn) HΦ".
+    iIntros "%Φ (HΨ & (%l & -> & #Hhdr & Hmodel) & Hfn) HΦ".
     wp_rec. rewrite /array_data /array_size. wp_load.
     rewrite !location_add_0.
     wp_smart_apply (chunk_apply_spec Ψ with "[$HΨ $Hmodel $Hfn]") as (ws) "(-> & Hmodel & HΨ)"; first lia.
@@ -2507,7 +3043,7 @@ Section zoo_G.
       Ψ (length vs) vs ws
     }}}.
   Proof.
-    iIntros "%Φ (HΨ & (%l & -> & #Hsz & Hmodel) & Hfn) HΦ".
+    iIntros "%Φ (HΨ & (%l & -> & #Hhdr & Hmodel) & Hfn) HΦ".
     wp_rec. rewrite /array_data /array_size. wp_load.
     rewrite !location_add_0.
     wp_smart_apply (chunk_apply_spec' Ψ with "[$HΨ $Hmodel $Hfn]") as (ws) "(-> & Hmodel & HΨ)"; first lia.
@@ -2534,7 +3070,7 @@ Section zoo_G.
       )
     }}}.
   Proof.
-    iIntros "%Φ ((%l & -> & #Hsz & Hmodel) & Hfn) HΦ".
+    iIntros "%Φ ((%l & -> & #Hhdr & Hmodel) & Hfn) HΦ".
     wp_rec. rewrite /array_data /array_size. wp_load.
     rewrite !location_add_0.
     wp_smart_apply (chunk_apply_spec_disentangled Ψ with "[$Hmodel $Hfn]") as (ws) "(-> & Hmodel & HΨ)"; first lia.
@@ -2558,7 +3094,7 @@ Section zoo_G.
       )
     }}}.
   Proof.
-    iIntros "%Φ ((%l & -> & #Hsz & Hmodel) & Hfn) HΦ".
+    iIntros "%Φ ((%l & -> & #Hhdr & Hmodel) & Hfn) HΦ".
     wp_rec. rewrite /array_data /array_size. wp_load.
     rewrite !location_add_0.
     wp_smart_apply (chunk_apply_spec_disentangled' Ψ with "[$Hmodel $Hfn]") as (ws) "(-> & Hmodel & HΨ)"; first lia.
@@ -2586,8 +3122,8 @@ Section zoo_G.
     wp_smart_apply (array_size_spec_slice with "Hslice1") as "Hslice1".
     wp_smart_apply (array_size_spec_slice with "Hslice2") as "Hslice2".
     repeat (wp_smart_apply assume_spec' as "_").
-    iDestruct "Hslice1" as "(%l1 & -> & #Hsz1 & Hmodel1)".
-    iDestruct "Hslice2" as "(%l2 & -> & #Hsz2 & Hmodel2)".
+    iDestruct "Hslice1" as "(%l1 & -> & #Hhdr1 & Hmodel1)".
+    iDestruct "Hslice2" as "(%l2 & -> & #Hhdr2 & Hmodel2)".
     wp_smart_apply (chunk_copy_spec with "[$Hmodel1 $Hmodel2]"); [lia.. |].
     iSteps.
   Qed.
@@ -2769,10 +3305,10 @@ Section zoo_G.
       array_model t' (DfracOwn 1) (take (Z.to_nat n) vs)
     }}}.
   Proof.
-    iIntros (-> ->) "%Φ (%l & -> & #Hsz & Hmodel) HΦ".
+    iIntros (-> ->) "%Φ (%l & -> & #Hhdr & Hmodel) HΦ".
     wp_rec. rewrite /array_size /array_data. wp_load.
     repeat (wp_smart_apply assume_spec' as "_").
-    wp_smart_apply (array_make_spec with "[//]") as "%t' (%l' & -> & #Hsz' & Hmodel')"; first lia.
+    wp_smart_apply (array_make_spec with "[//]") as "%t' (%l' & -> & #Hhdr' & Hmodel')"; first lia.
     iEval (rewrite location_add_0) in "Hmodel'".
     wp_smart_apply (chunk_copy_spec with "[$Hmodel $Hmodel']") as "(Hmodel & Hmodel')"; first lia.
     { rewrite replicate_length //. }
@@ -2863,44 +3399,6 @@ Section zoo_G.
     iApply ("HΦ" with "[$Hmodel $Hmodel']").
   Qed.
 
-  Lemma array_fill_slice_spec t sz vs i (i_ n : Z) v :
-    i_ = Z.of_nat i →
-    n = length vs →
-    {{{
-      array_slice t sz i (DfracOwn 1) vs
-    }}}
-      array_fill_slice t #i_ #n v
-    {{{
-      RET ();
-      array_slice t sz i (DfracOwn 1) (replicate (Z.to_nat n) v)
-    }}}.
-  Proof.
-    iIntros (-> ->) "%Φ (%l & -> & #Hsz & Hmodel) HΦ".
-    wp_rec. rewrite /array_size /array_data.
-    wp_load.
-    repeat (wp_smart_apply assume_spec' as "_").
-    wp_smart_apply (chunk_fill_spec with "Hmodel"); first lia.
-    iSteps.
-  Qed.
-
-  Lemma array_fill_spec t vs v :
-    {{{
-      array_model t (DfracOwn 1) vs
-    }}}
-      array_fill t v
-    {{{
-      RET ();
-      array_model t (DfracOwn 1) (replicate (length vs) v)
-    }}}.
-  Proof.
-    iIntros "%Φ Hmodel HΦ".
-    wp_rec.
-    wp_smart_apply (array_size_spec with "Hmodel") as "Hmodel".
-    wp_apply (array_fill_slice_spec with "Hmodel") as "model"; [lia | done |].
-    iApply "HΦ".
-    rewrite Nat2Z.id -{1}(replicate_length (length vs) v) //.
-  Qed.
-
   Lemma array_cget_spec_atomic t (i : Z) :
     <<<
       True
@@ -2911,16 +3409,17 @@ Section zoo_G.
       array_cget t #i
     <<<
       array_cslice t sz i_ dq [v]
-    | RET v; £ 1
+    | RET v;
+      £ 1
     >>>.
   Proof.
     iIntros "!> %Φ _ HΦ".
     wp_rec.
     awp_smart_apply (array_size_spec_atomic_cslice with "[//]").
     iApply (aacc_aupd_abort with "HΦ"); first done. iIntros "%sz %i_ %dq %v (-> & Hcslice)".
-    iAaccIntro with "Hcslice"; first iSteps. iSteps as (l) "Hsz HΦ H£". clear.
+    iAaccIntro with "Hcslice"; first iSteps. iSteps as (l) "Hhdr HΦ H£". clear.
     awp_apply (chunk_cget_spec_atomic with "[//]").
-    iApply (aacc_aupd_commit with "HΦ"); first done. iSteps as (i l dq v) "Hsz Hcslice".
+    iApply (aacc_aupd_commit with "HΦ"); first done. iSteps as (i l dq v) "Hhdr Hcslice".
     rewrite /atomic_acc /=. iSteps.
   Qed.
   Lemma array_cget_spec t sz (i : Z) i_ dq v :
@@ -2955,16 +3454,17 @@ Section zoo_G.
       array_cset t #i v
     <<<
       array_cslice t sz i_ (DfracOwn 1) [v]
-    | RET (); £ 1
+    | RET ();
+      £ 1
     >>>.
   Proof.
     iIntros "!> %Φ _ HΦ".
     wp_rec.
     awp_smart_apply (array_size_spec_atomic_cslice with "[//]").
     iApply (aacc_aupd_abort with "HΦ"); first done. iIntros "%sz %i_ %w (-> & Hcslice)".
-    iAaccIntro with "Hcslice"; first iSteps. iSteps as (l) "Hsz HΦ H£". clear.
+    iAaccIntro with "Hcslice"; first iSteps. iSteps as (l) "Hhdr HΦ H£". clear.
     awp_apply (chunk_cset_spec_atomic with "[//]").
-    iApply (aacc_aupd_commit with "HΦ"); first done. iSteps as (i l w) "Hsz Hcslice".
+    iApply (aacc_aupd_commit with "HΦ"); first done. iSteps as (i l w) "Hhdr Hcslice".
     rewrite /atomic_acc /=. iSteps.
   Qed.
   Lemma array_cset_spec t sz (i : Z) i_ w v :
@@ -3005,7 +3505,7 @@ Section zoo_G.
       array_cslice t2 sz2 i2_ (DfracOwn 1) (take n_ vs1 ++ drop n_ vs2)
     }}}.
   Proof.
-    iIntros (n_ -> -> Hn) "%Φ ((%l1 & -> & #Hsz1 & Hcslice1) & (%l2 & -> & #Hsz2 & Hcslice2)) HΦ".
+    iIntros (n_ -> -> Hn) "%Φ ((%l1 & -> & #Hhdr1 & Hcslice1) & (%l2 & -> & #Hhdr2 & Hcslice2)) HΦ".
     wp_rec. rewrite /array_size /array_data. do 2 wp_load.
     wp_smart_apply (chunk_cblit_spec with "[$Hcslice1 $Hcslice2]"); [done.. |].
     iSteps.
@@ -3057,8 +3557,8 @@ Section zoo_G.
     wp_rec.
     iApply wp_fupd.
     wp_apply (chunk_make_spec with "[//]") as "%l (Hl & _)".
-    iDestruct (chunk_model_cons_2 with "Hl") as "(Hsz & _)".
-    rewrite -{1}(location_add_0 l). iMod (pointsto_persist with "Hsz") as "#Hsz".
+    iDestruct (chunk_model_cons_2 with "Hl") as "(Hhdr & _)".
+    rewrite -{1}(location_add_0 l). iMod (pointsto_persist with "Hhdr") as "#Hhdr".
     iApply "HΦ". iExists l. repeat iSplitR; [iSteps.. |].
     iApply itype_chunk_0.
   Qed.
@@ -3080,10 +3580,10 @@ Section zoo_G.
     Z_to_nat sz. rewrite Nat2Z.id.
     wp_smart_apply (chunk_make_spec with "[//]") as "%l (Hl & _)".
     rewrite Z.add_1_l Z2Nat.inj_succ; first lia. rewrite Nat2Z.id.
-    iDestruct (chunk_model_cons_2 with "Hl") as "(Hsz & Hdata)".
+    iDestruct (chunk_model_cons_2 with "Hl") as "(Hhdr & Hdata)".
     rewrite -{1}(location_add_0 l).
     wp_store. wp_pures.
-    iMod (pointsto_persist with "Hsz") as "#Hsz".
+    iMod (pointsto_persist with "Hhdr") as "#Hhdr".
     iApply "HΦ". iStep. iExists l. repeat iSplitR; [iSteps.. |].
     iApply inv_alloc. iExists _. iFrame. rewrite replicate_length. iSteps.
     iApply big_sepL_intro. iIntros "%k %_v" ((-> & Hk)%lookup_replicate). iSteps.
@@ -3105,8 +3605,8 @@ Section zoo_G.
     wp_smart_apply assume_spec' as "%Hsz".
     wp_smart_apply (chunk_make_spec with "[//]") as "%l (Hmodel & _)".
     rewrite Z.add_1_l Z2Nat.inj_succ //.
-    iDestruct (chunk_model_cons with "Hmodel") as "(Hsz & Hmodel)".
-    iMod (pointsto_persist with "Hsz") as "#Hsz".
+    iDestruct (chunk_model_cons with "Hmodel") as "(Hhdr & Hmodel)".
+    iMod (pointsto_persist with "Hhdr") as "#Hhdr".
     wp_smart_apply (chunk_applyi_spec_disentangled (λ _, τ) with "[$Hmodel]"); rewrite ?replicate_length; [lia | iSteps |].
     iIntros "%vs (%Hvs & Hmodel & #Hτ)".
     wp_pures.
@@ -3455,7 +3955,7 @@ Section zoo_G.
     wp_rec. rewrite {2}/array_data.
     wp_smart_apply (array_size_type with "Ht") as "_".
     repeat (wp_smart_apply assume_spec' as "%").
-    wp_smart_apply (array_make_spec with "[//]") as "%t' (%l' & -> & #Hsz' & Hdata')"; first done.
+    wp_smart_apply (array_make_spec with "[//]") as "%t' (%l' & -> & #Hhdr' & Hdata')"; first done.
     wp_smart_apply (array_data_type with "Ht") as "%data Hdata".
     iDestruct (itype_chunk_shift i with "Hdata") as "Hdata"; first lia.
     iDestruct (itype_chunk_le (Z.to_nat n) with "Hdata") as "Hdata"; first lia.
@@ -3621,15 +4121,19 @@ Section zoo_G.
   Qed.
 End zoo_G.
 
+#[global] Opaque array_unsafe_alloc.
+#[global] Opaque array_alloc.
 #[global] Opaque array_create.
-#[global] Opaque array_make.
-#[global] Opaque array_initi.
-#[global] Opaque array_init.
 #[global] Opaque array_size.
 #[global] Opaque array_unsafe_get.
 #[global] Opaque array_get.
 #[global] Opaque array_unsafe_set.
 #[global] Opaque array_set.
+#[global] Opaque array_unsafe_fill_slice.
+#[global] Opaque array_fill_slice.
+#[global] Opaque array_fill.
+#[global] Opaque array_unsafe_make.
+#[global] Opaque array_make.
 #[global] Opaque array_foldli.
 #[global] Opaque array_foldl.
 #[global] Opaque array_foldri.
@@ -3638,22 +4142,34 @@ End zoo_G.
 #[global] Opaque array_iter.
 #[global] Opaque array_applyi.
 #[global] Opaque array_apply.
-#[global] Opaque array_blit.
+#[global] Opaque array_unsafe_initi.
+#[global] Opaque array_initi.
+#[global] Opaque array_unsafe_init.
+#[global] Opaque array_init.
+#[global] Opaque array_mapi.
+#[global] Opaque array_map.
+#[global] Opaque array_unsafe_copy_slice.
+#[global] Opaque array_copy_slice.
+#[global] Opaque array_unsafe_copy.
 #[global] Opaque array_copy.
+#[global] Opaque array_unsafe_grow.
 #[global] Opaque array_grow.
+#[global] Opaque array_unsafe_sub.
 #[global] Opaque array_sub.
+#[global] Opaque array_unsafe_shrink.
 #[global] Opaque array_shrink.
 #[global] Opaque array_clone.
-#[global] Opaque array_fill_slice.
-#[global] Opaque array_fill.
+#[global] Opaque array_unsafe_cget.
 #[global] Opaque array_cget.
+#[global] Opaque array_unsafe_cset.
 #[global] Opaque array_cset.
-#[global] Opaque array_cblit.
+#[global] Opaque array_unsafe_ccopy_slice.
+#[global] Opaque array_ccopy_slice.
+#[global] Opaque array_unsafe_ccopy.
 #[global] Opaque array_ccopy.
 
 #[global] Opaque array_inv.
 #[global] Opaque array_slice.
 #[global] Opaque array_model.
-#[global] Opaque array_span.
 #[global] Opaque array_cslice.
 #[global] Opaque itype_array.
