theories/common/option.v
@@ -1,0 +1,14 @@
+From stdpp Require Export
+  option.
+
+From zoo Require Import
+  prelude.
+From zoo Require Import
+  options.
+
+Lemma from_option_default {A B} (f : A → B) x o :
+  from_option f (f x) o = f (default x o).
+Proof.
+  destruct o; done.
+Qed.
+
